Include all abstract state transitions in the formal model (#77)
* System transition: IC Management Canister: Canister creation [DONE]

* System transition: IC Management Canister: Changing settings [DONE]

* System transition: IC Management Canister: Canister status [DONE]

* refactoring

* System transition: IC Management Canister: Code installation [DONE]

* System transition: IC Management Canister: Code upgrade [DONE]

* System transition: IC Management Canister: Code uninstallation [DONE]

* System transition: IC Management Canister: Canister deletion [DONE]

* System transition: IC Management Canister: Depositing cycles [DONE]

* System transition: IC Management Canister: Random numbers [DONE]

* System transition: IC Management Canister: Starting a canister [DONE]

* System transition: IC Management Canister: Stopping a canister [DONE]

* System transition: Callback invocation [DONE]

* System transition: Respond to user request [DONE]

* System transition: Request clean up [DONE]

* System transition: Time progressing and cycle consumption [DONE]

* drop MAX_CANISTER_BALANCE

* System transition: Canister out of cycles [DONE]

* state machine

* System transition: IC Management Canister: Canister creation with cycles [DONE]

* System transition: IC Management Canister: Top up canister [DONE]

* export_code

* refactoring

* typo

* System transition: API Request submission [DONE]

* sync formal model and textual spec

* introduce type_synonym method_name

* fix freezing_threshold in canister creation

* typo

* add uninstall_code to accepted ingress message method names

* fix and prove invariants

* sync text with formal model

* typos

Co-authored-by: Martin Raszyk <martin.raszyk@dfinity.org>

theories/IC.thy
@@ -2,6 +2,11 @@ theory IC
   imports "HOL-Library.AList"
 begin
 
+(* General helper lemmas *)
+
+lemma in_set_updD: "x \<in> set (xs[n := z]) \<Longrightarrow> x \<in> set xs \<or> x = z"
+  by (meson insert_iff set_update_subset_insert subsetD)
+
 (* Partial maps *)
 
 typedef ('a, 'b) list_map = "{f :: ('a \<times> 'b) list. distinct (map fst f)}"
@@ -9,11 +14,22 @@ typedef ('a, 'b) list_map = "{f :: ('a \<times> 'b) list. distinct (map fst f)}"
 
 setup_lifting type_definition_list_map
 
+lift_bnf (dead 'k, set: 'v) list_map [wits: "[] :: ('k \<times> 'v) list"] for map: map rel: rel
+  by auto
+
+hide_const (open) map set rel
+
 lift_definition list_map_dom :: "('a, 'b) list_map \<Rightarrow> 'a set" is
   "set \<circ> map fst" .
 
-lift_definition list_map_vals :: "('a, 'b) list_map \<Rightarrow> 'b set" is
+lift_definition list_map_vals :: "('a, 'b) list_map \<Rightarrow> 'b list" is
+  "map snd" .
+
+lift_definition list_map_range :: "('a, 'b) list_map \<Rightarrow> 'b set" is
   "set \<circ> map snd" .
+
+lemma in_set_map_filter_vals: "z \<in> set (List.map_filter g (list_map_vals f)) \<Longrightarrow> \<exists>w \<in> list_map_range f. g w = Some z"
+  by transfer (force simp: List.map_filter_def)
 
 lift_definition list_map_sum_vals :: "('b \<Rightarrow> nat) \<Rightarrow> ('a, 'b) list_map \<Rightarrow> nat" is
   "\<lambda>g. sum_list \<circ> (map (g \<circ> snd))" .
@@ -21,19 +37,89 @@ lift_definition list_map_sum_vals :: "('b \<Rightarrow> nat) \<Rightarrow> ('a, 
 lift_definition list_map_get :: "('a, 'b) list_map \<Rightarrow> 'a \<Rightarrow> 'b option" is
   "map_of" .
 
+lemma list_map_get_dom[dest]: "x \<in> list_map_dom f \<Longrightarrow> list_map_get f x = None \<Longrightarrow> False"
+  by transfer auto
+
+lemma list_map_get_range: "list_map_get f x = Some y \<Longrightarrow> y \<in> list_map_range f"
+  by transfer force
+
 lift_definition list_map_set :: "('a, 'b) list_map \<Rightarrow> 'a \<Rightarrow> 'b \<Rightarrow> ('a, 'b) list_map" is
   "\<lambda>f x y. AList.update x y f"
   by (rule distinct_update)
+
+lemma list_map_get_set: "list_map_get (list_map_set f x y) z = (if x = z then Some y else list_map_get f z)"
+  by transfer (auto simp add: update_Some_unfold update_conv)
+
+lemma list_map_dom_set[simp]: "list_map_dom (list_map_set f x y) = list_map_dom f \<union> {x}"
+  by transfer (auto simp add: dom_update)
+
+lemma list_map_range_setD: "z \<in> list_map_range (list_map_set f x y) \<Longrightarrow> z \<in> list_map_range f \<or> z = y"
+  apply transfer
+  apply auto
+  apply (metis distinct_update image_iff map_of_eq_Some_iff snd_eqD update_Some_unfold)
+  done
 
 lift_definition list_map_del :: "('a, 'b) list_map \<Rightarrow> 'a \<Rightarrow> ('a, 'b) list_map" is
   "\<lambda>f x. AList.delete x f"
   by (rule distinct_delete)
 
+lemma list_map_get_del: "list_map_get (list_map_del f x) z = (if x = z then None else list_map_get f z)"
+  by transfer (auto simp add: delete_conv')
+
+lemma list_map_dom_del[simp]: "list_map_dom (list_map_del f x) = list_map_dom f - {x}"
+  by transfer (simp add: delete_keys)
+
+lemma list_map_range_del: "z \<in> list_map_range (list_map_del f x) \<Longrightarrow> z \<in> list_map_range f"
+  apply transfer
+  apply auto
+  apply (metis Some_eq_map_of_iff delete_notin_dom distinct_delete fst_eqD imageI map_of_delete snd_eqD)
+  done
+
 lift_definition list_map_empty :: "('a, 'b) list_map" is "[]"
   by auto
 
+lemma list_map_get_empty[simp]: "list_map_get list_map_empty x = None"
+  by transfer auto
+
 lemma list_map_empty_dom[simp]: "list_map_dom list_map_empty = {}"
   by transfer auto
+
+lemma list_map_empty_range[simp]: "list_map_range list_map_empty = {}"
+  by transfer auto
+
+lift_definition list_map_init :: "('a \<times> 'b) list \<Rightarrow> ('a, 'b) list_map" is
+  "\<lambda>xys. AList.updates (map fst xys) (map snd xys) []"
+  using distinct_updates
+  by force
+
+lift_definition list_map_map :: "('b \<Rightarrow> 'c) \<Rightarrow> ('a, 'b) list_map \<Rightarrow> ('a, 'c) list_map" is
+  "\<lambda>f xs. map (\<lambda>(k, v). (k, f v)) xs"
+  by (auto simp: comp_def case_prod_beta)
+
+lemma list_map_dom_map_map[simp]: "list_map_dom (list_map_map g f) = list_map_dom f"
+  by transfer force
+
+lemma list_map_range_map_map[simp]: "list_map_range (list_map_map g f) = g ` list_map_range f"
+  by transfer force
+
+lemma list_map_sum_vals_split: "(\<And>ctxt. ctxt \<in> list_map_range xs \<Longrightarrow> f (g ctxt) \<le> f ctxt) \<Longrightarrow> list_map_sum_vals f xs =
+  list_map_sum_vals id
+    (list_map_map (\<lambda>ctxt. if P ctxt then f ctxt - f (g ctxt) else 0) xs) +
+  list_map_sum_vals f
+    (list_map_map (\<lambda>ctxt. if P ctxt then g ctxt else ctxt) xs)"
+  apply (transfer fixing: f g P)
+  subgoal for xs
+    by (induction xs) auto
+  done
+
+lemma list_map_sum_vals_filter:
+  assumes "\<And>b. b \<in> list_map_range xs \<Longrightarrow> P b = None \<Longrightarrow> f b = 0" "\<And>b y. b \<in> list_map_range xs \<Longrightarrow> P b = Some y \<Longrightarrow> f b = g y"
+  shows "list_map_sum_vals id (list_map_map f xs) = sum_list (map g (List.map_filter P (list_map_vals xs)))"
+  using assms
+  apply (transfer fixing: f g P)
+  subgoal for xs
+    by (induction xs) (auto simp: List.map_filter_def)
+  done
 
 lemma list_map_sum_in_ge_aux:
   fixes g :: "'a \<Rightarrow> nat"
@@ -83,12 +169,15 @@ lemma list_map_del_sum: "list_map_get f x = Some y \<Longrightarrow> list_map_su
 
 (* Abstract canisters *)
 
+type_synonym 's method_name = 's
+
 type_synonym 'b arg = 'b
+type_synonym 'p caller_id = 'p
 
 type_synonym timestamp = nat
 datatype status = Running | Stopping | Stopped
 record ('b) env =
-  env_time :: timestamp
+  time :: timestamp
   balance :: nat
   freezing_limit :: nat
   certificate :: "'b option"
@@ -100,15 +189,15 @@ datatype ('b, 's) response =
 | Reject reject_code 's
 record ('p, 'canid, 's, 'b, 'c) method_call =
   callee :: 'canid
-  method_name :: 's
+  method_name :: "'s method_name"
   arg :: 'b
   transferred_cycles :: nat
   callback :: 'c
 
-record trap_return = cycles_used :: nat
 record 'x cycles_return =
   return :: 'x
   cycles_used :: nat
+type_synonym trap_return = "unit cycles_return"
 record ('w, 'p, 'canid, 's, 'b, 'c) update_return =
   new_state :: 'w
   new_calls :: "('p, 'canid, 's, 'b, 'c) method_call list"
@@ -131,14 +220,14 @@ type_synonym refunded_cycles = nat
 
 datatype inspect_method_result = Accept | Reject
 record ('p, 'canid, 'b, 'w, 'sm, 'c, 's) canister_module_rec =
-  init :: "'canid \<times> 'b arg \<times> 'p \<times> 'b env \<Rightarrow> trap_return + 'w cycles_return"
+  init :: "'canid \<times> 'b arg \<times> 'p caller_id \<times> 'b env \<Rightarrow> trap_return + 'w cycles_return"
   pre_upgrade :: "'w \<times> 'p \<times> 'b env \<Rightarrow> trap_return + 'sm cycles_return"
-  post_upgrade :: "'canid \<times> 'sm \<times> 'b arg \<times> 'p \<times> 'b env \<Rightarrow> trap_return + 'w cycles_return"
-  update_methods :: "('s, ('b arg \<times> 'p \<times> 'b env \<times> available_cycles) \<Rightarrow> ('w, 'p, 'canid, 's, 'b, 'c) update_func) list_map"
-  query_methods :: "('s, ('b arg \<times> 'p \<times> 'b env) \<Rightarrow> ('w, 'b, 's) query_func) list_map"
+  post_upgrade :: "'canid \<times> 'sm \<times> 'b arg \<times> 'p caller_id \<times> 'b env \<Rightarrow> trap_return + 'w cycles_return"
+  update_methods :: "('s method_name, ('b arg \<times> 'p caller_id \<times> 'b env \<times> available_cycles) \<Rightarrow> ('w, 'p, 'canid, 's, 'b, 'c) update_func) list_map"
+  query_methods :: "('s method_name, ('b arg \<times> 'p caller_id \<times> 'b env) \<Rightarrow> ('w, 'b, 's) query_func) list_map"
   heartbeat :: "'b env \<Rightarrow> 'w heartbeat_func"
   callbacks :: "('c \<times> ('b, 's) response \<times> refunded_cycles \<times> 'b env \<times> available_cycles) \<Rightarrow> ('w, 'p, 'canid, 's, 'b, 'c) update_func"
-  inspect_message :: "('s \<times> 'w \<times> 'b arg \<times> 'p \<times> 'b env) \<Rightarrow> trap_return + inspect_method_result cycles_return"
+  inspect_message :: "('s method_name \<times> 'w \<times> 'b arg \<times> 'p caller_id \<times> 'b env) \<Rightarrow> trap_return + inspect_method_result cycles_return"
 typedef ('p, 'canid, 'b, 'w, 'sm, 'c, 's) canister_module =
   "{m :: ('p, 'canid, 'b, 'w, 'sm, 'c, 's) canister_module_rec. list_map_dom (update_methods m) \<inter> list_map_dom (query_methods m) = {}}"
   by (auto intro: exI[of _ "\<lparr>init = undefined, pre_upgrade = undefined, post_upgrade = undefined,
@@ -147,17 +236,18 @@ typedef ('p, 'canid, 'b, 'w, 'sm, 'c, 's) canister_module =
 
 setup_lifting type_definition_canister_module
 
+lift_definition canister_module_init :: "('p, 'canid, 'b, 'w, 'sm, 'c, 's) canister_module \<Rightarrow> 'canid \<times> 'b arg \<times> 'p \<times> 'b env \<Rightarrow> trap_return + 'w cycles_return" is "init" .
+lift_definition canister_module_pre_upgrade :: "('p, 'canid, 'b, 'w, 'sm, 'c, 's) canister_module \<Rightarrow> 'w \<times> 'p \<times> 'b env \<Rightarrow> trap_return + 'sm cycles_return" is pre_upgrade .
+lift_definition canister_module_post_upgrade :: "('p, 'canid, 'b, 'w, 'sm, 'c, 's) canister_module \<Rightarrow> 'canid \<times> 'sm \<times> 'b arg \<times> 'p \<times> 'b env \<Rightarrow> trap_return + 'w cycles_return" is post_upgrade .
+lift_definition canister_module_update_methods :: "('p, 'canid, 'b, 'w, 'sm, 'c, 's) canister_module \<Rightarrow> ('s, ('b arg \<times> 'p \<times> 'b env \<times> available_cycles) \<Rightarrow> ('w, 'p, 'canid, 's, 'b, 'c) update_func) list_map" is update_methods .
+lift_definition canister_module_query_methods :: "('p, 'canid, 'b, 'w, 'sm, 'c, 's) canister_module \<Rightarrow> ('s, ('b arg \<times> 'p \<times> 'b env) \<Rightarrow> ('w, 'b, 's) query_func) list_map" is query_methods .
+lift_definition canister_module_heartbeat :: "('p, 'canid, 'b, 'w, 'sm, 'c, 's) canister_module \<Rightarrow> 'b env \<Rightarrow> 'w heartbeat_func" is heartbeat .
+lift_definition canister_module_callbacks :: "('p, 'canid, 'b, 'w, 'sm, 'c, 's) canister_module \<Rightarrow> ('c \<times> ('b, 's) response \<times> refunded_cycles \<times> 'b env \<times> available_cycles) \<Rightarrow> ('w, 'p, 'canid, 's, 'b, 'c) update_func" is callbacks .
+lift_definition canister_module_inspect_message :: "('p, 'canid, 'b, 'w, 'sm, 'c, 's) canister_module \<Rightarrow> ('s \<times> 'w \<times> 'b arg \<times> 'p \<times> 'b env) \<Rightarrow> trap_return + inspect_method_result cycles_return" is inspect_message .
+
 lift_definition dispatch_method :: "'s \<Rightarrow> ('p, 'canid, 'b, 'w, 'sm, 'c, 's) canister_module \<Rightarrow>
-  ((('b arg \<times> 'p \<times> 'b env \<times> available_cycles) \<Rightarrow> ('w, 'p, 'canid, 's, 'b, 'c) update_func) +
-   (('b arg \<times> 'p \<times> 'b env) \<Rightarrow> ('w, 'b, 's) query_func)) option" is
-  "\<lambda>f m. case list_map_get (update_methods m) f of Some f' \<Rightarrow> None | None \<Rightarrow> (case list_map_get (query_methods m) f of Some f' \<Rightarrow> None | None \<Rightarrow> None)" .
-
-lift_definition canister_module_callbacks :: "('p, 'canid, 'b, 'w, 'sm, 'c, 's) canister_module \<Rightarrow>
-  ('c \<times> ('b, 's) response \<times> refunded_cycles \<times> 'b env \<times> available_cycles) \<Rightarrow> ('w, 'p, 'canid, 's, 'b, 'c) update_func" is
-  callbacks .
-
-lift_definition canister_module_heartbeat :: "('p, 'canid, 'b, 'w, 'sm, 'c, 's) canister_module \<Rightarrow> 'b env \<Rightarrow> 'w heartbeat_func" is
-  heartbeat .
+  ((('b arg \<times> 'p \<times> 'b env \<times> available_cycles) \<Rightarrow> ('w, 'p, 'canid, 's, 'b, 'c) update_func) + (('b arg \<times> 'p \<times> 'b env) \<Rightarrow> ('w, 'b, 's) query_func)) option" is
+  "\<lambda>f m. case list_map_get (update_methods m) f of Some f' \<Rightarrow> Some (Inl f') | None \<Rightarrow> (case list_map_get (query_methods m) f of Some f' \<Rightarrow> Some (Inr f') | None \<Rightarrow> None)" .
 
 (* Call contexts *)
 
@@ -185,26 +275,26 @@ typedef ('p, 'uid, 'canid, 'b, 's, 'c, 'cid) call_ctxt = "{ctxt :: ('p, 'uid, 'c
 
 setup_lifting type_definition_call_ctxt
 
-lift_definition call_ctxt_origin :: "('p, 'uid, 'canid, 'b, 's, 'c, 'cid) call_ctxt \<Rightarrow> ('b, 'p, 'uid, 'canid, 's, 'c, 'cid) call_origin" is
-  "\<lambda>ctxt. origin ctxt" .
+lift_definition call_ctxt_canister :: "('p, 'uid, 'canid, 'b, 's, 'c, 'cid) call_ctxt \<Rightarrow> 'canid" is "canister" .
+lift_definition call_ctxt_origin :: "('p, 'uid, 'canid, 'b, 's, 'c, 'cid) call_ctxt \<Rightarrow> ('b, 'p, 'uid, 'canid, 's, 'c, 'cid) call_origin" is "origin" .
+lift_definition call_ctxt_needs_to_respond :: "('p, 'uid, 'canid, 'b, 's, 'c, 'cid) call_ctxt \<Rightarrow> bool" is needs_to_respond .
+lift_definition call_ctxt_deleted :: "('p, 'uid, 'canid, 'b, 's, 'c, 'cid) call_ctxt \<Rightarrow> bool" is deleted .
+lift_definition call_ctxt_available_cycles :: "('p, 'uid, 'canid, 'b, 's, 'c, 'cid) call_ctxt \<Rightarrow> nat" is available_cycles .
 
-lift_definition call_ctxt_needs_to_respond :: "('p, 'uid, 'canid, 'b, 's, 'c, 'cid) call_ctxt \<Rightarrow> bool" is
-  "\<lambda>ctxt. needs_to_respond ctxt" .
-
-lift_definition call_ctxt_available_cycles :: "('p, 'uid, 'canid, 'b, 's, 'c, 'cid) call_ctxt \<Rightarrow> nat" is
-  "\<lambda>ctxt. available_cycles ctxt" .
-
-lemma call_ctxt_inv: "\<not>call_ctxt_needs_to_respond x2 \<Longrightarrow> call_ctxt_available_cycles x2 = 0"
+lemma call_ctxt_not_needs_to_respond_available_cycles: "\<not>call_ctxt_needs_to_respond x2 \<Longrightarrow> call_ctxt_available_cycles x2 = 0"
   by transfer auto
 
 lift_definition call_ctxt_respond :: "('p, 'uid, 'canid, 'b, 's, 'c, 'cid) call_ctxt \<Rightarrow> ('p, 'uid, 'canid, 'b, 's, 'c, 'cid) call_ctxt" is
-  "\<lambda>ctxt. ctxt\<lparr>available_cycles := 0, needs_to_respond := False\<rparr>"
+  "\<lambda>ctxt. ctxt\<lparr>needs_to_respond := False, available_cycles := 0\<rparr>"
   by auto
 
-lemma call_ctxt_respond_available_cycles[simp]: "call_ctxt_available_cycles (call_ctxt_respond ctxt) = 0"
+lemma call_ctxt_respond_origin[simp]: "call_ctxt_origin (call_ctxt_respond ctxt) = call_ctxt_origin ctxt"
   by transfer auto
 
 lemma call_ctxt_respond_needs_to_respond[dest]: "call_ctxt_needs_to_respond (call_ctxt_respond ctxt) \<Longrightarrow> False"
+  by transfer auto
+
+lemma call_ctxt_respond_available_cycles[simp]: "call_ctxt_available_cycles (call_ctxt_respond ctxt) = 0"
   by transfer auto
 
 lift_definition call_ctxt_deduct_cycles :: "nat \<Rightarrow> ('p, 'uid, 'canid, 'b, 's, 'c, 'cid) call_ctxt \<Rightarrow> ('p, 'uid, 'canid, 'b, 's, 'c, 'cid) call_ctxt" is
@@ -220,12 +310,19 @@ lemma call_ctxt_deduct_cycles_needs_to_respond[simp]: "call_ctxt_needs_to_respon
 lemma call_ctxt_deduct_cycles_available_cycles[simp]: "call_ctxt_available_cycles (call_ctxt_deduct_cycles n ctxt) = call_ctxt_available_cycles ctxt - n"
   by transfer auto
 
+lift_definition call_ctxt_delete :: "('p, 'uid, 'canid, 'b, 's, 'c, 'cid) call_ctxt \<Rightarrow> ('p, 'uid, 'canid, 'b, 's, 'c, 'cid) call_ctxt" is
+  "\<lambda>ctxt. ctxt\<lparr>deleted := True, needs_to_respond := False, available_cycles := 0\<rparr>"
+  by auto
+
+lemma call_ctxt_delete_needs_to_respond[simp]: "call_ctxt_needs_to_respond (call_ctxt_delete ctxt) = False"
+  by transfer auto
+
 (* Calls and Messages *)
 
 datatype 'canid queue_origin = System | Canister 'canid
 datatype 'canid queue = Unordered | Queue "'canid queue_origin" 'canid
 datatype ('s, 'p, 'b, 'c) entry_point =
-  Public_method "'s" "'p" "'b"
+  Public_method "'s method_name" "'p" "'b"
 | Callback "'c" "('b, 's) response" "refunded_cycles"
 | Heartbeat
 
@@ -250,11 +347,21 @@ record ('b, 'uid, 'canid, 's) CanisterQuery =
   method_name :: 's
   arg :: 'b
 type_synonym ('b, 'uid, 'canid, 's) APIReadRequest = "('b, 'uid) StateRead + ('b, 'uid, 'canid, 's) CanisterQuery"
-record ('b, 'p, 'uid, 'canid, 's, 'pk, 'sig, 'sd) envelope =
+
+record ('p, 'canid, 'pk, 'sig) delegation =
+  pubkey :: 'pk
+  targets :: "'canid list option"
+  senders :: "'p list option"
+  expiration :: timestamp
+record ('p, 'canid, 'pk, 'sig) signed_delegation =
+  delegation :: "('p, 'canid, 'pk, 'sig) delegation"
+  signature :: "'sig"
+
+record ('b, 'p, 'uid, 'canid, 's, 'pk, 'sig) envelope =
   content :: "('b, 'p, 'uid, 'canid, 's) request + ('b, 'uid, 'canid, 's) APIReadRequest"
   sender_pubkey :: "'pk option"
   sender_sig :: "'sig option"
-  sender_delegation :: 'sd
+  sender_delegation :: "('p, 'canid, 'pk, 'sig) delegation list"
 
 datatype ('b, 's) request_status = Received | Processing | Rejected reject_code 's | Replied 'b | Done
 
@@ -282,20 +389,163 @@ record ('p, 'uid, 'canid, 'b, 'w, 'sm, 'c, 's, 'cid, 'pk) ic =
   messages :: "('b, 'p, 'uid, 'canid, 's, 'c, 'cid) message list"
   root_key :: 'pk
 
+fun simple_status :: "('b, 'p, 'uid, 'canid, 's, 'c, 'cid) can_status \<Rightarrow> status" where
+  "simple_status can_status.Running = status.Running"
+| "simple_status (can_status.Stopping _) = status.Stopping"
+| "simple_status can_status.Stopped = status.Stopped"
+
+(* Initial state *)
+
+definition initial_ic :: "nat \<Rightarrow> 'pk \<Rightarrow> ('p, 'uid, 'canid, 'b, 'w, 'sm, 'c, 's, 'cid, 'pk) ic" where
+  "initial_ic t pk = \<lparr>requests = list_map_empty,
+    canisters = list_map_empty,
+    controllers = list_map_empty,
+    freezing_threshold = list_map_empty,
+    canister_status = list_map_empty,
+    time = list_map_empty,
+    balances = list_map_empty,
+    certified_data = list_map_empty,
+    system_time = t,
+    call_contexts = list_map_empty,
+    messages = [],
+    root_key = pk\<rparr>"
+
+(* Invariants *)
+
+definition ic_can_status_inv :: "('b, 'p, 'uid, 'canid, 's, 'c, 'cid) can_status set \<Rightarrow> 'cid set \<Rightarrow> bool" where
+  "ic_can_status_inv st c = (\<forall>can_status \<in> st.
+    case can_status of Stopping os \<Rightarrow> \<forall>(orig, cycles) \<in> set os. (case orig of
+      From_canister ctxt_id _ \<Rightarrow> ctxt_id \<in> c
+      | _ \<Rightarrow> True)
+    | _ \<Rightarrow> True)"
+
+lemma ic_can_status_inv_mono1: "ic_can_status_inv x y \<Longrightarrow>
+  z \<subseteq> x \<union> {can_status.Running, can_status.Stopped} \<Longrightarrow>
+  ic_can_status_inv z y"
+  by (fastforce simp: ic_can_status_inv_def split: can_status.splits call_origin.splits)
+
+lemma ic_can_status_inv_mono2: "ic_can_status_inv x y \<Longrightarrow>
+  y \<subseteq> z \<Longrightarrow>
+  ic_can_status_inv x z"
+  by (force simp: ic_can_status_inv_def split: can_status.splits call_origin.splits)
+
+lemma ic_can_status_inv_stopping: "ic_can_status_inv x y \<Longrightarrow>
+  (\<And>ctxt_id c. os = From_canister ctxt_id c \<Longrightarrow> ctxt_id \<in> y) \<Longrightarrow>
+  z \<subseteq> x \<union> {can_status.Stopping [(os, cyc)]} \<Longrightarrow>
+  ic_can_status_inv z y"
+  by (fastforce simp: ic_can_status_inv_def split: can_status.splits call_origin.splits)
+
+lemma ic_can_status_inv_stopping_app: "ic_can_status_inv x y \<Longrightarrow>
+  can_status.Stopping w \<in> x \<Longrightarrow>
+  (\<And>ctxt_id c. os = From_canister ctxt_id c \<Longrightarrow> ctxt_id \<in> y) \<Longrightarrow>
+  z \<subseteq> x \<union> {can_status.Stopping (w @ [(os, cyc)])} \<Longrightarrow>
+  ic_can_status_inv z y"
+  by (force simp: ic_can_status_inv_def split: can_status.splits call_origin.splits dest!: subsetD[where ?A=z])
+
+lemma ic_can_status_inv_del: "ic_can_status_inv x z \<Longrightarrow>
+  (\<And>os other_ctxt_id c cyc. Stopping os \<in> x \<Longrightarrow> (From_canister other_ctxt_id c, cyc) \<in> set os \<Longrightarrow> ctxt_id \<noteq> other_ctxt_id) \<Longrightarrow>
+  ic_can_status_inv x (z - {ctxt_id})"
+  by (fastforce simp: ic_can_status_inv_def split: can_status.splits call_origin.splits)
+
+definition ic_inv :: "('p, 'uid, 'canid, 'b, 'w, 'sm, 'c, 's, 'cid, 'pk) ic \<Rightarrow> bool" where
+  "ic_inv S = ((\<forall>msg \<in> set (messages S). case msg of
+    Call_message (From_canister ctxt_id _) _ _ _ _ _ _ \<Rightarrow> ctxt_id \<in> list_map_dom (call_contexts S)
+  | Response_message (From_canister ctxt_id _) _ _ \<Rightarrow> ctxt_id \<in> list_map_dom (call_contexts S)
+  | _ \<Rightarrow> True) \<and>
+  (\<forall>ctxt \<in> list_map_range (call_contexts S). call_ctxt_needs_to_respond ctxt \<longrightarrow>
+    (case call_ctxt_origin ctxt of From_canister ctxt_id _ \<Rightarrow> ctxt_id \<in> list_map_dom (call_contexts S)
+    | _ \<Rightarrow> True)) \<and>
+  ic_can_status_inv (list_map_range (canister_status S)) (list_map_dom (call_contexts S)))"
+
+lemma ic_initial_inv: "ic_inv (initial_ic t pk)"
+  by (auto simp: ic_inv_def ic_can_status_inv_def initial_ic_def split: call_origin.splits)
+
+(* Candid *)
+
+datatype ('s, 'b, 'p) candid =
+    Candid_nat nat
+  | Candid_text 's
+  | Candid_blob (candid_unwrap_blob: 'b)
+  | Candid_opt "('s, 'b, 'p) candid"
+  | Candid_vec "('s, 'b, 'p) candid list"
+  | Candid_record "('s, ('s, 'b, 'p) candid) list_map"
+  | Candid_null
+  | Candid_empty
+
+fun candid_is_blob :: "('s, 'b, 'p) candid \<Rightarrow> bool" where
+  "candid_is_blob (Candid_blob b) = True"
+| "candid_is_blob _ = False"
+
+fun candid_lookup :: "('s, 'b, 'p) candid \<Rightarrow> 's \<Rightarrow> ('s, 'b, 'p) candid option" where
+  "candid_lookup (Candid_record m) s = list_map_get m s"
+| "candid_lookup _ _ = None"
+
 (* State transitions *)
 
 context fixes
   CANISTER_ERROR :: reject_code
+  and CANISTER_REJECT :: reject_code
   and SYS_FATAL :: reject_code
   and SYS_TRANSIENT :: reject_code
   and MAX_CYCLES_PER_MESSAGE :: nat
   and MAX_CYCLES_PER_RESPONSE :: nat
   and MAX_CANISTER_BALANCE :: nat
-  and ic_freezing_limit :: "('p, 'uid, 'canid, 'b, 'w, 'sm, 'c, 's, 'cid, 'pk) ic \<Rightarrow> 'canid \<Rightarrow> nat"
+  and ic_idle_cycles_burned_rate :: "('p :: linorder, 'uid, 'canid, 'b, 'w, 'sm, 'c, 's, 'cid, 'pk) ic \<Rightarrow> 'canid \<Rightarrow> nat"
+  and blob_length :: "'b \<Rightarrow> nat"
+  and sha_256 :: "'b \<Rightarrow> 'b"
+  and ic_principal :: 'canid
+  and blob_of_candid :: "('s, 'b, 'p) candid \<Rightarrow> 'b"
+  and parse_candid :: "'b \<Rightarrow> ('s, 'b, 'p) candid option"
+  and parse_principal :: "'b \<Rightarrow> 'p option"
+  and blob_of_principal :: "'p \<Rightarrow> 'b"
+  and empty_blob :: 'b
+  and is_system_assigned :: "'p \<Rightarrow> bool"
   and encode_string :: "string \<Rightarrow> 's"
   and principal_of_uid :: "'uid \<Rightarrow> 'p"
   and principal_of_canid :: "'canid \<Rightarrow> 'p"
+  and canid_of_principal :: "'p \<Rightarrow> 'canid option"
+  and parse_wasm_mod :: "'b \<Rightarrow> ('p, 'canid, 'b, 'w, 'sm, 'c, 's) canister_module option"
+  and parse_public_custom_sections :: "'b \<Rightarrow> ('s, 'b) list_map option"
+  and parse_private_custom_sections :: "'b \<Rightarrow> ('s, 'b) list_map option"
+  and verify_envelope :: "('b, 'p, 'uid, 'canid, 's, 'pk, 'sig) envelope \<Rightarrow> 'p \<Rightarrow> nat \<Rightarrow> 'p set" (* TODO *)
+  and principal_list_of_set :: "'p set \<Rightarrow> 'p list"
 begin
+
+(* Type conversion functions *)
+
+definition canid_of_blob :: "'b \<Rightarrow> 'canid option" where
+  "canid_of_blob b = (case parse_principal b of Some p \<Rightarrow> canid_of_principal p | _ \<Rightarrow> None)"
+
+definition blob_of_canid :: "'canid \<Rightarrow> 'b" where
+  "blob_of_canid = blob_of_principal \<circ> principal_of_canid"
+
+(* Candid helper functions *)
+
+definition candid_nested_lookup :: "'b \<Rightarrow> 's list \<Rightarrow> ('s, 'b, 'p) candid option" where
+  "candid_nested_lookup b = foldl (\<lambda>c s. case c of Some c' \<Rightarrow> candid_lookup c' s | _ \<Rightarrow> None) (parse_candid b)"
+
+definition candid_parse_nat :: "'b \<Rightarrow> 's list \<Rightarrow> nat option" where
+  "candid_parse_nat b s = (case candid_nested_lookup b s of Some (Candid_nat n') \<Rightarrow> Some n' | _ \<Rightarrow> None)"
+
+definition candid_parse_text :: "'b \<Rightarrow> 's list \<Rightarrow> 's option" where
+  "candid_parse_text b s = (case candid_nested_lookup b s of Some (Candid_text t') \<Rightarrow> Some t' | _ \<Rightarrow> None)"
+
+definition candid_parse_blob :: "'b \<Rightarrow> 's list \<Rightarrow> 'b option" where
+  "candid_parse_blob b s = (case candid_nested_lookup b s of Some (Candid_blob b') \<Rightarrow> Some b' | _ \<Rightarrow> None)"
+
+definition candid_parse_cid :: "'b \<Rightarrow> 'canid option" where
+  "candid_parse_cid b = (case candid_parse_blob b [encode_string ''canister_id''] of Some b' \<Rightarrow> canid_of_blob b' | _ \<Rightarrow> None)"
+
+definition candid_parse_controllers :: "'b \<Rightarrow> 'p set option" where
+  "candid_parse_controllers b = (case candid_nested_lookup b [encode_string ''settings'', encode_string ''controllers''] of Some (Candid_vec xs) \<Rightarrow>
+    if (\<forall>c'' \<in> set xs. candid_is_blob c'' \<and> parse_principal (candid_unwrap_blob c'') \<noteq> None) then
+      Some (the ` parse_principal ` candid_unwrap_blob ` set xs)
+    else None | _ \<Rightarrow> None)"
+
+fun candid_of_status :: "status \<Rightarrow> ('s, 'b, 'p) candid" where
+  "candid_of_status status.Running = Candid_text (encode_string ''Running'')"
+| "candid_of_status status.Stopping = Candid_text (encode_string ''Stopping'')"
+| "candid_of_status status.Stopped = Candid_text (encode_string ''Stopped'')"
 
 (* Cycles *)
 
@@ -313,6 +563,10 @@ fun message_cycles :: "('b, 'p, 'uid, 'canid, 's, 'c, 'cid) message \<Rightarrow
 | "message_cycles (Func_message _ _ ep _) = cycles_reserved ep"
 | "message_cycles (Response_message orig _ ref_cycles) = carried_cycles orig + ref_cycles"
 
+fun status_cycles :: "('b, 'p, 'uid, 'canid, 's, 'c, 'cid) can_status \<Rightarrow> nat" where
+  "status_cycles (Stopping os) = sum_list (map (carried_cycles \<circ> fst) os) + sum_list (map snd os)"
+| "status_cycles _ = 0"
+
 lift_definition call_ctxt_carried_cycles :: "('p, 'uid, 'canid, 'b, 's, 'c, 'cid) call_ctxt \<Rightarrow> nat" is
   "\<lambda>ctxt. (if needs_to_respond ctxt
     then available_cycles ctxt + carried_cycles (origin ctxt)
@@ -325,12 +579,16 @@ lemma call_ctxt_carried_cycles: "call_ctxt_carried_cycles ctxt = (if call_ctxt_n
   then call_ctxt_available_cycles ctxt + carried_cycles (call_ctxt_origin ctxt) else 0)"
   by transfer auto
 
+lemma call_ctxt_delete_carried_cycles[simp]: "call_ctxt_carried_cycles (call_ctxt_delete ctxt) = 0"
+  by transfer auto
+
 definition total_cycles :: "('p, 'uid, 'canid, 'b, 'w, 'sm, 'c, 's, 'cid, 'pk) ic \<Rightarrow> nat" where
   "total_cycles ic = (
     let cycles_in_balances = list_map_sum_vals id (balances ic) in
     let cycles_in_messages = sum_list (map message_cycles (messages ic)) in
     let cycles_in_contexts = list_map_sum_vals call_ctxt_carried_cycles (call_contexts ic) in
-    cycles_in_balances + cycles_in_messages + cycles_in_contexts)"
+    let cycles_in_statuses = list_map_sum_vals status_cycles (canister_status ic) in
+    cycles_in_balances + cycles_in_messages + cycles_in_contexts + cycles_in_statuses)"
 
 (* Accessor functions *)
 
@@ -343,40 +601,141 @@ fun message_queue :: "('b, 'p, 'uid, 'canid, 's, 'c, 'cid) message \<Rightarrow>
 | "message_queue (Func_message _ _ _ q) = Some q"
 | "message_queue _ = None"
 
-(* Type conversion functions *)
+(* Effective canister IDs *)
 
-fun simple_status :: "('b, 'p, 'uid, 'canid, 's, 'c, 'cid) can_status \<Rightarrow> status" where
-  "simple_status can_status.Running = status.Running"
-| "simple_status (can_status.Stopping _) = status.Stopping"
-| "simple_status can_status.Stopped = status.Stopped"
+definition is_effective_canister_id :: "('b, 'p, 'uid, 'canid, 's) request \<Rightarrow> 'p \<Rightarrow> bool" where
+  "is_effective_canister_id r p = (if request.canister_id r = ic_principal then
+      (case candid_parse_cid (request.arg r) of Some cid \<Rightarrow> principal_of_canid cid = p
+      | _ \<Rightarrow> request.method_name r = encode_string ''provisional_create_canister_with_cycles'')
+    else principal_of_canid (request.canister_id r) = p)"
+
+lemma is_effective_canister_id_code[code_unfold]:
+  "(\<exists>p. is_effective_canister_id r p) = (if request.canister_id r = ic_principal then
+      (case candid_parse_cid (request.arg r) of Some cid \<Rightarrow> True
+      | _ \<Rightarrow> request.method_name r = encode_string ''provisional_create_canister_with_cycles'')
+    else True)"
+  by (auto simp: is_effective_canister_id_def split: option.splits)
 
 
 
 (* System transition: API Request submission [DONE] *)
 
-definition request_submission_pre :: "('b, 'p, 'uid, 'canid, 's, 'pk, 'sig, 'sd) envelope \<Rightarrow> ('p, 'uid, 'canid, 'b, 'w, 'sm, 'c, 's, 'cid, 'pk) ic \<Rightarrow> bool" where
-  "request_submission_pre E S = (case content E of Inl req \<Rightarrow> req \<notin> list_map_dom (requests S) | _ \<Rightarrow> False)"
+definition ic_freezing_limit :: "('p :: linorder, 'uid, 'canid, 'b, 'w, 'sm, 'c, 's, 'cid, 'pk) ic \<Rightarrow> 'canid \<Rightarrow> nat" where
+  "ic_freezing_limit S cid = ic_idle_cycles_burned_rate S cid * (the (list_map_get (freezing_threshold S) cid)) div (24 * 60 * 60)"
 
-definition request_submission_post :: "('b, 'p, 'uid, 'canid, 's, 'pk, 'sig, 'sd) envelope \<Rightarrow> ('p, 'uid, 'canid, 'b, 'w, 'sm, 'c, 's, 'cid, 'pk) ic \<Rightarrow> ('p, 'uid, 'canid, 'b, 'w, 'sm, 'c, 's, 'cid, 'pk) ic" where
-  "request_submission_post E S = S\<lparr>requests := list_map_set (requests S) (projl (content E)) Received\<rparr>"
+definition request_submission_pre :: "('b, 'p, 'uid, 'canid, 's, 'pk, 'sig) envelope \<Rightarrow> ('p, 'uid, 'canid, 'b, 'w, 'sm, 'c, 's, 'cid, 'pk) ic \<Rightarrow> bool" where
+  "request_submission_pre E S = (case content E of Inl req \<Rightarrow>
+    principal_of_canid (request.canister_id req) \<in> verify_envelope E (principal_of_uid (request.sender req)) (system_time S) \<and>
+    req \<notin> list_map_dom (requests S) \<and>
+    system_time S \<le> request.ingress_expiry req \<and>
+    (\<exists>ECID. is_effective_canister_id req ECID) \<and>
+    (
+      (
+        request.canister_id req = ic_principal \<and>
+        (case candid_parse_cid (request.arg req) of Some cid \<Rightarrow>
+          (case list_map_get (controllers S) cid of Some ctrls \<Rightarrow>
+            principal_of_uid (request.sender req) \<in> ctrls \<and>
+            request.method_name req \<in> {encode_string ''install_code'', encode_string ''uninstall_code'', encode_string ''update_settings'',
+              encode_string ''start_canister'', encode_string ''stop_canister'',
+              encode_string ''canister_status'', encode_string ''delete_canister'',
+              encode_string ''provisional_create_canister_with_cycles'', encode_string ''provisional_top_up_canister''}
+          | _ \<Rightarrow> False)
+        | _ \<Rightarrow> False)
+      )
+    \<or>
+      (
+        request.canister_id req \<noteq> ic_principal \<and>
+        (case (list_map_get (canisters S) (request.canister_id req), list_map_get (time S) (request.canister_id req), list_map_get (balances S) (request.canister_id req), list_map_get (canister_status S) (request.canister_id req)) of
+          (Some (Some can), Some t, Some bal, Some can_status) \<Rightarrow>
+          let env = \<lparr>env.time = t, balance = bal, freezing_limit = ic_freezing_limit S (request.canister_id req), certificate = None, status = simple_status can_status\<rparr> in
+          (case canister_module_inspect_message (module can) (request.method_name req, wasm_state can, request.arg req, principal_of_uid (request.sender req), env) of Inr ret \<Rightarrow>
+            cycles_return.return ret = Accept \<and> cycles_return.cycles_used ret \<le> bal
+          | _ \<Rightarrow> False)
+        | _ \<Rightarrow> False)
+      )
+    )
+  | _ \<Rightarrow> False)"
+
+definition request_submission_post :: "('b, 'p, 'uid, 'canid, 's, 'pk, 'sig) envelope \<Rightarrow> ('p, 'uid, 'canid, 'b, 'w, 'sm, 'c, 's, 'cid, 'pk) ic \<Rightarrow> ('p, 'uid, 'canid, 'b, 'w, 'sm, 'c, 's, 'cid, 'pk) ic" where
+  "request_submission_post E S = (
+    let req = projl (content E);
+    cid = request.canister_id req;
+    balances = (if cid \<noteq> ic_principal then
+      (case (list_map_get (canisters S) cid, list_map_get (time S) cid, list_map_get (balances S) cid, list_map_get (canister_status S) cid) of
+        (Some (Some can), Some t, Some bal, Some can_status) \<Rightarrow>
+        let env = \<lparr>env.time = t, balance = bal, freezing_limit = ic_freezing_limit S cid, certificate = None, status = simple_status can_status\<rparr> in
+        (case canister_module_inspect_message (module can) (request.method_name req, wasm_state can, request.arg req, principal_of_uid (request.sender req), env) of Inr ret \<Rightarrow>
+          list_map_set (balances S) cid (bal - cycles_return.cycles_used ret)))
+      else balances S) in
+    S\<lparr>requests := list_map_set (requests S) req Received, balances := balances\<rparr>)"
+
+definition request_submission_burned_cycles :: "('b, 'p, 'uid, 'canid, 's, 'pk, 'sig) envelope \<Rightarrow> ('p, 'uid, 'canid, 'b, 'w, 'sm, 'c, 's, 'cid, 'pk) ic \<Rightarrow> nat" where
+  "request_submission_burned_cycles E S = (
+    let req = projl (content E);
+    cid = request.canister_id req in
+    (if request.canister_id req \<noteq> ic_principal then
+      (case (list_map_get (canisters S) (request.canister_id req), list_map_get (time S) (request.canister_id req), list_map_get (balances S) (request.canister_id req), list_map_get (canister_status S) (request.canister_id req)) of
+        (Some (Some can), Some t, Some bal, Some can_status) \<Rightarrow>
+        let env = \<lparr>env.time = t, balance = bal, freezing_limit = ic_freezing_limit S (request.canister_id req), certificate = None, status = simple_status can_status\<rparr> in
+        (case canister_module_inspect_message (module can) (request.method_name req, wasm_state can, request.arg req, principal_of_uid (request.sender req), env) of Inr ret \<Rightarrow>
+          cycles_return.cycles_used ret))
+      else 0))"
 
 lemma request_submission_cycles_inv:
-  "request_submission_pre E S \<Longrightarrow> total_cycles S = total_cycles (request_submission_post E S)"
-  by (auto simp: request_submission_pre_def request_submission_post_def total_cycles_def)
+  assumes "request_submission_pre E S"
+  shows "total_cycles S = total_cycles (request_submission_post E S) + request_submission_burned_cycles E S"
+proof -
+  obtain req where req_def: "content E = Inl req"
+    using assms
+    by (auto simp: request_submission_pre_def split: sum.splits)
+  {
+    assume "request.canister_id req \<noteq> ic_principal"
+    then have "(case (list_map_get (canisters S) (request.canister_id req), list_map_get (time S) (request.canister_id req), list_map_get (balances S) (request.canister_id req), list_map_get (canister_status S) (request.canister_id req)) of
+      (Some (Some can), Some t, Some bal, Some can_status) \<Rightarrow>
+      let env = \<lparr>env.time = t, balance = bal, freezing_limit = ic_freezing_limit S (request.canister_id req), certificate = None, status = simple_status can_status\<rparr> in
+      (case canister_module_inspect_message (module can) (request.method_name req, wasm_state can, request.arg req, principal_of_uid (request.sender req), env) of Inr ret \<Rightarrow>
+        cycles_return.return ret = Accept \<and> cycles_return.cycles_used ret \<le> bal
+      | _ \<Rightarrow> False)
+    | _ \<Rightarrow> False)"
+      using assms
+      by (auto simp: request_submission_pre_def req_def split: option.splits sum.splits prod.splits)
+    then have ?thesis
+      using list_map_sum_in_ge[where ?f="balances S" and ?g=id and ?x="request.canister_id req"]
+      by (auto simp: request_submission_pre_def request_submission_post_def request_submission_burned_cycles_def total_cycles_def req_def list_map_sum_in[where ?f="balances S"]
+          split: option.splits sum.splits)
+  }
+  then show ?thesis
+    by (auto simp: request_submission_pre_def request_submission_post_def request_submission_burned_cycles_def total_cycles_def req_def)
+qed
+
+lemma request_submission_ic_inv:
+  assumes "request_submission_pre E S" "ic_inv S"
+  shows "ic_inv (request_submission_post E S)"
+  using assms
+  by (auto simp: ic_inv_def request_submission_pre_def request_submission_post_def Let_def
+      split: sum.splits message.splits call_origin.splits)
 
 
 
 (* System transition: Request rejection [DONE] *)
 
-definition request_rejection_pre :: "('b, 'p, 'uid, 'canid, 's, 'pk, 'sig, 'sd) envelope \<Rightarrow> ('b, 'p, 'uid, 'canid, 's) request \<Rightarrow> reject_code \<Rightarrow> 's \<Rightarrow> ('p, 'uid, 'canid, 'b, 'w, 'sm, 'c, 's, 'cid, 'pk) ic \<Rightarrow> bool" where
+definition request_rejection_pre :: "('b, 'p, 'uid, 'canid, 's, 'pk, 'sig) envelope \<Rightarrow> ('b, 'p, 'uid, 'canid, 's) request \<Rightarrow> reject_code \<Rightarrow> 's \<Rightarrow> ('p, 'uid, 'canid, 'b, 'w, 'sm, 'c, 's, 'cid, 'pk) ic \<Rightarrow> bool" where
   "request_rejection_pre E req code msg S = (list_map_get (requests S) req = Some Received \<and> (code = SYS_FATAL \<or> code = SYS_TRANSIENT))"
 
-definition request_rejection_post :: "('b, 'p, 'uid, 'canid, 's, 'pk, 'sig, 'sd) envelope \<Rightarrow> ('b, 'p, 'uid, 'canid, 's) request \<Rightarrow> reject_code \<Rightarrow> 's \<Rightarrow> ('p, 'uid, 'canid, 'b, 'w, 'sm, 'c, 's, 'cid, 'pk) ic \<Rightarrow> ('p, 'uid, 'canid, 'b, 'w, 'sm, 'c, 's, 'cid, 'pk) ic" where
+definition request_rejection_post :: "('b, 'p, 'uid, 'canid, 's, 'pk, 'sig) envelope \<Rightarrow> ('b, 'p, 'uid, 'canid, 's) request \<Rightarrow> reject_code \<Rightarrow> 's \<Rightarrow> ('p, 'uid, 'canid, 'b, 'w, 'sm, 'c, 's, 'cid, 'pk) ic \<Rightarrow> ('p, 'uid, 'canid, 'b, 'w, 'sm, 'c, 's, 'cid, 'pk) ic" where
   "request_rejection_post E req code msg S = S\<lparr>requests := list_map_set (requests S) req (Rejected code msg)\<rparr>"
 
 lemma request_rejection_cycles_inv:
-  "request_rejection_pre E req code msg S \<Longrightarrow> total_cycles S = total_cycles (request_rejection_post E req code msg S)"
+  assumes "request_rejection_pre E req code msg S"
+  shows "total_cycles S = total_cycles (request_rejection_post E req code msg S)"
   by (auto simp: request_rejection_pre_def request_rejection_post_def total_cycles_def)
+
+lemma request_rejection_ic_inv:
+  assumes "request_rejection_pre E req code msg S" "ic_inv S"
+  shows "ic_inv (request_rejection_post E req code msg S)"
+  using assms
+  by (auto simp: ic_inv_def request_rejection_pre_def request_rejection_post_def Let_def
+      split: sum.splits message.splits call_origin.splits)
 
 
 
@@ -397,9 +756,16 @@ definition initiate_canister_call_post :: "('b, 'p, 'uid, 'canid, 's) request \<
       (request.arg req) 0 Unordered # messages S\<rparr>"
 
 lemma initiate_canister_call_cycles_inv:
-  "initiate_canister_call_pre R S \<Longrightarrow>
-  total_cycles S = total_cycles (initiate_canister_call_post R S)"
+  assumes "initiate_canister_call_pre R S"
+  shows "total_cycles S = total_cycles (initiate_canister_call_post R S)"
   by (auto simp: initiate_canister_call_pre_def initiate_canister_call_post_def total_cycles_def)
+
+lemma initiate_canister_call_ic_inv:
+  assumes "initiate_canister_call_pre R S" "ic_inv S"
+  shows "ic_inv (initiate_canister_call_post R S)"
+  using assms
+  by (auto simp: ic_inv_def initiate_canister_call_pre_def initiate_canister_call_post_def Let_def
+      split: sum.splits message.splits call_origin.splits)
 
 
 
@@ -407,7 +773,7 @@ lemma initiate_canister_call_cycles_inv:
 
 definition call_reject_pre :: "nat \<Rightarrow> ('p, 'uid, 'canid, 'b, 'w, 'sm, 'c, 's, 'cid, 'pk) ic \<Rightarrow> bool" where
   "call_reject_pre n S = (n < length (messages S) \<and> (case messages S ! n of
-    Call_message orig cer cee mn d trans_cycles q \<Rightarrow>
+    Call_message orig cer cee mn a trans_cycles q \<Rightarrow>
       (q = Unordered \<or> (\<forall>j < n. message_queue (messages S ! j) \<noteq> Some q)) \<and>
       (case list_map_get (canister_status S) cee of Some Stopped \<Rightarrow> True
       | Some (Stopping l) \<Rightarrow> True
@@ -415,19 +781,19 @@ definition call_reject_pre :: "nat \<Rightarrow> ('p, 'uid, 'canid, 'b, 'w, 'sm,
     | _ \<Rightarrow> False))"
 
 definition call_reject_post :: "nat \<Rightarrow> ('p, 'uid, 'canid, 'b, 'w, 'sm, 'c, 's, 'cid, 'pk) ic \<Rightarrow> ('p, 'uid, 'canid, 'b, 'w, 'sm, 'c, 's, 'cid, 'pk) ic" where
-  "call_reject_post n S = (case messages S ! n of Call_message orig cer cee mn d trans_cycles q \<Rightarrow>
+  "call_reject_post n S = (case messages S ! n of Call_message orig cer cee mn a trans_cycles q \<Rightarrow>
     S\<lparr>messages := take n (messages S) @ drop (Suc n) (messages S) @ [Response_message orig (response.Reject CANISTER_ERROR (encode_string ''canister not running'')) trans_cycles]\<rparr>)"
 
 lemma call_reject_cycles_inv:
   assumes "call_reject_pre n S"
   shows "total_cycles S = total_cycles (call_reject_post n S)"
 proof -
-  obtain orig cer cee mn d trans_cycles q where msg: "messages S ! n = Call_message orig cer cee mn d trans_cycles q"
+  obtain orig cer cee mn a trans_cycles q where msg: "messages S ! n = Call_message orig cer cee mn a trans_cycles q"
     using assms
     by (auto simp: call_reject_pre_def split: message.splits)
   define older where "older = take n (messages S)"
   define younger where "younger = drop (Suc n) (messages S)"
-  have msgs: "messages S = older @ Call_message orig cer cee mn d trans_cycles q # younger" "(older @ w # younger) ! n = w"
+  have msgs: "messages S = older @ Call_message orig cer cee mn a trans_cycles q # younger" "(older @ w # younger) ! n = w"
     "take n older = older" "take (n - length older) ws = []" "drop (Suc n) older = []"
     "drop (Suc n - length older) (w # ws) = ws" for w ws
     using id_take_nth_drop[of n "messages S"] assms
@@ -437,6 +803,14 @@ proof -
     by (auto simp: call_reject_pre_def call_reject_post_def total_cycles_def Let_def msgs split: message.splits option.splits)
 qed
 
+lemma call_reject_ic_inv:
+  assumes "call_reject_pre n S" "ic_inv S"
+  shows "ic_inv (call_reject_post n S)"
+  using assms
+  by (auto simp: ic_inv_def call_reject_pre_def call_reject_post_def Let_def
+      split: sum.splits message.splits call_origin.splits
+      dest!: in_set_takeD in_set_dropD nth_mem[of n "messages S"])
+
 
 
 (* System transition: Call context creation: Public entry points [DONE] *)
@@ -444,7 +818,7 @@ qed
 definition call_context_create_pre :: "nat \<Rightarrow> 'cid
   \<Rightarrow> ('p, 'uid, 'canid, 'b, 'w, 'sm, 'c, 's, 'cid, 'pk) ic \<Rightarrow> bool" where
   "call_context_create_pre n ctxt_id S = (n < length (messages S) \<and> (case messages S ! n of
-    Call_message orig cer cee mn d trans_cycles q \<Rightarrow>
+    Call_message orig cer cee mn a trans_cycles q \<Rightarrow>
       (case list_map_get (canisters S) cee of Some (Some can) \<Rightarrow> True | _ \<Rightarrow> False) \<and>
       list_map_get (canister_status S) cee = Some Running \<and>
       (case list_map_get (balances S) cee of Some bal \<Rightarrow> bal \<ge> ic_freezing_limit S cee + MAX_CYCLES_PER_MESSAGE | None \<Rightarrow> False) \<and>
@@ -456,13 +830,16 @@ lift_definition create_call_ctxt :: "'canid \<Rightarrow> ('b, 'p, 'uid, 'canid,
   "\<lambda>cee orig trans_cycles. \<lparr>canister = cee, origin = orig, needs_to_respond = True, deleted = False, available_cycles = trans_cycles\<rparr>"
   by auto
 
+lemma create_call_ctxt_origin[simp]: "call_ctxt_origin (create_call_ctxt cee orig trans_cycles) = orig"
+  by transfer auto
+
 lemma create_call_ctxt_carried_cycles[simp]: "call_ctxt_carried_cycles (create_call_ctxt cee orig trans_cycles) = carried_cycles orig + trans_cycles"
   by transfer auto
 
 definition call_context_create_post :: "nat \<Rightarrow> 'cid \<Rightarrow> ('p, 'uid, 'canid, 'b, 'w, 'sm, 'c, 's, 'cid, 'pk) ic \<Rightarrow> ('p, 'uid, 'canid, 'b, 'w, 'sm, 'c, 's, 'cid, 'pk) ic" where
-  "call_context_create_post n ctxt_id S = (case messages S ! n of Call_message orig cer cee mn d trans_cycles q \<Rightarrow>
+  "call_context_create_post n ctxt_id S = (case messages S ! n of Call_message orig cer cee mn a trans_cycles q \<Rightarrow>
     case list_map_get (balances S) cee of Some bal \<Rightarrow>
-    S\<lparr>messages := list_update (messages S) n (Func_message ctxt_id cee (Public_method mn cer d) q),
+    S\<lparr>messages := list_update (messages S) n (Func_message ctxt_id cee (Public_method mn cer a) q),
       call_contexts := list_map_set (call_contexts S) ctxt_id (create_call_ctxt cee orig trans_cycles),
       balances := list_map_set (balances S) cee (bal - MAX_CYCLES_PER_MESSAGE)\<rparr>)"
 
@@ -470,20 +847,29 @@ lemma call_context_create_cycles_inv:
   assumes "call_context_create_pre n ctxt_id S"
   shows "total_cycles S = total_cycles (call_context_create_post n ctxt_id S)"
 proof -
-  obtain orig cer cee mn d trans_cycles q where msg: "messages S ! n = Call_message orig cer cee mn d trans_cycles q"
+  obtain orig cer cee mn a trans_cycles q where msg: "messages S ! n = Call_message orig cer cee mn a trans_cycles q"
     using assms
     by (auto simp: call_context_create_pre_def split: message.splits)
-  define xs where "xs = take n (messages S)"
-  define older where "older = drop (Suc n) (messages S)"
-  have msgs: "messages S = xs @ Call_message orig cer cee mn d trans_cycles q # older" "(xs @ m # older) ! n = m"
-    and msgs_upd: "(xs @ Call_message orig cer cee mn d trans_cycles q # older)[n := m] = xs @ m # older" for m
+  define older where "older = take n (messages S)"
+  define younger where "younger = drop (Suc n) (messages S)"
+  have msgs: "messages S = older @ Call_message orig cer cee mn a trans_cycles q # younger" "(older @ m # younger) ! n = m"
+    and msgs_upd: "(older @ Call_message orig cer cee mn a trans_cycles q # younger)[n := m] = older @ m # younger" for m
     using id_take_nth_drop[of n "messages S"] upd_conv_take_nth_drop[of n "messages S"] assms
-    by (auto simp: call_context_create_pre_def msg xs_def older_def nth_append)
+    by (auto simp: call_context_create_pre_def msg older_def younger_def nth_append)
   show ?thesis
     using assms list_map_sum_in_ge[of "balances S" cee, where ?g=id]
     by (auto simp: call_context_create_pre_def call_context_create_post_def total_cycles_def
         list_map_sum_in[where ?g=id, simplified] list_map_sum_out msgs msgs_upd split: option.splits)
 qed
+
+lemma call_context_create_ic_inv:
+  assumes "call_context_create_pre n ctxt_id S" "ic_inv S"
+  shows "ic_inv (call_context_create_post n ctxt_id S)"
+  using assms
+  by (auto simp: ic_inv_def call_context_create_pre_def call_context_create_post_def Let_def
+      split: sum.splits message.splits call_origin.splits option.splits
+      dest!: in_set_takeD in_set_dropD nth_mem[of n "messages S"] in_set_updD list_map_range_setD
+      intro: ic_can_status_inv_mono2)
 
 
 
@@ -500,6 +886,9 @@ lift_definition create_call_ctxt_heartbeat :: "'canid \<Rightarrow> ('p, 'uid, '
   "\<lambda>cee. \<lparr>canister = cee, origin = From_heartbeat, needs_to_respond = False, deleted = False, available_cycles = 0\<rparr>"
   by auto
 
+lemma create_call_ctxt_heartbeat_needs_to_respond[simp]: "call_ctxt_needs_to_respond (create_call_ctxt_heartbeat cee) = False"
+  by transfer auto
+
 lemma create_call_ctxt_heartbeat_carried_cycles[simp]: "call_ctxt_carried_cycles (create_call_ctxt_heartbeat cee) = 0"
   by transfer auto
 
@@ -511,11 +900,20 @@ definition call_context_heartbeat_post :: "'canid \<Rightarrow> 'cid \<Rightarro
     balances := list_map_set (balances S) cee (bal - MAX_CYCLES_PER_MESSAGE)\<rparr>)"
 
 lemma call_context_heartbeat_cycles_inv:
-  "call_context_heartbeat_pre cee ctxt_id S \<Longrightarrow>
-    total_cycles S = total_cycles (call_context_heartbeat_post cee ctxt_id S)"
-  using list_map_sum_in_ge[of "balances S" cee, where ?g=id, simplified]
+  assumes "call_context_heartbeat_pre cee ctxt_id S"
+  shows "total_cycles S = total_cycles (call_context_heartbeat_post cee ctxt_id S)"
+  using assms list_map_sum_in_ge[of "balances S" cee, where ?g=id, simplified]
   by (auto simp: call_context_heartbeat_pre_def call_context_heartbeat_post_def total_cycles_def
       list_map_sum_in[where ?g=id, simplified] list_map_sum_out split: option.splits)
+
+lemma call_context_heartbeat_ic_inv:
+  assumes "call_context_heartbeat_pre cee ctxt_id S" "ic_inv S"
+  shows "ic_inv (call_context_heartbeat_post cee ctxt_id S)"
+  using assms
+  by (auto simp: ic_inv_def call_context_heartbeat_pre_def call_context_heartbeat_post_def Let_def
+      split: sum.splits message.splits call_origin.splits option.splits
+      dest!: in_set_takeD in_set_dropD in_set_updD list_map_range_setD
+      intro: ic_can_status_inv_mono2)
 
 
 
@@ -527,17 +925,18 @@ fun query_as_update :: "(('b arg \<times> 'p \<times> 'b env) \<Rightarrow> ('w,
       update_return.response = Some (query_return.response res), update_return.cycles_accepted = 0, update_return.cycles_used = query_return.cycles_used res\<rparr>)"
 
 fun heartbeat_as_update :: "('b env \<Rightarrow> 'w heartbeat_func) \<times> 'b env \<Rightarrow> ('w, 'p, 'canid, 's, 'b, 'c) update_func" where
-  "heartbeat_as_update (f, e) w = (case f e w of Inl t \<Rightarrow> Inl t |
+  "heartbeat_as_update (f, e) = (\<lambda>w. case f e w of Inl t \<Rightarrow> Inl t |
     Inr res \<Rightarrow> Inr \<lparr>update_return.new_state = heartbeat_return.new_state res, update_return.new_calls = [], update_return.new_certified_data = None,
       update_return.response = None, update_return.cycles_accepted = 0, update_return.cycles_used = heartbeat_return.cycles_used res\<rparr>)"
 
 fun exec_function :: "('s, 'p, 'b, 'c) entry_point \<Rightarrow> 'b env \<Rightarrow> nat \<Rightarrow> ('p, 'canid, 'b, 'w, 'sm, 'c, 's) canister_module \<Rightarrow> ('w, 'p, 'canid, 's, 'b, 'c) update_func" where
-  "exec_function (entry_point.Public_method mn c d) e bal m = (
-    case dispatch_method mn m of Some (Inl upd) \<Rightarrow> upd (d, c, e, bal)
-    | Some (Inr query) \<Rightarrow> query_as_update (query, d, c, e) | None \<Rightarrow>
-    undefined)"
-| "exec_function (entry_point.Callback cb resp ref_cycles) e bal m =
-    canister_module_callbacks m (cb, resp, ref_cycles, e, bal)"
+  "exec_function (entry_point.Public_method mn c a) e bal m = (
+    case dispatch_method mn m of Some (Inl upd) \<Rightarrow> upd (a, c, e, bal)
+    | Some (Inr query) \<Rightarrow> query_as_update (query, a, c, e)
+    | None \<Rightarrow> undefined
+  )"
+| "exec_function (entry_point.Callback c resp ref_cycles) e bal m =
+    canister_module_callbacks m (c, resp, ref_cycles, e, bal)"
 | "exec_function (entry_point.Heartbeat) e bal m = heartbeat_as_update ((canister_module_heartbeat m), e)"
 
 definition message_execution_pre :: "nat \<Rightarrow> ('p, 'uid, 'canid, 'b, 'w, 'sm, 'c, 's, 'cid, 'pk) ic \<Rightarrow> bool" where
@@ -556,11 +955,11 @@ definition message_execution_post :: "nat \<Rightarrow> ('p, 'uid, 'canid, 'b, '
       (Some (Some can), Some bal, Some can_status, Some t, Some ctxt) \<Rightarrow> (
         let Mod = module can;
         Is_response = (case ep of Callback _ _ _ \<Rightarrow> True | _ \<Rightarrow> False);
-        Env = \<lparr>env_time = t, balance = bal, freezing_limit = ic_freezing_limit S recv, certificate = None, status = simple_status can_status\<rparr>;
+        Env = \<lparr>env.time = t, balance = bal, freezing_limit = ic_freezing_limit S recv, certificate = None, status = simple_status can_status\<rparr>;
         Available = call_ctxt_available_cycles ctxt;
         F = exec_function ep Env Available Mod;
         R = F (wasm_state can);
-        cyc_used = (case R of Inr res \<Rightarrow> update_return.cycles_used res | Inl trap \<Rightarrow> trap_return.cycles_used trap);
+        cyc_used = (case R of Inr res \<Rightarrow> update_return.cycles_used res | Inl trap \<Rightarrow> cycles_return.cycles_used trap);
         (cycles_accepted_res, new_calls_res) = (case R of Inr res \<Rightarrow> (update_return.cycles_accepted res, update_return.new_calls res));
         New_balance = bal + cycles_accepted_res + (if Is_response then MAX_CYCLES_PER_RESPONSE else MAX_CYCLES_PER_MESSAGE)
           - (cyc_used + sum_list (map (\<lambda>x. MAX_CYCLES_PER_RESPONSE + transferred_cycles x) new_calls_res));
@@ -572,8 +971,8 @@ definition message_execution_post :: "nat \<Rightarrow> ('p, 'uid, 'canid, 'b, '
           New_balance \<ge> (if Is_response then 0 else ic_freezing_limit S recv) \<and>
           (no_response \<or> call_ctxt_needs_to_respond ctxt) then
           (let result = projr R;
-            new_call_to_message = (\<lambda>call. Call_message (From_canister ctxt_id (callback call)) (principal_of_canid recv)
-              (callee call) (method_call.method_name call) (method_call.arg call) (transferred_cycles call) (Queue (Canister recv) (callee call)));
+            new_call_to_message = (\<lambda>call. Call_message (From_canister ctxt_id (method_call.callback call)) (principal_of_canid recv)
+              (method_call.callee call) (method_call.method_name call) (method_call.arg call) (method_call.transferred_cycles call) (Queue (Canister recv) (method_call.callee call)));
             response_messages = (case update_return.response result of None \<Rightarrow> []
               | Some resp \<Rightarrow> [Response_message (call_ctxt_origin ctxt) resp (Available - cycles_accepted_res)]);
             messages = take n (messages S) @ drop (Suc n) (messages S) @ map new_call_to_message new_calls_res @ response_messages;
@@ -584,30 +983,30 @@ definition message_execution_post :: "nat \<Rightarrow> ('p, 'uid, 'canid, 'b, '
               | Some cd \<Rightarrow> list_map_set (certified_data S) recv cd)
             in S\<lparr>canisters := list_map_set (canisters S) recv (Some (can\<lparr>wasm_state := update_return.new_state result\<rparr>)),
               messages := messages, call_contexts := list_map_set (call_contexts S) ctxt_id new_ctxt,
-              balances := list_map_set (balances S) recv New_balance, certified_data := certified_data\<rparr>)
+              certified_data := certified_data, balances := list_map_set (balances S) recv New_balance\<rparr>)
         else S\<lparr>messages := take n (messages S) @ drop (Suc n) (messages S),
           balances := list_map_set (balances S) recv ((bal + (if Is_response then MAX_CYCLES_PER_RESPONSE else MAX_CYCLES_PER_MESSAGE))
             - min cyc_used (if Is_response then MAX_CYCLES_PER_RESPONSE else MAX_CYCLES_PER_MESSAGE))\<rparr>))
     | _ \<Rightarrow> undefined)"
 
-definition message_execution_lost_cycles :: "nat \<Rightarrow> ('p, 'uid, 'canid, 'b, 'w, 'sm, 'c, 's, 'cid, 'pk) ic \<Rightarrow> nat" where
-  "message_execution_lost_cycles n S = (case messages S ! n of Func_message ctxt_id recv ep q \<Rightarrow>
+definition message_execution_burned_cycles :: "nat \<Rightarrow> ('p, 'uid, 'canid, 'b, 'w, 'sm, 'c, 's, 'cid, 'pk) ic \<Rightarrow> nat" where
+  "message_execution_burned_cycles n S = (case messages S ! n of Func_message ctxt_id recv ep q \<Rightarrow>
     (case (list_map_get (canisters S) recv, list_map_get (balances S) recv, list_map_get (canister_status S) recv,
       list_map_get (time S) recv, list_map_get (call_contexts S) ctxt_id) of
       (Some (Some can), Some bal, Some can_status, Some t, Some ctxt) \<Rightarrow> (
         let Mod = module can;
         Is_response = (case ep of Callback _ _ _ \<Rightarrow> True | _ \<Rightarrow> False);
-        Env = \<lparr>env_time = t, balance = bal, freezing_limit = ic_freezing_limit S recv, certificate = None, status = simple_status can_status\<rparr>;
+        Env = \<lparr>env.time = t, balance = bal, freezing_limit = ic_freezing_limit S recv, certificate = None, status = simple_status can_status\<rparr>;
         Available = call_ctxt_available_cycles ctxt;
         F = exec_function ep Env Available Mod;
         R = F (wasm_state can);
-        cyc_used = (case R of Inr res \<Rightarrow> update_return.cycles_used res | Inl trap \<Rightarrow> trap_return.cycles_used trap) in
+        cyc_used = (case R of Inr res \<Rightarrow> update_return.cycles_used res | Inl trap \<Rightarrow> cycles_return.cycles_used trap) in
         min cyc_used (if Is_response then MAX_CYCLES_PER_RESPONSE else MAX_CYCLES_PER_MESSAGE)
       )))"
 
 lemma message_execution_cycles_monotonic:
   assumes pre: "message_execution_pre n S"
-  shows "total_cycles S = total_cycles (message_execution_post n S) + message_execution_lost_cycles n S"
+  shows "total_cycles S = total_cycles (message_execution_post n S) + message_execution_burned_cycles n S"
 proof -
   obtain ctxt_id recv ep q can bal can_status t ctxt where msg: "messages S ! n = Func_message ctxt_id recv ep q"
     and prod: "list_map_get (canisters S) recv = Some (Some can)"
@@ -619,11 +1018,11 @@ proof -
     by (auto simp: message_execution_pre_def split: message.splits option.splits)
   define Mod where "Mod = can_state_rec.module can"
   define Is_response where "Is_response = (case ep of Callback _ _ _ \<Rightarrow> True | _ \<Rightarrow> False)"
-  define Env :: "'b env" where "Env = \<lparr>env_time = t, balance = bal, freezing_limit = ic_freezing_limit S recv, certificate = None, status = simple_status can_status\<rparr>"
+  define Env :: "'b env" where "Env = \<lparr>env.time = t, balance = bal, freezing_limit = ic_freezing_limit S recv, certificate = None, status = simple_status can_status\<rparr>"
   define Available where "Available = call_ctxt_available_cycles ctxt"
   define F where "F = exec_function ep Env Available Mod"
   define R where "R = F (wasm_state can)"
-  define cyc_used where "cyc_used = (case R of Inr res \<Rightarrow> update_return.cycles_used res | Inl trap \<Rightarrow> trap_return.cycles_used trap)"
+  define cyc_used where "cyc_used = (case R of Inr res \<Rightarrow> update_return.cycles_used res | Inl trap \<Rightarrow> cycles_return.cycles_used trap)"
   obtain cycles_accepted_res new_calls_res where res: "(cycles_accepted_res, new_calls_res) = (case R of Inr res \<Rightarrow> (update_return.cycles_accepted res, new_calls res))"
     by (cases "(case R of Inr res \<Rightarrow> (update_return.cycles_accepted res, new_calls res))") auto
   define New_balance where "New_balance = bal + cycles_accepted_res + (if Is_response then MAX_CYCLES_PER_RESPONSE else MAX_CYCLES_PER_MESSAGE)
@@ -653,9 +1052,9 @@ proof -
   proof (cases cond)
     case False
     have "message_execution_post n S = S''"
-      "message_execution_lost_cycles n S = min cyc_used (if Is_response then MAX_CYCLES_PER_RESPONSE else MAX_CYCLES_PER_MESSAGE)"
+      "message_execution_burned_cycles n S = min cyc_used (if Is_response then MAX_CYCLES_PER_RESPONSE else MAX_CYCLES_PER_MESSAGE)"
       using False
-      by (simp_all add: message_execution_post_def message_execution_lost_cycles_def Let_def msg prod
+      by (simp_all add: message_execution_post_def message_execution_burned_cycles_def Let_def msg prod
           Mod_def[symmetric] Is_response_def[symmetric] Env_def[symmetric] Available_def[symmetric] F_def[symmetric] R_def[symmetric] cyc_used_def[symmetric] res[symmetric]
           New_balance_def[symmetric] no_response_def[symmetric] S''_def[symmetric] cond_def[symmetric] del: min_less_iff_conj split del: if_split)
     then show ?thesis
@@ -666,7 +1065,7 @@ proof -
     define result where "result = projr R"
     have R_Inr: "R = Inr result"
       using True
-      by (auto simp: cond_def result_def)
+      by (auto simp: cond_def result_def split: option.splits)
     define response_messages where "response_messages = (case update_return.response result of None \<Rightarrow> []
       | Some resp \<Rightarrow> [Response_message (call_ctxt_origin ctxt) resp (Available - cycles_accepted_res)])"
     define new_call_to_message :: "(?'p, 'canid, 's, 'b, 'c) method_call \<Rightarrow> ('b, 'p, 'uid, 'canid, 's, 'c, 'cid) message" where
@@ -680,7 +1079,7 @@ proof -
       | Some cd \<Rightarrow> list_map_set (ic.certified_data S) recv cd)"
     define S' where "S' = S\<lparr>canisters := list_map_set (canisters S) recv (Some (can\<lparr>wasm_state := update_return.new_state result\<rparr>)),
       messages := messages, call_contexts := list_map_set (call_contexts S) ctxt_id new_ctxt,
-      balances := list_map_set (balances S) recv New_balance, certified_data := certified_data\<rparr>"
+      certified_data := certified_data, balances := list_map_set (balances S) recv New_balance\<rparr>"
     have cycles_accepted_res_def: "cycles_accepted_res = update_return.cycles_accepted result"
       and new_calls_res_def: "new_calls_res = new_calls result"
       using res
@@ -688,9 +1087,9 @@ proof -
     have no_response: "no_response = (update_return.response result = None)"
       by (auto simp: no_response_def R_Inr)
     have msg_exec: "message_execution_post n S = S'"
-      and lost: "message_execution_lost_cycles n S = min cyc_used (if Is_response then MAX_CYCLES_PER_RESPONSE else MAX_CYCLES_PER_MESSAGE)"
+      and lost: "message_execution_burned_cycles n S = min cyc_used (if Is_response then MAX_CYCLES_PER_RESPONSE else MAX_CYCLES_PER_MESSAGE)"
       using True
-      by (simp_all add: message_execution_post_def message_execution_lost_cycles_def Let_def msg prod
+      by (simp_all add: message_execution_post_def message_execution_burned_cycles_def Let_def msg prod
           Mod_def[symmetric] Is_response_def[symmetric] Env_def[symmetric] Available_def[symmetric] F_def[symmetric] R_def[symmetric] cyc_used_def[symmetric] res[symmetric]
           New_balance_def[symmetric] no_response_def[symmetric] S''_def[symmetric] cond_def[symmetric]
           messages_def[symmetric] new_ctxt_def[symmetric] certified_data_def[symmetric] S'_def[symmetric]
@@ -714,9 +1113,129 @@ proof -
     have messages_msgs: "messages = older @ younger @ map new_call_to_message new_calls_res @ response_messages"
       by (auto simp: messages_def older_def younger_def)
     show ?thesis
-      using lm(2,4) True call_ctxt_inv[of ctxt]
+      using lm(2,4) True call_ctxt_not_needs_to_respond_available_cycles[of ctxt]
       by (auto simp: cond_def msg_exec S'_def total_cycles_def lm(1,3) msgs messages_msgs A1 A2 A3 A4 New_balance_def
           reserve cycles_accepted_res_def no_response_def R_Inr lost Available_def split: option.splits)
+  qed
+qed
+
+lemma message_execution_ic_inv:
+  assumes "message_execution_pre n S" "ic_inv S"
+  shows "ic_inv (message_execution_post n S)"
+proof -
+  obtain ctxt_id recv ep q can bal can_status t ctxt where msg: "messages S ! n = Func_message ctxt_id recv ep q"
+    and prod: "list_map_get (canisters S) recv = Some (Some can)"
+    "list_map_get (balances S) recv = Some bal"
+    "list_map_get (canister_status S) recv = Some can_status"
+    "list_map_get (time S) recv = Some t"
+    "list_map_get (call_contexts S) ctxt_id = Some ctxt"
+    using assms
+    by (auto simp: message_execution_pre_def split: message.splits option.splits)
+  define Mod where "Mod = can_state_rec.module can"
+  define Is_response where "Is_response = (case ep of Callback _ _ _ \<Rightarrow> True | _ \<Rightarrow> False)"
+  define Env :: "'b env" where "Env = \<lparr>env.time = t, balance = bal, freezing_limit = ic_freezing_limit S recv, certificate = None, status = simple_status can_status\<rparr>"
+  define Available where "Available = call_ctxt_available_cycles ctxt"
+  define F where "F = exec_function ep Env Available Mod"
+  define R where "R = F (wasm_state can)"
+  define cyc_used where "cyc_used = (case R of Inr res \<Rightarrow> update_return.cycles_used res | Inl trap \<Rightarrow> cycles_return.cycles_used trap)"
+  obtain cycles_accepted_res new_calls_res where res: "(cycles_accepted_res, new_calls_res) = (case R of Inr res \<Rightarrow> (update_return.cycles_accepted res, new_calls res))"
+    by (cases "(case R of Inr res \<Rightarrow> (update_return.cycles_accepted res, new_calls res))") auto
+  define New_balance where "New_balance = bal + cycles_accepted_res + (if Is_response then MAX_CYCLES_PER_RESPONSE else MAX_CYCLES_PER_MESSAGE)
+    - (cyc_used + sum_list (map (\<lambda>x. MAX_CYCLES_PER_RESPONSE + transferred_cycles x) new_calls_res))"
+  define no_response where "no_response = (case R of Inr result \<Rightarrow> update_return.response result = None)"
+  define older where "older = take n (messages S)"
+  define younger where "younger = drop (Suc n) (messages S)"
+  have msgs: "messages S = older @ Func_message ctxt_id recv ep q # younger"
+    "take n older = older" "drop (Suc n) older = []"
+    "take (n - length older) ws = []" "drop (Suc n - length older) (w # ws) = ws"
+    for w and ws :: "('b, 'p, 'uid, 'canid, 's, 'c, 'cid) message list"
+    using id_take_nth_drop[of n "messages S"] assms
+    by (auto simp: message_execution_pre_def msg older_def younger_def)
+  define S'' where "S'' = S\<lparr>messages := take n (messages S) @ drop (Suc n) (messages S),
+    balances := list_map_set (balances S) recv ((bal + (if Is_response then MAX_CYCLES_PER_RESPONSE else MAX_CYCLES_PER_MESSAGE)) - min cyc_used (if Is_response then MAX_CYCLES_PER_RESPONSE else MAX_CYCLES_PER_MESSAGE))\<rparr>"
+  define cond where "cond = (\<not>isl R \<and> cyc_used \<le> (if Is_response then MAX_CYCLES_PER_RESPONSE else MAX_CYCLES_PER_MESSAGE) \<and>
+    cycles_accepted_res \<le> Available \<and>
+    cyc_used + sum_list (map (\<lambda>x. MAX_CYCLES_PER_RESPONSE + transferred_cycles x) new_calls_res) \<le>
+      bal + cycles_accepted_res + (if Is_response then MAX_CYCLES_PER_RESPONSE else MAX_CYCLES_PER_MESSAGE) \<and>
+    New_balance \<ge> (if Is_response then 0 else ic_freezing_limit S recv) \<and>
+    (no_response \<or> call_ctxt_needs_to_respond ctxt))"
+  show ?thesis
+  proof (cases cond)
+    case False
+    have "message_execution_post n S = S''"
+      using False
+      by (simp_all add: message_execution_post_def Let_def msg prod
+          Mod_def[symmetric] Is_response_def[symmetric] Env_def[symmetric] Available_def[symmetric] F_def[symmetric] R_def[symmetric] cyc_used_def[symmetric] res[symmetric]
+          New_balance_def[symmetric] no_response_def[symmetric] S''_def[symmetric] cond_def[symmetric])
+    then show ?thesis
+      using assms(2)
+      apply (auto simp: ic_inv_def S''_def msgs split: message.splits call_origin.splits)
+         apply force
+        apply fast
+       apply force
+      apply fast
+      done
+  next
+    case True
+    define result where "result = projr R"
+    have R_Inr: "R = Inr result"
+      using True
+      by (auto simp: cond_def result_def split: option.splits)
+    define response_messages where "response_messages = (case update_return.response result of None \<Rightarrow> []
+      | Some resp \<Rightarrow> [Response_message (call_ctxt_origin ctxt) resp (Available - cycles_accepted_res)])"
+    define new_call_to_message :: "(?'p, 'canid, 's, 'b, 'c) method_call \<Rightarrow> ('b, 'p, 'uid, 'canid, 's, 'c, 'cid) message" where
+      "new_call_to_message = (\<lambda>call. Call_message (From_canister ctxt_id (callback call)) (principal_of_canid recv)
+        (callee call) (method_call.method_name call) (method_call.arg call) (transferred_cycles call) (Queue (Canister recv) (callee call)))"
+    define messages where "messages = take n (ic.messages S) @ drop (Suc n) (ic.messages S) @ map new_call_to_message new_calls_res @ response_messages"
+    define new_ctxt where "new_ctxt = (case update_return.response result of
+        None \<Rightarrow> call_ctxt_deduct_cycles cycles_accepted_res ctxt
+      | Some _ \<Rightarrow> call_ctxt_respond ctxt)"
+    define certified_data where "certified_data = (case new_certified_data result of None \<Rightarrow> ic.certified_data S
+      | Some cd \<Rightarrow> list_map_set (ic.certified_data S) recv cd)"
+    define S' where "S' = S\<lparr>canisters := list_map_set (canisters S) recv (Some (can\<lparr>wasm_state := update_return.new_state result\<rparr>)),
+      messages := messages, call_contexts := list_map_set (call_contexts S) ctxt_id new_ctxt,
+      certified_data := certified_data, balances := list_map_set (balances S) recv New_balance\<rparr>"
+    have cycles_accepted_res_def: "cycles_accepted_res = update_return.cycles_accepted result"
+      and new_calls_res_def: "new_calls_res = new_calls result"
+      using res
+      by (auto simp: R_Inr)
+    have no_response: "no_response = (update_return.response result = None)"
+      by (auto simp: no_response_def R_Inr)
+    have msg_exec: "message_execution_post n S = S'"
+      using True
+      by (simp_all add: message_execution_post_def Let_def msg prod
+          Mod_def[symmetric] Is_response_def[symmetric] Env_def[symmetric] Available_def[symmetric] F_def[symmetric] R_def[symmetric] cyc_used_def[symmetric] res[symmetric]
+          New_balance_def[symmetric] no_response_def[symmetric] S''_def[symmetric] cond_def[symmetric]
+          messages_def[symmetric] new_ctxt_def[symmetric] certified_data_def[symmetric] S'_def[symmetric]
+          result_def[symmetric] response_messages_def[symmetric] new_call_to_message_def[symmetric])
+    have messages_msgs: "messages = older @ younger @ map new_call_to_message new_calls_res @ response_messages"
+      by (auto simp: messages_def older_def younger_def)
+    have ctxt_in_range: "ctxt \<in> list_map_range (call_contexts S)"
+      using prod(5)
+      by (simp add: list_map_get_range)
+    have response_msgsD: "msg \<in> set response_messages \<Longrightarrow> update_return.response result \<noteq> None \<and>
+      (\<exists>resp. msg = Response_message (call_ctxt_origin ctxt) resp (Available - cycles_accepted_res))" for msg
+      by (auto simp: response_messages_def) metis
+    have call_ctxt_origin_new_ctxt: "call_ctxt_origin new_ctxt = call_ctxt_origin ctxt"
+      by (auto simp: new_ctxt_def split: option.splits)
+    have call_ctxt_needs_to_respond_new_ctxtD: "call_ctxt_needs_to_respond new_ctxt \<Longrightarrow> call_ctxt_needs_to_respond ctxt"
+      by (auto simp: new_ctxt_def split: option.splits)
+    show ?thesis
+      using assms(2) ctxt_in_range True call_ctxt_not_needs_to_respond_available_cycles[of ctxt]
+      apply (auto simp: cond_def msg_exec S'_def ic_inv_def msgs messages_msgs new_call_to_message_def
+          no_response_def R_Inr call_ctxt_origin_new_ctxt
+          split: option.splits message.splits call_origin.splits
+          dest!: list_map_range_setD response_msgsD call_ctxt_needs_to_respond_new_ctxtD
+          intro: ic_can_status_inv_mono2)
+             apply blast
+            apply fast
+           apply blast
+          apply fast
+         apply blast
+        apply fast
+       apply blast
+      apply fast
+      done
   qed
 qed
 
@@ -726,13 +1245,14 @@ qed
 
 definition call_context_starvation_pre :: "'cid \<Rightarrow> ('p, 'uid, 'canid, 'b, 'w, 'sm, 'c, 's, 'cid, 'pk) ic \<Rightarrow> bool" where
   "call_context_starvation_pre ctxt_id S =
-  (case list_map_get (call_contexts S) ctxt_id of Some call_context \<Rightarrow> call_ctxt_needs_to_respond call_context \<and>
+  (case list_map_get (call_contexts S) ctxt_id of Some call_context \<Rightarrow>
+    call_ctxt_needs_to_respond call_context \<and>
     call_ctxt_origin call_context \<noteq> From_heartbeat \<and>
     (\<forall>msg \<in> set (messages S). case msg of
         Call_message orig _ _ _ _ _ _ \<Rightarrow> calling_context orig \<noteq> Some ctxt_id
       | Response_message orig _ _ \<Rightarrow> calling_context orig \<noteq> Some ctxt_id
       | _ \<Rightarrow> True) \<and>
-    (\<forall>other_call_context \<in> list_map_vals (call_contexts S).
+    (\<forall>other_call_context \<in> list_map_range (call_contexts S).
       call_ctxt_needs_to_respond other_call_context \<longrightarrow>
       calling_context (call_ctxt_origin other_call_context) \<noteq> Some ctxt_id)
   | None \<Rightarrow> False)"
@@ -746,11 +1266,20 @@ definition call_context_starvation_post :: "'cid \<Rightarrow>
         messages := messages S @ [msg]\<rparr>)"
 
 lemma call_context_starvation_cycles_inv:
-  "call_context_starvation_pre ctxt_id S \<Longrightarrow>
-  total_cycles S = total_cycles (call_context_starvation_post ctxt_id S)"
-  using list_map_sum_in_ge[where ?f="call_contexts S" and ?x=ctxt_id and ?g=call_ctxt_carried_cycles]
+  assumes "call_context_starvation_pre ctxt_id S"
+  shows "total_cycles S = total_cycles (call_context_starvation_post ctxt_id S)"
+  using assms list_map_sum_in_ge[where ?f="call_contexts S" and ?x=ctxt_id and ?g=call_ctxt_carried_cycles]
   by (auto simp: call_context_starvation_pre_def call_context_starvation_post_def total_cycles_def
       call_ctxt_carried_cycles list_map_sum_in[where ?g=call_ctxt_carried_cycles] split: option.splits)
+
+lemma call_context_starvation_ic_inv:
+  assumes "call_context_starvation_pre ctxt_id S" "ic_inv S"
+  shows "ic_inv (call_context_starvation_post ctxt_id S)"
+  using assms
+  by (auto simp: ic_inv_def call_context_starvation_pre_def call_context_starvation_post_def Let_def
+      split: sum.splits message.splits call_origin.splits option.splits
+      dest!: in_set_takeD in_set_dropD in_set_updD list_map_range_setD list_map_get_range
+      intro: ic_can_status_inv_mono2)
 
 
 
@@ -768,21 +1297,1517 @@ definition call_context_removal_pre :: "'cid \<Rightarrow> ('p, 'uid, 'canid, 'b
           Call_message ctxt _ _ _ _ _ _ \<Rightarrow> calling_context ctxt \<noteq> Some ctxt_id
         | Response_message ctxt _ _ \<Rightarrow> calling_context ctxt \<noteq> Some ctxt_id
         | _ \<Rightarrow> True) \<and>
-      (\<forall>other_call_context \<in> list_map_vals (call_contexts S).
+      (\<forall>other_call_context \<in> list_map_range (call_contexts S).
         call_ctxt_needs_to_respond other_call_context \<longrightarrow>
-        calling_context (call_ctxt_origin other_call_context) \<noteq> Some ctxt_id)
+        calling_context (call_ctxt_origin other_call_context) \<noteq> Some ctxt_id) \<and>
+      (\<forall>can_status \<in> list_map_range (canister_status S). case can_status of Stopping os \<Rightarrow>
+        \<forall>(orig, cyc) \<in> set os. (case orig of From_canister other_ctxt_id _ \<Rightarrow> ctxt_id \<noteq> other_ctxt_id | _ \<Rightarrow> True)
+      | _ \<Rightarrow> True)
     | None \<Rightarrow> False))"
 
 definition call_context_removal_post :: "'cid \<Rightarrow>
   ('p, 'uid, 'canid, 'b, 'w, 'sm, 'c, 's, 'cid, 'pk) ic \<Rightarrow> ('p, 'uid, 'canid, 'b, 'w, 'sm, 'c, 's, 'cid, 'pk) ic" where
   "call_context_removal_post ctxt_id S = S\<lparr>call_contexts := list_map_del (call_contexts S) ctxt_id\<rparr>"
 
-lemma call_context_removal_cycles_inv:
-  "call_context_removal_pre ctxt_id S \<Longrightarrow>
-  total_cycles S = total_cycles (call_context_removal_post ctxt_id S) +
-    (case list_map_get (call_contexts S) ctxt_id of Some call_context \<Rightarrow> call_ctxt_available_cycles call_context)"
-  using call_ctxt_inv
-  by (auto simp: call_context_removal_pre_def call_context_removal_post_def total_cycles_def call_ctxt_carried_cycles list_map_del_sum split: option.splits)
+definition call_context_removal_burned_cycles :: "'cid \<Rightarrow> ('p, 'uid, 'canid, 'b, 'w, 'sm, 'c, 's, 'cid, 'pk) ic \<Rightarrow> nat" where
+  "call_context_removal_burned_cycles ctxt_id S = call_ctxt_available_cycles (the (list_map_get (call_contexts S) ctxt_id))"
+
+lemma call_context_removal_cycles_monotonic:
+  assumes "call_context_removal_pre ctxt_id S"
+  shows "total_cycles S = total_cycles (call_context_removal_post ctxt_id S) + call_context_removal_burned_cycles ctxt_id S"
+  using assms call_ctxt_not_needs_to_respond_available_cycles
+  by (auto simp: call_context_removal_pre_def call_context_removal_post_def call_context_removal_burned_cycles_def total_cycles_def call_ctxt_carried_cycles list_map_del_sum split: option.splits)
+
+lemma call_context_removal_ic_inv:
+  assumes "call_context_removal_pre ctxt_id S" "ic_inv S"
+  shows "ic_inv (call_context_removal_post ctxt_id S)"
+  using assms
+  by (force simp: ic_inv_def call_context_removal_pre_def call_context_removal_post_def Let_def
+      split: sum.splits message.splits call_origin.splits option.splits
+      dest!: in_set_takeD in_set_dropD in_set_updD list_map_range_setD list_map_get_range list_map_range_del
+      intro!: ic_can_status_inv_del[where ?z="list_map_dom (call_contexts S)"])
+
+
+
+(* System transition: IC Management Canister: Canister creation [DONE] *)
+
+definition ic_canister_creation_pre :: "nat \<Rightarrow> 'canid \<Rightarrow> nat \<Rightarrow> ('p, 'uid, 'canid, 'b, 'w, 'sm, 'c, 's, 'cid, 'pk) ic \<Rightarrow> bool" where
+  "ic_canister_creation_pre n cid t S = (n < length (messages S) \<and> (case messages S ! n of
+    Call_message orig cer cee mn a trans_cycles q \<Rightarrow>
+      (q = Unordered \<or> (\<forall>j < n. message_queue (messages S ! j) \<noteq> Some q)) \<and>
+      cee = ic_principal \<and>
+      mn = encode_string ''create_canister'' \<and>
+      parse_candid a \<noteq> None \<and>
+      is_system_assigned (principal_of_canid cid) \<and>
+      cid \<notin> list_map_dom (canisters S) \<and>
+      cid \<notin> list_map_dom (time S) \<and>
+      cid \<notin> list_map_dom (controllers S) \<and>
+      cid \<notin> list_map_dom (balances S) \<and>
+      cid \<notin> list_map_dom (certified_data S) \<and>
+      cid \<notin> list_map_dom (canister_status S)
+    | _ \<Rightarrow> False))"
+
+definition ic_canister_creation_post :: "nat \<Rightarrow> 'canid \<Rightarrow> nat \<Rightarrow> ('p, 'uid, 'canid, 'b, 'w, 'sm, 'c, 's, 'cid, 'pk) ic \<Rightarrow> ('p, 'uid, 'canid, 'b, 'w, 'sm, 'c, 's, 'cid, 'pk) ic" where
+  "ic_canister_creation_post n cid t S = (case messages S ! n of Call_message orig cer cee mn a trans_cycles q \<Rightarrow>
+    let ctrls = (case candid_parse_controllers a of Some ctrls \<Rightarrow> ctrls | _ \<Rightarrow> {cer}) in
+    S\<lparr>canisters := list_map_set (canisters S) cid None,
+      time := list_map_set (time S) cid t,
+      controllers := list_map_set (controllers S) cid ctrls,
+      freezing_threshold := list_map_set (freezing_threshold S) cid 2592000,
+      balances := list_map_set (balances S) cid trans_cycles,
+      certified_data := list_map_set (certified_data S) cid empty_blob,
+      messages := take n (messages S) @ drop (Suc n) (messages S) @ [Response_message orig (Reply (blob_of_candid
+        (Candid_record (list_map_init [(encode_string ''canister_id'', Candid_blob (blob_of_canid cid))])))) 0],
+      canister_status := list_map_set (canister_status S) cid Running\<rparr>)"
+
+lemma ic_canister_creation_cycles_inv:
+  assumes "ic_canister_creation_pre n cid t S"
+  shows "total_cycles S = total_cycles (ic_canister_creation_post n cid t S)"
+proof -
+  obtain orig cer cee mn a trans_cycles q where msg: "messages S ! n = Call_message orig cer cee mn a trans_cycles q"
+    using assms
+    by (auto simp: ic_canister_creation_pre_def split: message.splits)
+  define older where "older = take n (messages S)"
+  define younger where "younger = drop (Suc n) (messages S)"
+  have msgs: "messages S = older @ Call_message orig cer cee mn a trans_cycles q # younger" "(older @ w # younger) ! n = w"
+    "take n older = older" "take (n - length older) ws = []" "drop (Suc n) older = []"
+    "drop (Suc n - length older) (w # ws) = ws" for w ws
+    using id_take_nth_drop[of n "messages S"] assms
+    by (auto simp: ic_canister_creation_pre_def msg younger_def older_def nth_append)
+  show ?thesis
+    using assms
+    by (auto simp: ic_canister_creation_pre_def ic_canister_creation_post_def total_cycles_def Let_def msgs
+        list_map_sum_out[where ?g=id] list_map_sum_out[where ?g=status_cycles] split: message.splits option.splits)
+qed
+
+lemma ic_canister_creation_ic_inv:
+  assumes "ic_canister_creation_pre n cid t S" "ic_inv S"
+  shows "ic_inv (ic_canister_creation_post n cid t S)"
+  using assms
+  by (auto simp: ic_inv_def ic_canister_creation_pre_def ic_canister_creation_post_def Let_def
+      split: sum.splits message.splits call_origin.splits option.splits
+      dest!: in_set_takeD in_set_dropD nth_mem[of n "messages S"] in_set_updD list_map_range_setD list_map_get_range list_map_range_del
+      intro: ic_can_status_inv_mono1)
+
+
+
+(* System transition: IC Management Canister: Changing settings [DONE] *)
+
+definition ic_update_settings_pre :: "nat \<Rightarrow> ('p, 'uid, 'canid, 'b, 'w, 'sm, 'c, 's, 'cid, 'pk) ic \<Rightarrow> bool" where
+  "ic_update_settings_pre n S = (n < length (messages S) \<and> (case messages S ! n of
+    Call_message orig cer cee mn a trans_cycles q \<Rightarrow>
+      (q = Unordered \<or> (\<forall>j < n. message_queue (messages S ! j) \<noteq> Some q)) \<and>
+      cee = ic_principal \<and>
+      mn = encode_string ''update_settings'' \<and>
+      (case candid_parse_cid a of Some cid \<Rightarrow>
+      (case list_map_get (controllers S) cid of Some ctrls \<Rightarrow> cer \<in> ctrls
+      | _ \<Rightarrow> False) | _ \<Rightarrow> False)
+    | _ \<Rightarrow> False))"
+
+definition ic_update_settings_post :: "nat \<Rightarrow> ('p, 'uid, 'canid, 'b, 'w, 'sm, 'c, 's, 'cid, 'pk) ic \<Rightarrow> ('p, 'uid, 'canid, 'b, 'w, 'sm, 'c, 's, 'cid, 'pk) ic" where
+  "ic_update_settings_post n S = (case messages S ! n of Call_message orig cer cee mn a trans_cycles q \<Rightarrow>
+    let cid = the (candid_parse_cid a);
+    ctrls = (case candid_parse_controllers a of Some ctrls \<Rightarrow> list_map_set (controllers S) cid ctrls | _ \<Rightarrow> controllers S);
+    freezing_thres = (case candid_nested_lookup a [encode_string '''settings'', encode_string ''freezing_threshold''] of Some (Candid_nat freeze) \<Rightarrow>
+      list_map_set (freezing_threshold S) cid freeze | _ \<Rightarrow> freezing_threshold S) in
+    S\<lparr>controllers := ctrls, freezing_threshold := freezing_thres, messages := take n (messages S) @ drop (Suc n) (messages S) @
+        [Response_message orig (Reply (blob_of_candid Candid_empty)) trans_cycles]\<rparr>)"
+
+lemma ic_update_settings_cycles_inv:
+  assumes "ic_update_settings_pre n S"
+  shows "total_cycles S = total_cycles (ic_update_settings_post n S)"
+proof -
+  obtain orig cer cee mn a trans_cycles q where msg: "messages S ! n = Call_message orig cer cee mn a trans_cycles q"
+    using assms
+    by (auto simp: ic_update_settings_pre_def split: message.splits)
+  define older where "older = take n (messages S)"
+  define younger where "younger = drop (Suc n) (messages S)"
+  have msgs: "messages S = older @ Call_message orig cer cee mn a trans_cycles q # younger" "(older @ w # younger) ! n = w"
+    "take n older = older" "take (n - length older) ws = []" "drop (Suc n) older = []"
+    "drop (Suc n - length older) (w # ws) = ws" for w ws
+    using id_take_nth_drop[of n "messages S"] assms
+    by (auto simp: ic_update_settings_pre_def msg younger_def older_def nth_append)
+  show ?thesis
+    using assms
+    by (auto simp: ic_update_settings_pre_def ic_update_settings_post_def total_cycles_def Let_def msgs split: message.splits option.splits)
+qed
+
+lemma ic_update_settings_ic_inv:
+  assumes "ic_update_settings_pre n S" "ic_inv S"
+  shows "ic_inv (ic_update_settings_post n S)"
+  using assms
+  by (auto simp: ic_inv_def ic_update_settings_pre_def ic_update_settings_post_def Let_def
+      split: sum.splits message.splits call_origin.splits option.splits
+      dest!: in_set_takeD in_set_dropD nth_mem[of n "messages S"] in_set_updD list_map_range_setD list_map_get_range list_map_range_del)
+
+
+
+(* System transition: IC Management Canister: Canister status [DONE] *)
+
+definition ic_canister_status_pre :: "nat \<Rightarrow> nat \<Rightarrow> ('p, 'uid, 'canid, 'b, 'w, 'sm, 'c, 's, 'cid, 'pk) ic \<Rightarrow> bool" where
+  "ic_canister_status_pre n m S = (n < length (messages S) \<and> (case messages S ! n of Call_message orig cer cee mn a trans_cycles q \<Rightarrow>
+    (q = Unordered \<or> (\<forall>j < n. message_queue (messages S ! j) \<noteq> Some q)) \<and>
+    cee = ic_principal \<and>
+    mn = encode_string ''canister_status'' \<and>
+    (case candid_parse_cid a of Some cid \<Rightarrow>
+      cid \<in> list_map_dom (canisters S) \<and>
+      cid \<in> list_map_dom (canister_status S) \<and>
+      cid \<in> list_map_dom (balances S) \<and>
+      cid \<in> list_map_dom (freezing_threshold S) \<and>
+    (case list_map_get (controllers S) cid of Some ctrls \<Rightarrow> cer \<in> ctrls | _ \<Rightarrow> False) | _ \<Rightarrow> False)
+  | _ \<Rightarrow> False))"
+
+definition ic_canister_status_post :: "nat \<Rightarrow> nat \<Rightarrow> ('p, 'uid, 'canid, 'b, 'w, 'sm, 'c, 's, 'cid, 'pk) ic \<Rightarrow> ('p, 'uid, 'canid, 'b, 'w, 'sm, 'c, 's, 'cid, 'pk) ic" where
+  "ic_canister_status_post n m S = (case messages S ! n of Call_message orig cer cee mn a trans_cycles q \<Rightarrow>
+    let cid = the (candid_parse_cid a);
+    hash = (case the (list_map_get (canisters S) cid) of None \<Rightarrow> Candid_null
+      | Some can \<Rightarrow> Candid_opt (Candid_blob (sha_256 (raw_module can)))) in
+    S\<lparr>messages := take n (messages S) @ drop (Suc n) (messages S) @ [Response_message orig (Reply (blob_of_candid
+      (Candid_record (list_map_init [(encode_string ''status'', candid_of_status (simple_status (the (list_map_get (canister_status S) cid)))),
+        (encode_string ''module_hash'', hash),
+        (encode_string ''controllers'', Candid_vec (map (Candid_blob \<circ> blob_of_principal) (principal_list_of_set (the (list_map_get (controllers S) cid))))),
+        (encode_string ''memory_size'', Candid_nat m),
+        (encode_string ''cycles'', Candid_nat (the (list_map_get (balances S) cid))),
+        (encode_string ''freezing_threshold'', Candid_nat (the (list_map_get (freezing_threshold S) cid))),
+        (encode_string ''idle_cycles_burned_per_day'', Candid_nat (ic_idle_cycles_burned_rate S cid))])))) trans_cycles]\<rparr>)"
+
+lemma ic_canister_status_cycles_inv:
+  assumes "ic_canister_status_pre n m S"
+  shows "total_cycles S = total_cycles (ic_canister_status_post n m S)"
+proof -
+  obtain orig cer cee mn a trans_cycles q where msg: "messages S ! n = Call_message orig cer cee mn a trans_cycles q"
+    using assms
+    by (auto simp: ic_canister_status_pre_def split: message.splits)
+  define older where "older = take n (messages S)"
+  define younger where "younger = drop (Suc n) (messages S)"
+  have msgs: "messages S = older @ Call_message orig cer cee mn a trans_cycles q # younger" "(older @ w # younger) ! n = w"
+    "take n older = older" "take (n - length older) ws = []" "drop (Suc n) older = []"
+    "drop (Suc n - length older) (w # ws) = ws" for w ws
+    using id_take_nth_drop[of n "messages S"] assms
+    by (auto simp: ic_canister_status_pre_def msg younger_def older_def nth_append)
+  show ?thesis
+    using assms
+    by (auto simp: ic_canister_status_pre_def ic_canister_status_post_def total_cycles_def Let_def msgs split: message.splits option.splits)
+qed
+
+lemma ic_canister_status_ic_inv:
+  assumes "ic_canister_status_pre n m S" "ic_inv S"
+  shows "ic_inv (ic_canister_status_post n m S)"
+  using assms
+  by (auto simp: ic_inv_def ic_canister_status_pre_def ic_canister_status_post_def Let_def
+      split: sum.splits message.splits call_origin.splits option.splits
+      dest!: in_set_takeD in_set_dropD nth_mem[of n "messages S"] in_set_updD list_map_range_setD list_map_get_range list_map_range_del)
+
+
+
+(* System transition: IC Management Canister: Code installation [DONE] *)
+
+definition ic_code_installation_pre :: "nat \<Rightarrow> ('p, 'uid, 'canid, 'b, 'w, 'sm, 'c, 's, 'cid, 'pk) ic \<Rightarrow> bool" where
+  "ic_code_installation_pre n S = (n < length (messages S) \<and> (case messages S ! n of Call_message orig cer cee mn a trans_cycles q \<Rightarrow>
+    (q = Unordered \<or> (\<forall>j < n. message_queue (messages S ! j) \<noteq> Some q)) \<and>
+    cee = ic_principal \<and>
+    mn = encode_string ''install_code'' \<and>
+    (case candid_parse_cid a of Some cid \<Rightarrow>
+    (case (candid_parse_text a [encode_string ''mode''], candid_parse_blob a [encode_string ''wasm_module''], candid_parse_blob a [encode_string ''arg'']) of
+      (Some mode, Some w, Some ar) \<Rightarrow>
+    (case parse_wasm_mod w of Some m \<Rightarrow>
+      parse_public_custom_sections w \<noteq> None \<and>
+      parse_private_custom_sections w \<noteq> None \<and>
+    (case (list_map_get (controllers S) cid, list_map_get (time S) cid, list_map_get (balances S) cid, list_map_get (canister_status S) cid) of
+      (Some ctrls, Some t, Some bal, Some can_status) \<Rightarrow>
+      let env = \<lparr>env.time = t, balance = bal, freezing_limit = ic_freezing_limit S cid, certificate = None, status = simple_status can_status\<rparr> in
+      ((mode = encode_string ''install'' \<and> (case list_map_get (canisters S) cid of Some None \<Rightarrow> True | _ \<Rightarrow> False)) \<or> mode = encode_string ''reinstall'') \<and>
+      cer \<in> ctrls \<and>
+      (case canister_module_init m (cid, ar, cer, env) of Inl _ \<Rightarrow> False
+      | Inr ret \<Rightarrow> cycles_return.cycles_used ret \<le> bal) \<and>
+      list_map_dom (canister_module_update_methods m) \<inter> list_map_dom (canister_module_query_methods m) = {}
+    | _ \<Rightarrow> False) | _ \<Rightarrow> False) | _ \<Rightarrow> False) | _ \<Rightarrow> False)
+  | _ \<Rightarrow> False))"
+
+definition ic_code_installation_post :: "nat \<Rightarrow> ('p, 'uid, 'canid, 'b, 'w, 'sm, 'c, 's, 'cid, 'pk) ic \<Rightarrow> ('p, 'uid, 'canid, 'b, 'w, 'sm, 'c, 's, 'cid, 'pk) ic" where
+  "ic_code_installation_post n S = (case messages S ! n of Call_message orig cer cee mn a trans_cycles q \<Rightarrow>
+    (case candid_parse_cid a of Some cid \<Rightarrow>
+    (case (candid_parse_text a [encode_string ''mode''], candid_parse_blob a [encode_string ''wasm_module''], candid_parse_blob a [encode_string ''arg'']) of
+      (Some mode, Some w, Some a) \<Rightarrow>
+    (case parse_wasm_mod w of Some m \<Rightarrow>
+    (case (list_map_get (time S) cid, list_map_get (balances S) cid, list_map_get (canister_status S) cid) of
+      (Some t, Some bal, Some can_status) \<Rightarrow>
+      let env = \<lparr>env.time = t, balance = bal, freezing_limit = ic_freezing_limit S cid, certificate = None, status = simple_status can_status\<rparr>;
+      (new_state, cyc_used) = (case canister_module_init m (cid, a, cer, env) of Inr ret \<Rightarrow> (cycles_return.return ret, cycles_return.cycles_used ret)) in
+    S\<lparr>canisters := list_map_set (canisters S) cid (Some \<lparr>wasm_state = new_state, module = m, raw_module = w,
+        public_custom_sections = the (parse_public_custom_sections w), private_custom_sections = the (parse_private_custom_sections w)\<rparr>),
+      balances := list_map_set (balances S) cid (bal - cyc_used),
+      messages := take n (messages S) @ drop (Suc n) (messages S) @ [Response_message orig (Reply (blob_of_candid Candid_empty)) trans_cycles]\<rparr>)))))"
+
+definition ic_code_installation_burned_cycles :: "nat \<Rightarrow> ('p, 'uid, 'canid, 'b, 'w, 'sm, 'c, 's, 'cid, 'pk) ic \<Rightarrow> nat" where
+  "ic_code_installation_burned_cycles n S = (case messages S ! n of Call_message orig cer cee mn a trans_cycles q \<Rightarrow>
+    (case candid_parse_cid a of Some cid \<Rightarrow>
+    (case (candid_parse_blob a [encode_string ''wasm_module''], candid_parse_blob a [encode_string ''arg'']) of
+      (Some w, Some a) \<Rightarrow>
+    (case parse_wasm_mod w of Some m \<Rightarrow>
+    (case (list_map_get (time S) cid, list_map_get (balances S) cid, list_map_get (canister_status S) cid) of
+      (Some t, Some bal, Some can_status) \<Rightarrow>
+      let env = \<lparr>env.time = t, balance = bal, freezing_limit = ic_freezing_limit S cid, certificate = None, status = simple_status can_status\<rparr> in
+      (case canister_module_init m (cid, a, cer, env) of Inr ret \<Rightarrow> cycles_return.cycles_used ret))))))"
+
+lemma ic_code_installation_cycles_inv:
+  assumes "ic_code_installation_pre n S"
+  shows "total_cycles S = total_cycles (ic_code_installation_post n S) + ic_code_installation_burned_cycles n S"
+proof -
+  obtain orig cer cee mn a trans_cycles q where msg: "messages S ! n = Call_message orig cer cee mn a trans_cycles q"
+    using assms
+    by (auto simp: ic_code_installation_pre_def split: message.splits)
+  define older where "older = take n (messages S)"
+  define younger where "younger = drop (Suc n) (messages S)"
+  have msgs: "messages S = older @ Call_message orig cer cee mn a trans_cycles q # younger" "(older @ w # younger) ! n = w"
+    "take n older = older" "take (n - length older) ws = []" "drop (Suc n) older = []"
+    "drop (Suc n - length older) (w # ws) = ws" for w ws
+    using id_take_nth_drop[of n "messages S"] assms
+    by (auto simp: ic_code_installation_pre_def msg younger_def older_def nth_append)
+  show ?thesis
+    using assms list_map_sum_in_ge[where ?f="balances S" and ?g=id and ?x="the (candid_parse_cid a)"]
+    by (auto simp: ic_code_installation_pre_def ic_code_installation_post_def ic_code_installation_burned_cycles_def total_cycles_def Let_def msgs list_map_sum_in[where ?f="balances S"] split: message.splits option.splits sum.splits prod.splits)
+qed
+
+lemma ic_code_installation_ic_inv:
+  assumes "ic_code_installation_pre n S" "ic_inv S"
+  shows "ic_inv (ic_code_installation_post n S)"
+proof -
+  obtain orig cer cee mn a trans_cycles q cid mode w ar m ctrls t bal can_status where msg: "messages S ! n = Call_message orig cer cee mn a trans_cycles q"
+    and parse: "candid_parse_cid a = Some cid"
+    "candid_parse_text a [encode_string ''mode''] = Some mode"
+    "candid_parse_blob a [encode_string ''wasm_module''] = Some w"
+    "candid_parse_blob a [encode_string ''arg''] = Some ar"
+    "parse_wasm_mod w = Some m"
+    and list_map_get:
+    "list_map_get (controllers S) cid = Some ctrls"
+    "list_map_get (time S) cid = Some t"
+    "list_map_get (balances S) cid = Some bal"
+    "list_map_get (canister_status S) cid = Some can_status"
+    using assms
+    by (auto simp: ic_code_installation_pre_def split: message.splits option.splits)
+  show ?thesis
+    using assms
+    by (auto simp: ic_inv_def ic_code_installation_pre_def ic_code_installation_post_def msg parse list_map_get Let_def
+        split: sum.splits call_origin.splits message.splits
+        dest!: in_set_takeD in_set_dropD nth_mem[of n "messages S"] in_set_updD list_map_range_setD list_map_get_range list_map_range_del)
+qed
+
+
+
+(* System transition: IC Management Canister: Code upgrade [DONE] *)
+
+definition ic_code_upgrade_pre :: "nat \<Rightarrow> ('p, 'uid, 'canid, 'b, 'w, 'sm, 'c, 's, 'cid, 'pk) ic \<Rightarrow> bool" where
+  "ic_code_upgrade_pre n S = (n < length (messages S) \<and> (case messages S ! n of Call_message orig cer cee mn a trans_cycles q \<Rightarrow>
+    (q = Unordered \<or> (\<forall>j < n. message_queue (messages S ! j) \<noteq> Some q)) \<and>
+    cee = ic_principal \<and>
+    mn = encode_string ''install_code'' \<and>
+    (case candid_parse_cid a of Some cid \<Rightarrow>
+    (case (candid_parse_text a [encode_string ''mode''], candid_parse_blob a [encode_string ''wasm_module''], candid_parse_blob a [encode_string ''arg'']) of
+      (Some mode, Some w, Some ar) \<Rightarrow>
+    (case parse_wasm_mod w of Some m \<Rightarrow>
+      parse_public_custom_sections w \<noteq> None \<and>
+      parse_private_custom_sections w \<noteq> None \<and>
+    (case (list_map_get (canisters S) cid, list_map_get (controllers S) cid, list_map_get (time S) cid, list_map_get (balances S) cid, list_map_get (canister_status S) cid) of
+      (Some (Some can), Some ctrls, Some t, Some bal, Some can_status) \<Rightarrow>
+      let env = \<lparr>env.time = t, balance = bal, freezing_limit = ic_freezing_limit S cid, certificate = None, status = simple_status can_status\<rparr> in
+      mode = encode_string ''upgrade'' \<and>
+      cer \<in> ctrls \<and>
+      (case canister_module_pre_upgrade (module can) (wasm_state can, cer, env) of Inr pre_ret \<Rightarrow>
+      (case canister_module_post_upgrade m (cid, cycles_return.return pre_ret, ar, cer, env) of Inr post_ret \<Rightarrow>
+        cycles_return.cycles_used pre_ret + cycles_return.cycles_used post_ret \<le> bal
+      | _ \<Rightarrow> False) | _ \<Rightarrow> False) \<and>
+      list_map_dom (canister_module_update_methods m) \<inter> list_map_dom (canister_module_query_methods m) = {}
+    | _ \<Rightarrow> False) | _ \<Rightarrow> False) | _ \<Rightarrow> False) | _ \<Rightarrow> False)
+  | _ \<Rightarrow> False))"
+
+definition ic_code_upgrade_post :: "nat \<Rightarrow> ('p, 'uid, 'canid, 'b, 'w, 'sm, 'c, 's, 'cid, 'pk) ic \<Rightarrow> ('p, 'uid, 'canid, 'b, 'w, 'sm, 'c, 's, 'cid, 'pk) ic" where
+  "ic_code_upgrade_post n S = (case messages S ! n of Call_message orig cer cee mn a trans_cycles q \<Rightarrow>
+    (case candid_parse_cid a of Some cid \<Rightarrow>
+    (case (candid_parse_text a [encode_string ''mode''], candid_parse_blob a [encode_string ''wasm_module''], candid_parse_blob a [encode_string ''arg'']) of
+      (Some mode, Some w, Some ar) \<Rightarrow>
+    (case parse_wasm_mod w of Some m \<Rightarrow>
+    (case (list_map_get (canisters S) cid, list_map_get (time S) cid, list_map_get (balances S) cid, list_map_get (canister_status S) cid) of
+      (Some (Some can), Some t, Some bal, Some can_status) \<Rightarrow>
+      let env = \<lparr>env.time = t, balance = bal, freezing_limit = ic_freezing_limit S cid, certificate = None, status = simple_status can_status\<rparr> in
+      (case canister_module_pre_upgrade (module can) (wasm_state can, cer, env) of Inr pre_ret \<Rightarrow>
+      (case canister_module_post_upgrade m (cid, cycles_return.return pre_ret, ar, cer, env) of Inr post_ret \<Rightarrow>
+    S\<lparr>canisters := list_map_set (canisters S) cid (Some \<lparr>wasm_state = cycles_return.return post_ret, module = m, raw_module = w,
+        public_custom_sections = the (parse_public_custom_sections w), private_custom_sections = the (parse_private_custom_sections w)\<rparr>),
+      balances := list_map_set (balances S) cid (bal - (cycles_return.cycles_used pre_ret + cycles_return.cycles_used post_ret)),
+      messages := take n (messages S) @ drop (Suc n) (messages S) @ [Response_message orig (Reply (blob_of_candid Candid_empty)) trans_cycles]\<rparr>)))))))"
+
+definition ic_code_upgrade_burned_cycles :: "nat \<Rightarrow> ('p, 'uid, 'canid, 'b, 'w, 'sm, 'c, 's, 'cid, 'pk) ic \<Rightarrow> nat" where
+  "ic_code_upgrade_burned_cycles n S = (case messages S ! n of Call_message orig cer cee mn a trans_cycles q \<Rightarrow>
+    (case candid_parse_cid a of Some cid \<Rightarrow>
+    (case (candid_parse_text a [encode_string ''mode''], candid_parse_blob a [encode_string ''wasm_module''], candid_parse_blob a [encode_string ''arg'']) of
+      (Some mode, Some w, Some ar) \<Rightarrow>
+    (case parse_wasm_mod w of Some m \<Rightarrow>
+    (case (list_map_get (canisters S) cid, list_map_get (time S) cid, list_map_get (balances S) cid, list_map_get (canister_status S) cid) of
+      (Some (Some can), Some t, Some bal, Some can_status) \<Rightarrow>
+      let env = \<lparr>env.time = t, balance = bal, freezing_limit = ic_freezing_limit S cid, certificate = None, status = simple_status can_status\<rparr> in
+      (case canister_module_pre_upgrade (module can) (wasm_state can, cer, env) of Inr pre_ret \<Rightarrow>
+      (case canister_module_post_upgrade m (cid, cycles_return.return pre_ret, ar, cer, env) of Inr post_ret \<Rightarrow>
+      cycles_return.cycles_used pre_ret + cycles_return.cycles_used post_ret)))))))"
+
+lemma ic_code_upgrade_cycles_inv:
+  assumes "ic_code_upgrade_pre n S"
+  shows "total_cycles S = total_cycles (ic_code_upgrade_post n S) + ic_code_upgrade_burned_cycles n S"
+proof -
+  obtain orig cer cee mn a trans_cycles q where msg: "messages S ! n = Call_message orig cer cee mn a trans_cycles q"
+    using assms
+    by (auto simp: ic_code_upgrade_pre_def split: message.splits)
+  define older where "older = take n (messages S)"
+  define younger where "younger = drop (Suc n) (messages S)"
+  have msgs: "messages S = older @ Call_message orig cer cee mn a trans_cycles q # younger" "(older @ w # younger) ! n = w"
+    "take n older = older" "take (n - length older) ws = []" "drop (Suc n) older = []"
+    "drop (Suc n - length older) (w # ws) = ws" for w ws
+    using id_take_nth_drop[of n "messages S"] assms
+    by (auto simp: ic_code_upgrade_pre_def msg younger_def older_def nth_append)
+  show ?thesis
+    using assms list_map_sum_in_ge[where ?f="balances S" and ?g=id and ?x="the (candid_parse_cid a)"]
+    by (auto simp: ic_code_upgrade_pre_def ic_code_upgrade_post_def ic_code_upgrade_burned_cycles_def total_cycles_def Let_def msgs list_map_sum_in[where ?f="balances S"] split: message.splits option.splits sum.splits)
+qed
+
+lemma ic_code_upgrade_ic_inv:
+  assumes "ic_code_upgrade_pre n S" "ic_inv S"
+  shows "ic_inv (ic_code_upgrade_post n S)"
+proof -
+  obtain orig cer cee mn a trans_cycles q cid mode w ar m can ctrls t bal can_status where msg: "messages S ! n = Call_message orig cer cee mn a trans_cycles q"
+    and parse: "candid_parse_cid a = Some cid"
+    "candid_parse_text a [encode_string ''mode''] = Some mode"
+    "candid_parse_blob a [encode_string ''wasm_module''] = Some w"
+    "candid_parse_blob a [encode_string ''arg''] = Some ar"
+    "parse_wasm_mod w = Some m"
+    and list_map_get:
+    "list_map_get (canisters S) cid = Some (Some can)"
+    "list_map_get (controllers S) cid = Some ctrls"
+    "list_map_get (time S) cid = Some t"
+    "list_map_get (balances S) cid = Some bal"
+    "list_map_get (canister_status S) cid = Some can_status"
+    using assms
+    by (auto simp: ic_code_upgrade_pre_def split: message.splits option.splits)
+  show ?thesis
+    using assms
+    by (auto simp: ic_inv_def ic_code_upgrade_pre_def ic_code_upgrade_post_def msg parse list_map_get Let_def
+        split: sum.splits call_origin.splits message.splits
+        dest!: in_set_takeD in_set_dropD nth_mem[of n "messages S"] in_set_updD list_map_range_setD list_map_get_range list_map_range_del)
+qed
+
+
+
+(* System transition: IC Management Canister: Code uninstallation [DONE] *)
+
+definition ic_code_uninstallation_pre :: "nat \<Rightarrow> ('p, 'uid, 'canid, 'b, 'w, 'sm, 'c, 's, 'cid, 'pk) ic \<Rightarrow> bool" where
+  "ic_code_uninstallation_pre n S = (n < length (messages S) \<and> (case messages S ! n of Call_message orig cer cee mn a trans_cycles q \<Rightarrow>
+    (q = Unordered \<or> (\<forall>j < n. message_queue (messages S ! j) \<noteq> Some q)) \<and>
+    cee = ic_principal \<and>
+    mn = encode_string ''uninstall_code'' \<and>
+    (case candid_parse_cid a of Some cid \<Rightarrow>
+    (case list_map_get (controllers S) cid of Some ctrls \<Rightarrow> cer \<in> ctrls
+    | _ \<Rightarrow> False) | _ \<Rightarrow> False)
+  | _ \<Rightarrow> False))"
+
+definition ic_code_uninstallation_post :: "nat \<Rightarrow> ('p, 'uid, 'canid, 'b, 'w, 'sm, 'c, 's, 'cid, 'pk) ic \<Rightarrow> ('p, 'uid, 'canid, 'b, 'w, 'sm, 'c, 's, 'cid, 'pk) ic" where
+  "ic_code_uninstallation_post n S = (case messages S ! n of Call_message orig cer cee mn a trans_cycles q \<Rightarrow>
+    (case candid_parse_cid a of Some cid \<Rightarrow>
+    let call_ctxt_to_msg = (\<lambda>ctxt.
+      if call_ctxt_canister ctxt = cid \<and> call_ctxt_needs_to_respond ctxt then
+        Some (Response_message (call_ctxt_origin ctxt) (response.Reject CANISTER_REJECT (encode_string ''Canister has been uninstalled'')) (call_ctxt_available_cycles ctxt))
+      else None);
+    call_ctxt_to_ctxt = (\<lambda>ctxt. if call_ctxt_canister ctxt = cid then call_ctxt_delete ctxt else ctxt) in
+    S\<lparr>canisters := list_map_set (canisters S) cid None, certified_data := list_map_set (certified_data S) cid empty_blob,
+      messages := take n (messages S) @ drop (Suc n) (messages S) @ [Response_message orig (Reply (blob_of_candid Candid_empty)) trans_cycles] @
+        List.map_filter call_ctxt_to_msg (list_map_vals (call_contexts S)),
+      call_contexts := list_map_map call_ctxt_to_ctxt (call_contexts S)\<rparr>))"
+
+lemma ic_code_uninstallation_cycles_inv:
+  assumes "ic_code_uninstallation_pre n S"
+  shows "total_cycles S = total_cycles (ic_code_uninstallation_post n S)"
+proof -
+  obtain orig cer cee mn a trans_cycles q cid where msg: "messages S ! n = Call_message orig cer cee mn a trans_cycles q"
+    and cid_def: "candid_parse_cid a = Some cid"
+    using assms
+    by (auto simp: ic_code_uninstallation_pre_def split: message.splits option.splits)
+  define older where "older = take n (messages S)"
+  define younger where "younger = drop (Suc n) (messages S)"
+  have msgs: "messages S = older @ Call_message orig cer cee mn a trans_cycles q # younger" "(older @ w # younger) ! n = w"
+    "take n older = older" "take (n - length older) ws = []" "drop (Suc n) older = []"
+    "drop (Suc n - length older) (w # ws) = ws" for w ws
+    using id_take_nth_drop[of n "messages S"] assms
+    by (auto simp: ic_code_uninstallation_pre_def msg younger_def older_def nth_append)
+  have F1: "list_map_sum_vals call_ctxt_carried_cycles (call_contexts S) =
+    list_map_sum_vals id
+      (list_map_map (\<lambda>ctxt. if call_ctxt_canister ctxt = cid then call_ctxt_carried_cycles ctxt else 0) (call_contexts S)) +
+    list_map_sum_vals call_ctxt_carried_cycles
+      (list_map_map (\<lambda>ctxt. if call_ctxt_canister ctxt = cid then call_ctxt_delete ctxt else ctxt) (call_contexts S))"
+    using list_map_sum_vals_split[where ?f="call_ctxt_carried_cycles" and ?g="call_ctxt_delete", unfolded call_ctxt_delete_carried_cycles diff_zero]
+    by auto
+  show ?thesis
+    using assms
+    by (auto simp: ic_code_uninstallation_pre_def ic_code_uninstallation_post_def total_cycles_def call_ctxt_carried_cycles cid_def Let_def msgs F1
+        split: message.splits option.splits sum.splits if_splits intro!: list_map_sum_vals_filter)
+qed
+
+lemma ic_code_uninstallation_ic_inv:
+  assumes "ic_code_uninstallation_pre n S" "ic_inv S"
+  shows "ic_inv (ic_code_uninstallation_post n S)"
+  using assms
+  by (auto simp: ic_inv_def ic_code_uninstallation_pre_def ic_code_uninstallation_post_def Let_def
+      split: sum.splits message.splits call_origin.splits option.splits if_splits
+      dest!: in_set_takeD in_set_dropD nth_mem[of n "messages S"] in_set_updD list_map_range_setD list_map_get_range list_map_range_del
+      in_set_map_filter_vals)
+
+
+
+(* System transition: IC Management Canister: Stopping a canister (running) [DONE] *)
+
+definition ic_canister_stop_running_pre :: "nat \<Rightarrow> ('p, 'uid, 'canid, 'b, 'w, 'sm, 'c, 's, 'cid, 'pk) ic \<Rightarrow> bool" where
+  "ic_canister_stop_running_pre n S = (n < length (messages S) \<and> (case messages S ! n of Call_message orig cer cee mn a trans_cycles q \<Rightarrow>
+    (q = Unordered \<or> (\<forall>j < n. message_queue (messages S ! j) \<noteq> Some q)) \<and>
+    cee = ic_principal \<and>
+    mn = encode_string ''stop_canister'' \<and>
+    (case candid_parse_cid a of Some cid \<Rightarrow>
+    (case (list_map_get (canister_status S) cid, list_map_get (controllers S) cid) of (Some Running, Some ctrls) \<Rightarrow>
+      cer \<in> ctrls
+    | _ \<Rightarrow> False) | _ \<Rightarrow> False)
+  | _ \<Rightarrow> False))"
+
+definition ic_canister_stop_running_post :: "nat \<Rightarrow> ('p, 'uid, 'canid, 'b, 'w, 'sm, 'c, 's, 'cid, 'pk) ic \<Rightarrow> ('p, 'uid, 'canid, 'b, 'w, 'sm, 'c, 's, 'cid, 'pk) ic" where
+  "ic_canister_stop_running_post n S = (case messages S ! n of Call_message orig cer cee mn a trans_cycles q \<Rightarrow>
+    let cid = the (candid_parse_cid a) in
+    S\<lparr>messages := take n (messages S) @ drop (Suc n) (messages S),
+      canister_status := list_map_set (canister_status S) cid (Stopping [(orig, trans_cycles)])\<rparr>)"
+
+lemma ic_canister_stop_running_cycles_inv:
+  assumes "ic_canister_stop_running_pre n S"
+  shows "total_cycles S = total_cycles (ic_canister_stop_running_post n S)"
+proof -
+  obtain orig cer cee mn a trans_cycles q cid where msg: "messages S ! n = Call_message orig cer cee mn a trans_cycles q"
+    and cid_def: "candid_parse_cid a = Some cid"
+    using assms
+    by (auto simp: ic_canister_stop_running_pre_def split: message.splits option.splits)
+  define older where "older = take n (messages S)"
+  define younger where "younger = drop (Suc n) (messages S)"
+  have msgs: "messages S = older @ Call_message orig cer cee mn a trans_cycles q # younger" "(older @ w # younger) ! n = w"
+    "take n older = older" "take (n - length older) ws = []" "drop (Suc n) older = []"
+    "drop (Suc n - length older) (w # ws) = ws" for w ws
+    using id_take_nth_drop[of n "messages S"] assms
+    by (auto simp: ic_canister_stop_running_pre_def msg younger_def older_def nth_append)
+  show ?thesis
+    using assms
+    by (auto simp: ic_canister_stop_running_pre_def ic_canister_stop_running_post_def total_cycles_def call_ctxt_carried_cycles cid_def Let_def msgs
+        list_map_sum_in[where ?g=status_cycles] split: message.splits option.splits sum.splits can_status.splits)
+qed
+
+lemma ic_canister_stop_running_ic_inv:
+  assumes "ic_canister_stop_running_pre n S" "ic_inv S"
+  shows "ic_inv (ic_canister_stop_running_post n S)"
+proof -
+  obtain orig cer cee mn a trans_cycles q cid where msg: "messages S ! n = Call_message orig cer cee mn a trans_cycles q"
+    and cid_def: "candid_parse_cid a = Some cid"
+    using assms
+    by (auto simp: ic_canister_stop_running_pre_def split: message.splits option.splits)
+  show ?thesis
+    using assms
+    by (force simp: ic_inv_def ic_canister_stop_running_pre_def ic_canister_stop_running_post_def msg Let_def
+        split: sum.splits message.splits call_origin.splits option.splits if_splits can_status.splits
+        dest!: in_set_takeD in_set_dropD nth_mem[of n "messages S"] in_set_updD list_map_range_setD list_map_get_range list_map_range_del
+        in_set_map_filter_vals intro!: ic_can_status_inv_stopping[where ?x="list_map_range (canister_status S)" and ?os=orig])
+qed
+
+
+
+(* System transition: IC Management Canister: Stopping a canister (stopping) [DONE] *)
+
+definition ic_canister_stop_stopping_pre :: "nat \<Rightarrow> ('p, 'uid, 'canid, 'b, 'w, 'sm, 'c, 's, 'cid, 'pk) ic \<Rightarrow> bool" where
+  "ic_canister_stop_stopping_pre n S = (n < length (messages S) \<and> (case messages S ! n of Call_message orig cer cee mn a trans_cycles q \<Rightarrow>
+    (q = Unordered \<or> (\<forall>j < n. message_queue (messages S ! j) \<noteq> Some q)) \<and>
+    cee = ic_principal \<and>
+    mn = encode_string ''stop_canister'' \<and>
+    (case candid_parse_cid a of Some cid \<Rightarrow>
+    (case (list_map_get (canister_status S) cid, list_map_get (controllers S) cid) of (Some (Stopping os), Some ctrls) \<Rightarrow>
+      cer \<in> ctrls
+    | _ \<Rightarrow> False) | _ \<Rightarrow> False)
+  | _ \<Rightarrow> False))"
+
+definition ic_canister_stop_stopping_post :: "nat \<Rightarrow> ('p, 'uid, 'canid, 'b, 'w, 'sm, 'c, 's, 'cid, 'pk) ic \<Rightarrow> ('p, 'uid, 'canid, 'b, 'w, 'sm, 'c, 's, 'cid, 'pk) ic" where
+  "ic_canister_stop_stopping_post n S = (case messages S ! n of Call_message orig cer cee mn a trans_cycles q \<Rightarrow>
+    let cid = the (candid_parse_cid a) in
+    (case list_map_get (canister_status S) cid of Some (Stopping os) \<Rightarrow>
+    S\<lparr>messages := take n (messages S) @ drop (Suc n) (messages S),
+      canister_status := list_map_set (canister_status S) cid (Stopping (os @ [(orig, trans_cycles)]))\<rparr>))"
+
+lemma ic_canister_stop_stopping_cycles_inv:
+  assumes "ic_canister_stop_stopping_pre n S"
+  shows "total_cycles S = total_cycles (ic_canister_stop_stopping_post n S)"
+proof -
+  obtain orig cer cee mn a trans_cycles q cid where msg: "messages S ! n = Call_message orig cer cee mn a trans_cycles q"
+    and cid_def: "candid_parse_cid a = Some cid"
+    using assms
+    by (auto simp: ic_canister_stop_stopping_pre_def split: message.splits option.splits)
+  define older where "older = take n (messages S)"
+  define younger where "younger = drop (Suc n) (messages S)"
+  have msgs: "messages S = older @ Call_message orig cer cee mn a trans_cycles q # younger" "(older @ w # younger) ! n = w"
+    "take n older = older" "take (n - length older) ws = []" "drop (Suc n) older = []"
+    "drop (Suc n - length older) (w # ws) = ws" for w ws
+    using id_take_nth_drop[of n "messages S"] assms
+    by (auto simp: ic_canister_stop_stopping_pre_def msg younger_def older_def nth_append)
+  show ?thesis
+    using assms
+    by (auto simp: ic_canister_stop_stopping_pre_def ic_canister_stop_stopping_post_def total_cycles_def call_ctxt_carried_cycles cid_def Let_def msgs
+        list_map_sum_in[where ?g=status_cycles] split: message.splits option.splits sum.splits can_status.splits)
+qed
+
+lemma ic_canister_stop_stopping_ic_inv:
+  assumes "ic_canister_stop_stopping_pre n S" "ic_inv S"
+  shows "ic_inv (ic_canister_stop_stopping_post n S)"
+proof -
+  obtain orig cer cee mn a trans_cycles q cid where msg: "messages S ! n = Call_message orig cer cee mn a trans_cycles q"
+    and cid_def: "candid_parse_cid a = Some cid"
+    using assms
+    by (auto simp: ic_canister_stop_stopping_pre_def split: message.splits option.splits)
+  show ?thesis
+    using assms
+    by (force simp: ic_inv_def ic_canister_stop_stopping_pre_def ic_canister_stop_stopping_post_def msg Let_def
+        split: sum.splits message.splits call_origin.splits option.splits if_splits can_status.splits
+        dest!: in_set_takeD in_set_dropD nth_mem[of n "messages S"] in_set_updD list_map_range_setD list_map_get_range list_map_range_del
+        in_set_map_filter_vals intro!: ic_can_status_inv_stopping_app[where ?x="list_map_range (canister_status S)" and ?os=orig])
+qed
+
+
+
+(* System transition: IC Management Canister: Stopping a canister (done stopping) [DONE] *)
+
+definition ic_canister_stop_done_stopping_pre :: "'canid \<Rightarrow> ('p, 'uid, 'canid, 'b, 'w, 'sm, 'c, 's, 'cid, 'pk) ic \<Rightarrow> bool" where
+  "ic_canister_stop_done_stopping_pre cid S =
+    (case list_map_get (canister_status S) cid of Some (Stopping os) \<Rightarrow>
+      (\<forall>ctxt \<in> list_map_range (call_contexts S). call_ctxt_canister ctxt \<noteq> cid)
+    | _ \<Rightarrow> False)"
+
+definition ic_canister_stop_done_stopping_post :: "'canid \<Rightarrow> ('p, 'uid, 'canid, 'b, 'w, 'sm, 'c, 's, 'cid, 'pk) ic \<Rightarrow> ('p, 'uid, 'canid, 'b, 'w, 'sm, 'c, 's, 'cid, 'pk) ic" where
+  "ic_canister_stop_done_stopping_post cid S = (
+    let orig_cycles_to_msg = (\<lambda>(or, cyc). Response_message or (Reply (blob_of_candid Candid_empty)) cyc) in
+    (case list_map_get (canister_status S) cid of Some (Stopping os) \<Rightarrow>
+    S\<lparr>canister_status := list_map_set (canister_status S) cid Stopped,
+      messages := messages S @ map orig_cycles_to_msg os\<rparr>))"
+
+lemma ic_canister_stop_done_stopping_cycles_inv:
+  assumes "ic_canister_stop_done_stopping_pre cid S"
+  shows "total_cycles S = total_cycles (ic_canister_stop_done_stopping_post cid S)"
+proof -
+  have F1: "(message_cycles \<circ> (\<lambda>(or, y). Response_message or (Reply (blob_of_candid Candid_empty)) y)) = (\<lambda>(or, y). carried_cycles or + y)"
+    by auto
+  have F2: "(\<Sum>(or, y)\<leftarrow>xs. carried_cycles or + y) = sum_list (map (carried_cycles \<circ> fst) xs) + sum_list (map snd xs)" for xs
+    by (induction xs) auto
+  show ?thesis
+    using assms list_map_sum_in_ge[where ?g=status_cycles and ?f="canister_status S" and ?x=cid]
+    by (auto simp: ic_canister_stop_done_stopping_pre_def ic_canister_stop_done_stopping_post_def total_cycles_def call_ctxt_carried_cycles Let_def
+        F1 F2 list_map_sum_in[where ?g=status_cycles] split: message.splits option.splits sum.splits can_status.splits)
+qed
+
+lemma ic_canister_stop_done_stopping_ic_inv:
+  assumes "ic_canister_stop_done_stopping_pre cid S" "ic_inv S"
+  shows "ic_inv (ic_canister_stop_done_stopping_post cid S)"
+  using assms
+  by (force simp: ic_inv_def ic_can_status_inv_def ic_canister_stop_done_stopping_pre_def ic_canister_stop_done_stopping_post_def Let_def
+      split: sum.splits message.splits call_origin.splits option.splits if_splits can_status.splits
+      dest!: in_set_takeD in_set_dropD in_set_updD list_map_range_setD list_map_get_range list_map_range_del
+      in_set_map_filter_vals)
+
+
+
+(* System transition: IC Management Canister: Stopping a canister (stopped) [DONE] *)
+
+definition ic_canister_stop_stopped_pre :: "nat \<Rightarrow> ('p, 'uid, 'canid, 'b, 'w, 'sm, 'c, 's, 'cid, 'pk) ic \<Rightarrow> bool" where
+  "ic_canister_stop_stopped_pre n S = (n < length (messages S) \<and> (case messages S ! n of Call_message orig cer cee mn a trans_cycles q \<Rightarrow>
+    (q = Unordered \<or> (\<forall>j < n. message_queue (messages S ! j) \<noteq> Some q)) \<and>
+    cee = ic_principal \<and>
+    mn = encode_string ''stop_canister'' \<and>
+    (case candid_parse_cid a of Some cid \<Rightarrow>
+    (case (list_map_get (canister_status S) cid, list_map_get (controllers S) cid) of (Some Stopped, Some ctrls) \<Rightarrow>
+      cer \<in> ctrls
+    | _ \<Rightarrow> False) | _ \<Rightarrow> False)
+  | _ \<Rightarrow> False))"
+
+definition ic_canister_stop_stopped_post :: "nat \<Rightarrow> ('p, 'uid, 'canid, 'b, 'w, 'sm, 'c, 's, 'cid, 'pk) ic \<Rightarrow> ('p, 'uid, 'canid, 'b, 'w, 'sm, 'c, 's, 'cid, 'pk) ic" where
+  "ic_canister_stop_stopped_post n S = (case messages S ! n of Call_message orig cer cee mn a trans_cycles q \<Rightarrow>
+    S\<lparr>messages := take n (messages S) @ drop (Suc n) (messages S) @ [Response_message orig (Reply (blob_of_candid Candid_empty)) trans_cycles]\<rparr>)"
+
+lemma ic_canister_stop_stopped_cycles_inv:
+  assumes "ic_canister_stop_stopped_pre n S"
+  shows "total_cycles S = total_cycles (ic_canister_stop_stopped_post n S)"
+proof -
+  obtain orig cer cee mn a trans_cycles q cid where msg: "messages S ! n = Call_message orig cer cee mn a trans_cycles q"
+    and cid_def: "candid_parse_cid a = Some cid"
+    using assms
+    by (auto simp: ic_canister_stop_stopped_pre_def split: message.splits option.splits)
+  define older where "older = take n (messages S)"
+  define younger where "younger = drop (Suc n) (messages S)"
+  have msgs: "messages S = older @ Call_message orig cer cee mn a trans_cycles q # younger" "(older @ w # younger) ! n = w"
+    "take n older = older" "take (n - length older) ws = []" "drop (Suc n) older = []"
+    "drop (Suc n - length older) (w # ws) = ws" for w ws
+    using id_take_nth_drop[of n "messages S"] assms
+    by (auto simp: ic_canister_stop_stopped_pre_def msg younger_def older_def nth_append)
+  show ?thesis
+    using assms
+    by (auto simp: ic_canister_stop_stopped_pre_def ic_canister_stop_stopped_post_def total_cycles_def call_ctxt_carried_cycles cid_def Let_def msgs
+        split: message.splits option.splits sum.splits can_status.splits)
+qed
+
+lemma ic_canister_stop_stopped_ic_inv:
+  assumes "ic_canister_stop_stopped_pre n S" "ic_inv S"
+  shows "ic_inv (ic_canister_stop_stopped_post n S)"
+  using assms
+  by (auto simp: ic_inv_def ic_canister_stop_stopped_pre_def ic_canister_stop_stopped_post_def Let_def
+      split: sum.splits message.splits call_origin.splits option.splits if_splits can_status.splits
+      dest!: in_set_takeD in_set_dropD nth_mem[of n "messages S"] in_set_updD list_map_range_setD list_map_get_range list_map_range_del
+      in_set_map_filter_vals)
+
+
+
+(* System transition: IC Management Canister: Starting a canister (not stopping) [DONE] *)
+
+definition ic_canister_start_not_stopping_pre :: "nat \<Rightarrow> ('p, 'uid, 'canid, 'b, 'w, 'sm, 'c, 's, 'cid, 'pk) ic \<Rightarrow> bool" where
+  "ic_canister_start_not_stopping_pre n S = (n < length (messages S) \<and> (case messages S ! n of Call_message orig cer cee mn a trans_cycles q \<Rightarrow>
+    (q = Unordered \<or> (\<forall>j < n. message_queue (messages S ! j) \<noteq> Some q)) \<and>
+    cee = ic_principal \<and>
+    mn = encode_string ''start_canister'' \<and>
+    (case candid_parse_cid a of Some cid \<Rightarrow>
+    (case (list_map_get (canister_status S) cid, list_map_get (controllers S) cid) of (Some can_status, Some ctrls) \<Rightarrow>
+      (can_status = Running \<or> can_status = Stopped) \<and>
+      cer \<in> ctrls
+    | _ \<Rightarrow> False) | _ \<Rightarrow> False)
+  | _ \<Rightarrow> False))"
+
+definition ic_canister_start_not_stopping_post :: "nat \<Rightarrow> ('p, 'uid, 'canid, 'b, 'w, 'sm, 'c, 's, 'cid, 'pk) ic \<Rightarrow> ('p, 'uid, 'canid, 'b, 'w, 'sm, 'c, 's, 'cid, 'pk) ic" where
+  "ic_canister_start_not_stopping_post n S = (case messages S ! n of Call_message orig cer cee mn a trans_cycles q \<Rightarrow>
+    let cid = the (candid_parse_cid a) in
+    S\<lparr>canister_status := list_map_set (canister_status S) cid Running,
+      messages := take n (messages S) @ drop (Suc n) (messages S) @ [Response_message orig (Reply (blob_of_candid Candid_empty)) trans_cycles]\<rparr>)"
+
+lemma ic_canister_start_not_stopping_cycles_inv:
+  assumes "ic_canister_start_not_stopping_pre n S"
+  shows "total_cycles S = total_cycles (ic_canister_start_not_stopping_post n S)"
+proof -
+  obtain orig cer cee mn a trans_cycles q cid where msg: "messages S ! n = Call_message orig cer cee mn a trans_cycles q"
+    and cid_def: "candid_parse_cid a = Some cid"
+    using assms
+    by (auto simp: ic_canister_start_not_stopping_pre_def split: message.splits option.splits)
+  define older where "older = take n (messages S)"
+  define younger where "younger = drop (Suc n) (messages S)"
+  have msgs: "messages S = older @ Call_message orig cer cee mn a trans_cycles q # younger" "(older @ w # younger) ! n = w"
+    "take n older = older" "take (n - length older) ws = []" "drop (Suc n) older = []"
+    "drop (Suc n - length older) (w # ws) = ws" for w ws
+    using id_take_nth_drop[of n "messages S"] assms
+    by (auto simp: ic_canister_start_not_stopping_pre_def msg younger_def older_def nth_append)
+  show ?thesis
+    using assms
+    by (auto simp: ic_canister_start_not_stopping_pre_def ic_canister_start_not_stopping_post_def total_cycles_def call_ctxt_carried_cycles cid_def Let_def msgs
+        list_map_sum_in[where ?g=status_cycles] split: message.splits option.splits sum.splits)
+qed
+
+lemma ic_canister_start_not_stopping_ic_inv:
+  assumes "ic_canister_start_not_stopping_pre n S" "ic_inv S"
+  shows "ic_inv (ic_canister_start_not_stopping_post n S)"
+  using assms
+  by (auto simp: ic_inv_def ic_canister_start_not_stopping_pre_def ic_canister_start_not_stopping_post_def Let_def
+      split: sum.splits message.splits call_origin.splits option.splits if_splits can_status.splits
+      dest!: in_set_takeD in_set_dropD nth_mem[of n "messages S"] in_set_updD list_map_range_setD list_map_get_range list_map_range_del
+      in_set_map_filter_vals intro: ic_can_status_inv_mono1)
+
+
+
+(* System transition: IC Management Canister: Starting a canister (stopping) [DONE] *)
+
+definition ic_canister_start_stopping_pre :: "nat \<Rightarrow> ('p, 'uid, 'canid, 'b, 'w, 'sm, 'c, 's, 'cid, 'pk) ic \<Rightarrow> bool" where
+  "ic_canister_start_stopping_pre n S = (n < length (messages S) \<and> (case messages S ! n of Call_message orig cer cee mn a trans_cycles q \<Rightarrow>
+    (q = Unordered \<or> (\<forall>j < n. message_queue (messages S ! j) \<noteq> Some q)) \<and>
+    cee = ic_principal \<and>
+    mn = encode_string ''start_canister'' \<and>
+    (case candid_parse_cid a of Some cid \<Rightarrow>
+    (case (list_map_get (canister_status S) cid, list_map_get (controllers S) cid) of (Some (Stopping _), Some ctrls) \<Rightarrow>
+      cer \<in> ctrls
+    | _ \<Rightarrow> False) | _ \<Rightarrow> False)
+  | _ \<Rightarrow> False))"
+
+definition ic_canister_start_stopping_post :: "nat \<Rightarrow> ('p, 'uid, 'canid, 'b, 'w, 'sm, 'c, 's, 'cid, 'pk) ic \<Rightarrow> ('p, 'uid, 'canid, 'b, 'w, 'sm, 'c, 's, 'cid, 'pk) ic" where
+  "ic_canister_start_stopping_post n S = (case messages S ! n of Call_message orig cer cee mn a trans_cycles q \<Rightarrow>
+    let cid = the (candid_parse_cid a);
+    orig_cycles_to_msg = (\<lambda>(or, cyc). Response_message or (response.Reject CANISTER_REJECT (encode_string ''Canister has been restarted'')) cyc) in
+    (case list_map_get (canister_status S) cid of Some (Stopping os) \<Rightarrow>
+    S\<lparr>canister_status := list_map_set (canister_status S) cid Running,
+      messages := take n (messages S) @ drop (Suc n) (messages S) @ Response_message orig (Reply (blob_of_candid Candid_empty)) trans_cycles #
+      map orig_cycles_to_msg os\<rparr>))"
+
+lemma ic_canister_start_stopping_cycles_inv:
+  assumes "ic_canister_start_stopping_pre n S"
+  shows "total_cycles S = total_cycles (ic_canister_start_stopping_post n S)"
+proof -
+  obtain orig cer cee mn a trans_cycles q cid where msg: "messages S ! n = Call_message orig cer cee mn a trans_cycles q"
+    and cid_def: "candid_parse_cid a = Some cid"
+    using assms
+    by (auto simp: ic_canister_start_stopping_pre_def split: message.splits option.splits)
+  define older where "older = take n (messages S)"
+  define younger where "younger = drop (Suc n) (messages S)"
+  have msgs: "messages S = older @ Call_message orig cer cee mn a trans_cycles q # younger" "(older @ w # younger) ! n = w"
+    "take n older = older" "take (n - length older) ws = []" "drop (Suc n) older = []"
+    "drop (Suc n - length older) (w # ws) = ws" for w ws
+    using id_take_nth_drop[of n "messages S"] assms
+    by (auto simp: ic_canister_start_stopping_pre_def msg younger_def older_def nth_append)
+  have F1: "(message_cycles \<circ> (\<lambda>(or, y). Response_message or (response.Reject CANISTER_REJECT (encode_string ''Canister has been restarted'')) y)) = (\<lambda>(or, y). carried_cycles or + y)"
+    by auto
+  have F2: "(\<Sum>(or, y)\<leftarrow>xs. carried_cycles or + y) = sum_list (map (carried_cycles \<circ> fst) xs) + sum_list (map snd xs)" for xs
+    by (induction xs) auto
+  show ?thesis
+    using assms list_map_sum_in_ge[where ?g=status_cycles and ?f="canister_status S" and ?x=cid]
+    by (auto simp: ic_canister_start_stopping_pre_def ic_canister_start_stopping_post_def total_cycles_def call_ctxt_carried_cycles cid_def Let_def msgs F1 F2
+        list_map_sum_in[where ?g=status_cycles and ?f="canister_status S"]
+        split: message.splits option.splits sum.splits can_status.splits)
+qed
+
+lemma ic_canister_start_stopping_ic_inv:
+  assumes "ic_canister_start_stopping_pre n S" "ic_inv S"
+  shows "ic_inv (ic_canister_start_stopping_post n S)"
+  using assms
+  apply (auto simp: ic_inv_def ic_canister_start_stopping_pre_def ic_canister_start_stopping_post_def Let_def
+      split: sum.splits message.splits call_origin.splits option.splits if_splits can_status.splits
+      dest!: in_set_takeD in_set_dropD nth_mem[of n "messages S"] in_set_updD list_map_range_setD list_map_get_range list_map_range_del in_set_map_filter_vals
+      intro: ic_can_status_inv_mono1)
+   apply (fastforce simp: ic_can_status_inv_def)+
+  done
+
+
+
+(* System transition: IC Management Canister: Canister deletion [DONE] *)
+
+definition ic_canister_deletion_pre :: "nat \<Rightarrow> ('p, 'uid, 'canid, 'b, 'w, 'sm, 'c, 's, 'cid, 'pk) ic \<Rightarrow> bool" where
+  "ic_canister_deletion_pre n S = (n < length (messages S) \<and> (case messages S ! n of Call_message orig cer cee mn a trans_cycles q \<Rightarrow>
+    (q = Unordered \<or> (\<forall>j < n. message_queue (messages S ! j) \<noteq> Some q)) \<and>
+    cee = ic_principal \<and>
+    mn = encode_string ''delete_canister'' \<and>
+    (case candid_parse_cid a of Some cid \<Rightarrow>
+    (case (list_map_get (canister_status S) cid, list_map_get (controllers S) cid, list_map_get (balances S) cid) of (Some Stopped, Some ctrls, Some bal) \<Rightarrow>
+      cer \<in> ctrls
+    | _ \<Rightarrow> False) | _ \<Rightarrow> False)
+  | _ \<Rightarrow> False))"
+
+definition ic_canister_deletion_post :: "nat \<Rightarrow> ('p, 'uid, 'canid, 'b, 'w, 'sm, 'c, 's, 'cid, 'pk) ic \<Rightarrow> ('p, 'uid, 'canid, 'b, 'w, 'sm, 'c, 's, 'cid, 'pk) ic" where
+  "ic_canister_deletion_post n S = (case messages S ! n of Call_message orig cer cee mn a trans_cycles q \<Rightarrow>
+    let cid = the (candid_parse_cid a) in
+    S\<lparr>canisters := list_map_del (canisters S) cid,
+      controllers := list_map_del (controllers S) cid,
+      freezing_threshold := list_map_del (freezing_threshold S) cid,
+      canister_status := list_map_del (canister_status S) cid,
+      time := list_map_del (time S) cid,
+      balances := list_map_del (balances S) cid,
+      certified_data := list_map_del (certified_data S) cid,
+      messages := take n (messages S) @ drop (Suc n) (messages S) @ [Response_message orig (Reply (blob_of_candid Candid_empty)) trans_cycles]\<rparr>)"
+
+definition ic_canister_deletion_burned_cycles :: "nat \<Rightarrow> ('p, 'uid, 'canid, 'b, 'w, 'sm, 'c, 's, 'cid, 'pk) ic \<Rightarrow> nat" where
+  "ic_canister_deletion_burned_cycles n S = (case messages S ! n of Call_message orig cer cee mn a trans_cycles q \<Rightarrow>
+    let cid = the (candid_parse_cid a) in the (list_map_get (balances S) cid))"
+
+lemma ic_canister_deletion_cycles_monotonic:
+  assumes "ic_canister_deletion_pre n S"
+  shows "total_cycles S = total_cycles (ic_canister_deletion_post n S) + ic_canister_deletion_burned_cycles n S"
+proof -
+  obtain orig cer cee mn a trans_cycles q cid where msg: "messages S ! n = Call_message orig cer cee mn a trans_cycles q"
+    and cid_def: "candid_parse_cid a = Some cid"
+    using assms
+    by (auto simp: ic_canister_deletion_pre_def split: message.splits option.splits)
+  define older where "older = take n (messages S)"
+  define younger where "younger = drop (Suc n) (messages S)"
+  have msgs: "messages S = older @ Call_message orig cer cee mn a trans_cycles q # younger" "(older @ w # younger) ! n = w"
+    "take n older = older" "take (n - length older) ws = []" "drop (Suc n) older = []"
+    "drop (Suc n - length older) (w # ws) = ws" for w ws
+    using id_take_nth_drop[of n "messages S"] assms
+    by (auto simp: ic_canister_deletion_pre_def msg younger_def older_def nth_append)
+  show ?thesis
+    using assms
+    by (auto simp: ic_canister_deletion_pre_def ic_canister_deletion_post_def ic_canister_deletion_burned_cycles_def total_cycles_def call_ctxt_carried_cycles cid_def Let_def msgs
+        list_map_del_sum[where ?g=id and ?f="balances S"] list_map_del_sum[where ?g=status_cycles and ?f="canister_status S"]
+        split: message.splits option.splits sum.splits can_status.splits)
+qed
+
+lemma ic_canister_deletion_ic_inv:
+  assumes "ic_canister_deletion_pre n S" "ic_inv S"
+  shows "ic_inv (ic_canister_deletion_post n S)"
+  using assms
+  by (auto simp: ic_inv_def ic_canister_deletion_pre_def ic_canister_deletion_post_def Let_def
+      split: sum.splits message.splits call_origin.splits option.splits if_splits can_status.splits
+      dest!: in_set_takeD in_set_dropD nth_mem[of n "messages S"] in_set_updD list_map_range_setD list_map_get_range list_map_range_del in_set_map_filter_vals
+      intro: ic_can_status_inv_mono1)
+
+
+
+(* System transition: IC Management Canister: Depositing cycles [DONE] *)
+
+definition ic_depositing_cycles_pre :: "nat \<Rightarrow> ('p, 'uid, 'canid, 'b, 'w, 'sm, 'c, 's, 'cid, 'pk) ic \<Rightarrow> bool" where
+  "ic_depositing_cycles_pre n S = (n < length (messages S) \<and> (case messages S ! n of Call_message orig cer cee mn a trans_cycles q \<Rightarrow>
+    (q = Unordered \<or> (\<forall>j < n. message_queue (messages S ! j) \<noteq> Some q)) \<and>
+    cee = ic_principal \<and>
+    mn = encode_string ''deposit_cycles'' \<and>
+    (case candid_parse_cid a of Some cid \<Rightarrow>
+    (case list_map_get (balances S) cid of Some bal \<Rightarrow>
+      True
+    | _ \<Rightarrow> False) | _ \<Rightarrow> False)
+  | _ \<Rightarrow> False))"
+
+definition ic_depositing_cycles_post :: "nat \<Rightarrow> ('p, 'uid, 'canid, 'b, 'w, 'sm, 'c, 's, 'cid, 'pk) ic \<Rightarrow> ('p, 'uid, 'canid, 'b, 'w, 'sm, 'c, 's, 'cid, 'pk) ic" where
+  "ic_depositing_cycles_post n S = (case messages S ! n of Call_message orig cer cee mn a trans_cycles q \<Rightarrow>
+    let cid = the (candid_parse_cid a) in
+    (case list_map_get (balances S) cid of Some bal \<Rightarrow>
+    S\<lparr>balances := list_map_set (balances S) cid (bal + trans_cycles),
+      messages := take n (messages S) @ drop (Suc n) (messages S) @ [Response_message orig (Reply (blob_of_candid Candid_empty)) 0]\<rparr>))"
+
+lemma ic_depositing_cycles_cycles_monotonic:
+  assumes "ic_depositing_cycles_pre n S"
+  shows "total_cycles S = total_cycles (ic_depositing_cycles_post n S)"
+proof -
+  obtain orig cer cee mn a trans_cycles q cid where msg: "messages S ! n = Call_message orig cer cee mn a trans_cycles q"
+    and cid_def: "candid_parse_cid a = Some cid"
+    using assms
+    by (auto simp: ic_depositing_cycles_pre_def split: message.splits option.splits)
+  define older where "older = take n (messages S)"
+  define younger where "younger = drop (Suc n) (messages S)"
+  have msgs: "messages S = older @ Call_message orig cer cee mn a trans_cycles q # younger" "(older @ w # younger) ! n = w"
+    "take n older = older" "take (n - length older) ws = []" "drop (Suc n) older = []"
+    "drop (Suc n - length older) (w # ws) = ws" for w ws
+    using id_take_nth_drop[of n "messages S"] assms
+    by (auto simp: ic_depositing_cycles_pre_def msg younger_def older_def nth_append)
+  show ?thesis
+    using assms list_map_sum_in_ge[where ?g=id and ?f="balances S" and ?x=cid]
+    by (auto simp: ic_depositing_cycles_pre_def ic_depositing_cycles_post_def total_cycles_def call_ctxt_carried_cycles cid_def Let_def msgs
+        list_map_sum_in[where ?g=id and ?f="balances S"] min_def split: message.splits option.splits sum.splits)
+qed
+
+lemma ic_depositing_cycles_ic_inv:
+  assumes "ic_depositing_cycles_pre n S" "ic_inv S"
+  shows "ic_inv (ic_depositing_cycles_post n S)"
+  using assms
+  by (auto simp: ic_inv_def ic_depositing_cycles_pre_def ic_depositing_cycles_post_def Let_def
+      split: sum.splits message.splits call_origin.splits option.splits if_splits can_status.splits
+      dest!: in_set_takeD in_set_dropD nth_mem[of n "messages S"] in_set_updD list_map_range_setD list_map_get_range list_map_range_del
+      in_set_map_filter_vals)
+
+
+
+(* System transition: IC Management Canister: Random numbers [DONE] *)
+
+definition ic_random_numbers_pre :: "nat \<Rightarrow> 'b \<Rightarrow> ('p, 'uid, 'canid, 'b, 'w, 'sm, 'c, 's, 'cid, 'pk) ic \<Rightarrow> bool" where
+  "ic_random_numbers_pre n b S = (n < length (messages S) \<and> (case messages S ! n of Call_message orig cer cee mn a trans_cycles q \<Rightarrow>
+    (q = Unordered \<or> (\<forall>j < n. message_queue (messages S ! j) \<noteq> Some q)) \<and>
+    cee = ic_principal \<and>
+    mn = encode_string ''raw_rand'' \<and>
+    a = blob_of_candid Candid_empty \<and>
+    blob_length b = 32
+  | _ \<Rightarrow> False))"
+
+definition ic_random_numbers_post :: "nat \<Rightarrow> 'b \<Rightarrow> ('p, 'uid, 'canid, 'b, 'w, 'sm, 'c, 's, 'cid, 'pk) ic \<Rightarrow> ('p, 'uid, 'canid, 'b, 'w, 'sm, 'c, 's, 'cid, 'pk) ic" where
+  "ic_random_numbers_post n b S = (case messages S ! n of Call_message orig cer cee mn a trans_cycles q \<Rightarrow>
+    S\<lparr>messages := take n (messages S) @ drop (Suc n) (messages S) @ [Response_message orig (Reply (blob_of_candid (Candid_blob b))) trans_cycles]\<rparr>)"
+
+lemma ic_random_numbers_cycles_inv:
+  assumes "ic_random_numbers_pre n b S"
+  shows "total_cycles S = total_cycles (ic_random_numbers_post n b S)"
+proof -
+  obtain orig cer cee mn a trans_cycles q where msg: "messages S ! n = Call_message orig cer cee mn a trans_cycles q"
+    using assms
+    by (auto simp: ic_random_numbers_pre_def split: message.splits)
+  define older where "older = take n (messages S)"
+  define younger where "younger = drop (Suc n) (messages S)"
+  have msgs: "messages S = older @ Call_message orig cer cee mn a trans_cycles q # younger" "(older @ w # younger) ! n = w"
+    "take n older = older" "take (n - length older) ws = []" "drop (Suc n) older = []"
+    "drop (Suc n - length older) (w # ws) = ws" for w ws
+    using id_take_nth_drop[of n "messages S"] assms
+    by (auto simp: ic_random_numbers_pre_def msg younger_def older_def nth_append)
+  show ?thesis
+    using assms
+    by (auto simp: ic_random_numbers_pre_def ic_random_numbers_post_def total_cycles_def call_ctxt_carried_cycles Let_def msgs)
+qed
+
+lemma ic_random_numbers_ic_inv:
+  assumes "ic_random_numbers_pre n b S" "ic_inv S"
+  shows "ic_inv (ic_random_numbers_post n b S)"
+  using assms
+  by (auto simp: ic_inv_def ic_random_numbers_pre_def ic_random_numbers_post_def Let_def
+      split: sum.splits message.splits call_origin.splits option.splits if_splits can_status.splits
+      dest!: in_set_takeD in_set_dropD nth_mem[of n "messages S"] in_set_updD list_map_range_setD list_map_get_range list_map_range_del
+      in_set_map_filter_vals)
+
+
+
+(* System transition: IC Management Canister: Canister creation with cycles [DONE] *)
+
+definition ic_provisional_canister_creation_pre :: "nat \<Rightarrow> 'canid \<Rightarrow> nat \<Rightarrow> ('p, 'uid, 'canid, 'b, 'w, 'sm, 'c, 's, 'cid, 'pk) ic \<Rightarrow> bool" where
+  "ic_provisional_canister_creation_pre n cid t S = (n < length (messages S) \<and> (case messages S ! n of Call_message orig cer cee mn a trans_cycles q \<Rightarrow>
+    (case candid_parse_nat a [encode_string ''amount''] of Some cyc \<Rightarrow>
+      (q = Unordered \<or> (\<forall>j < n. message_queue (messages S ! j) \<noteq> Some q)) \<and>
+      cee = ic_principal \<and>
+      mn = encode_string ''provisional_create_canister_with_cycles'' \<and>
+      is_system_assigned (principal_of_canid cid) \<and>
+      cid \<notin> list_map_dom (canisters S) \<and>
+      cid \<notin> list_map_dom (time S) \<and>
+      cid \<notin> list_map_dom (controllers S) \<and>
+      cid \<notin> list_map_dom (balances S) \<and>
+      cid \<notin> list_map_dom (certified_data S) \<and>
+      cid \<notin> list_map_dom (canister_status S)
+    | _ \<Rightarrow> False) | _ \<Rightarrow> False))"
+
+definition ic_provisional_canister_creation_post :: "nat \<Rightarrow> 'canid \<Rightarrow> nat \<Rightarrow> ('p, 'uid, 'canid, 'b, 'w, 'sm, 'c, 's, 'cid, 'pk) ic \<Rightarrow> ('p, 'uid, 'canid, 'b, 'w, 'sm, 'c, 's, 'cid, 'pk) ic" where
+  "ic_provisional_canister_creation_post n cid t S = (case messages S ! n of Call_message orig cer cee mn a trans_cycles q \<Rightarrow>
+    let cyc = the (candid_parse_nat a [encode_string ''amount'']) in
+    S\<lparr>canisters := list_map_set (canisters S) cid None,
+      time := list_map_set (time S) cid t,
+      controllers := list_map_set (controllers S) cid {cer},
+      freezing_threshold := list_map_set (freezing_threshold S) cid 2592000,
+      balances := list_map_set (balances S) cid cyc,
+      certified_data := list_map_set (certified_data S) cid empty_blob,
+      messages := take n (messages S) @ drop (Suc n) (messages S) @ [Response_message orig (Reply (blob_of_candid
+        (Candid_record (list_map_init [(encode_string ''canister_id'', Candid_blob (blob_of_canid cid))])))) trans_cycles],
+      canister_status := list_map_set (canister_status S) cid Running\<rparr>)"
+
+definition ic_provisional_canister_creation_minted_cycles :: "nat \<Rightarrow> 'canid \<Rightarrow> nat \<Rightarrow> ('p, 'uid, 'canid, 'b, 'w, 'sm, 'c, 's, 'cid, 'pk) ic \<Rightarrow> nat" where
+  "ic_provisional_canister_creation_minted_cycles n cid t S = (case messages S ! n of Call_message orig cer cee mn a trans_cycles q \<Rightarrow>
+    the (candid_parse_nat a [encode_string ''amount'']))"
+
+lemma ic_provisional_canister_creation_cycles_antimonotonic:
+  assumes "ic_provisional_canister_creation_pre n cid t S"
+  shows "total_cycles S + ic_provisional_canister_creation_minted_cycles n cid t S  = total_cycles (ic_provisional_canister_creation_post n cid t S)"
+proof -
+  obtain orig cer cee mn a trans_cycles q where msg: "messages S ! n = Call_message orig cer cee mn a trans_cycles q"
+    using assms
+    by (auto simp: ic_provisional_canister_creation_pre_def split: message.splits)
+  define older where "older = take n (messages S)"
+  define younger where "younger = drop (Suc n) (messages S)"
+  have msgs: "messages S = older @ Call_message orig cer cee mn a trans_cycles q # younger" "(older @ w # younger) ! n = w"
+    "take n older = older" "take (n - length older) ws = []" "drop (Suc n) older = []"
+    "drop (Suc n - length older) (w # ws) = ws" for w ws
+    using id_take_nth_drop[of n "messages S"] assms
+    by (auto simp: ic_provisional_canister_creation_pre_def msg younger_def older_def nth_append)
+  show ?thesis
+    using assms
+    by (auto simp: ic_provisional_canister_creation_pre_def ic_provisional_canister_creation_post_def ic_provisional_canister_creation_minted_cycles_def total_cycles_def Let_def msgs
+        list_map_sum_out[where ?g=id] list_map_sum_out[where ?g=status_cycles] split: message.splits option.splits)
+qed
+
+lemma ic_provisional_canister_creation_ic_inv:
+  assumes "ic_provisional_canister_creation_pre n cid t S" "ic_inv S"
+  shows "ic_inv (ic_provisional_canister_creation_post n cid t S)"
+  using assms
+  by (auto simp: ic_inv_def ic_provisional_canister_creation_pre_def ic_provisional_canister_creation_post_def Let_def
+      split: sum.splits message.splits call_origin.splits option.splits if_splits can_status.splits
+      dest!: in_set_takeD in_set_dropD nth_mem[of n "messages S"] in_set_updD list_map_range_setD list_map_get_range list_map_range_del in_set_map_filter_vals
+      intro: ic_can_status_inv_mono1)
+
+
+
+(* System transition: IC Management Canister: Top up canister [DONE] *)
+
+definition ic_top_up_canister_pre :: "nat \<Rightarrow> ('p, 'uid, 'canid, 'b, 'w, 'sm, 'c, 's, 'cid, 'pk) ic \<Rightarrow> bool" where
+  "ic_top_up_canister_pre n S = (n < length (messages S) \<and> (case messages S ! n of Call_message orig cer cee mn a trans_cycles q \<Rightarrow>
+    (case (candid_parse_cid a, candid_parse_nat a [encode_string ''amount'']) of (Some cid, Some cyc) \<Rightarrow>
+      (q = Unordered \<or> (\<forall>j < n. message_queue (messages S ! j) \<noteq> Some q)) \<and>
+      cee = ic_principal \<and>
+      mn = encode_string ''provisional_top_up_canister'' \<and>
+      cid \<in> list_map_dom (balances S)
+    | _ \<Rightarrow> False) | _ \<Rightarrow> False))"
+
+definition ic_top_up_canister_post :: "nat \<Rightarrow> ('p, 'uid, 'canid, 'b, 'w, 'sm, 'c, 's, 'cid, 'pk) ic \<Rightarrow> ('p, 'uid, 'canid, 'b, 'w, 'sm, 'c, 's, 'cid, 'pk) ic" where
+  "ic_top_up_canister_post n S = (case messages S ! n of Call_message orig cer cee mn a trans_cycles q \<Rightarrow>
+    let cid = the (candid_parse_cid a);
+    cyc = the (candid_parse_nat a [encode_string ''amount'']);
+    bal = the (list_map_get (balances S) cid) in
+    S\<lparr>balances := list_map_set (balances S) cid (bal + cyc)\<rparr>)"
+
+definition ic_top_up_canister_minted_cycles :: "nat \<Rightarrow> ('p, 'uid, 'canid, 'b, 'w, 'sm, 'c, 's, 'cid, 'pk) ic \<Rightarrow> nat" where
+  "ic_top_up_canister_minted_cycles n S = (case messages S ! n of Call_message orig cer cee mn a trans_cycles q \<Rightarrow>
+    the (candid_parse_nat a [encode_string ''amount'']))"
+
+lemma ic_top_up_canister_cycles_antimonotonic:
+  assumes "ic_top_up_canister_pre n S"
+  shows "total_cycles S + ic_top_up_canister_minted_cycles n S  = total_cycles (ic_top_up_canister_post n S)"
+proof -
+  obtain orig cer cee mn a trans_cycles q where msg: "messages S ! n = Call_message orig cer cee mn a trans_cycles q"
+    using assms
+    by (auto simp: ic_top_up_canister_pre_def split: message.splits)
+  define older where "older = take n (messages S)"
+  define younger where "younger = drop (Suc n) (messages S)"
+  have msgs: "messages S = older @ Call_message orig cer cee mn a trans_cycles q # younger" "(older @ w # younger) ! n = w"
+    "take n older = older" "take (n - length older) ws = []" "drop (Suc n) older = []"
+    "drop (Suc n - length older) (w # ws) = ws" for w ws
+    using id_take_nth_drop[of n "messages S"] assms
+    by (auto simp: ic_top_up_canister_pre_def msg younger_def older_def nth_append)
+  define cid where "cid = the (candid_parse_cid a)"
+  show ?thesis
+    using assms
+    by (cases "list_map_get (balances S) cid")
+       (auto simp: ic_top_up_canister_pre_def ic_top_up_canister_post_def ic_top_up_canister_minted_cycles_def total_cycles_def Let_def msgs cid_def
+        list_map_sum_in[where ?g=id] split: message.splits option.splits)
+qed
+
+lemma ic_top_up_canister_ic_inv:
+  assumes "ic_top_up_canister_pre n S" "ic_inv S"
+  shows "ic_inv (ic_top_up_canister_post n S)"
+  using assms
+  by (auto simp: ic_inv_def ic_top_up_canister_pre_def ic_top_up_canister_post_def Let_def
+      split: sum.splits message.splits call_origin.splits option.splits if_splits can_status.splits
+      dest!: in_set_takeD in_set_dropD nth_mem[of n "messages S"] in_set_updD list_map_range_setD list_map_get_range list_map_range_del
+      in_set_map_filter_vals)
+
+
+
+(* System transition: Callback invocation (not deleted) [DONE] *)
+
+definition callback_invocation_not_deleted_pre :: "nat \<Rightarrow> ('p, 'uid, 'canid, 'b, 'w, 'sm, 'c, 's, 'cid, 'pk) ic \<Rightarrow> bool" where
+  "callback_invocation_not_deleted_pre n S = (n < length (messages S) \<and> (case messages S ! n of Response_message (From_canister ctxt_id c) resp ref_cycles \<Rightarrow>
+    (case list_map_get (call_contexts S) ctxt_id of Some ctxt \<Rightarrow>
+      let cid = call_ctxt_canister ctxt in
+      \<not>call_ctxt_deleted ctxt \<and>
+      (case list_map_get (balances S) cid of Some bal \<Rightarrow> True
+      | _ \<Rightarrow> False)
+    | _ \<Rightarrow> False)
+  | _ \<Rightarrow> False))"
+
+definition callback_invocation_not_deleted_post :: "nat \<Rightarrow> ('p, 'uid, 'canid, 'b, 'w, 'sm, 'c, 's, 'cid, 'pk) ic \<Rightarrow> ('p, 'uid, 'canid, 'b, 'w, 'sm, 'c, 's, 'cid, 'pk) ic" where
+  "callback_invocation_not_deleted_post n S = (case messages S ! n of Response_message (From_canister ctxt_id c) resp ref_cycles \<Rightarrow>
+    (case list_map_get (call_contexts S) ctxt_id of Some ctxt \<Rightarrow>
+      let cid = call_ctxt_canister ctxt in
+      (case list_map_get (balances S) cid of Some bal \<Rightarrow>
+        S\<lparr>balances := list_map_set (balances S) cid (bal + ref_cycles),
+          messages := list_update (messages S) n (Func_message ctxt_id cid (Callback c resp ref_cycles) Unordered)\<rparr>)))"
+
+lemma callback_invocation_not_deleted_cycles_inv:
+  assumes "callback_invocation_not_deleted_pre n S"
+  shows "total_cycles S = total_cycles (callback_invocation_not_deleted_post n S)"
+proof -
+  obtain ctxt_id c resp ref_cycles where msg: "messages S ! n = Response_message (From_canister ctxt_id c) resp ref_cycles"
+    using assms
+    by (auto simp: callback_invocation_not_deleted_pre_def split: message.splits option.splits call_origin.splits)
+  define older where "older = take n (messages S)"
+  define younger where "younger = drop (Suc n) (messages S)"
+  have msgs: "messages S = older @ Response_message (From_canister ctxt_id c) resp ref_cycles # younger" "(older @ w # younger) ! n = w"
+    and msgs_upd: "(older @ Response_message (From_canister ctxt_id c) resp ref_cycles # younger)[n := m] = older @ m # younger" for w m
+    using assms id_take_nth_drop[of n "messages S"] upd_conv_take_nth_drop[of n "messages S"] assms
+    by (auto simp: callback_invocation_not_deleted_pre_def msg older_def younger_def nth_append)
+  show ?thesis
+    using assms
+    by (auto simp: callback_invocation_not_deleted_pre_def callback_invocation_not_deleted_post_def total_cycles_def call_ctxt_carried_cycles Let_def msgs msgs_upd
+        list_map_sum_in[where ?g=id and ?f="balances S"] split: option.splits)
+qed
+
+lemma callback_invocation_not_deleted_ic_inv:
+  assumes "callback_invocation_not_deleted_pre n S" "ic_inv S"
+  shows "ic_inv (callback_invocation_not_deleted_post n S)"
+  using assms
+  by (auto simp: ic_inv_def callback_invocation_not_deleted_pre_def callback_invocation_not_deleted_post_def Let_def
+      split: sum.splits message.splits call_origin.splits option.splits if_splits can_status.splits
+      dest!: in_set_takeD in_set_dropD nth_mem[of n "messages S"] in_set_updD)
+
+
+
+(* System transition: Callback invocation (deleted) [DONE] *)
+
+definition callback_invocation_deleted_pre :: "nat \<Rightarrow> ('p, 'uid, 'canid, 'b, 'w, 'sm, 'c, 's, 'cid, 'pk) ic \<Rightarrow> bool" where
+  "callback_invocation_deleted_pre n S = (n < length (messages S) \<and> (case messages S ! n of Response_message (From_canister ctxt_id c) resp ref_cycles \<Rightarrow>
+    (case list_map_get (call_contexts S) ctxt_id of Some ctxt \<Rightarrow>
+      let cid = call_ctxt_canister ctxt in
+      call_ctxt_deleted ctxt \<and>
+      (case list_map_get (balances S) cid of Some bal \<Rightarrow> True
+      | _ \<Rightarrow> False)
+    | _ \<Rightarrow> False)
+  | _ \<Rightarrow> False))"
+
+definition callback_invocation_deleted_post :: "nat \<Rightarrow> ('p, 'uid, 'canid, 'b, 'w, 'sm, 'c, 's, 'cid, 'pk) ic \<Rightarrow> ('p, 'uid, 'canid, 'b, 'w, 'sm, 'c, 's, 'cid, 'pk) ic" where
+  "callback_invocation_deleted_post n S = (case messages S ! n of Response_message (From_canister ctxt_id c) resp ref_cycles \<Rightarrow>
+    (case list_map_get (call_contexts S) ctxt_id of Some ctxt \<Rightarrow>
+      let cid = call_ctxt_canister ctxt in
+      (case list_map_get (balances S) cid of Some bal \<Rightarrow>
+        S\<lparr>balances := list_map_set (balances S) cid (bal + ref_cycles + MAX_CYCLES_PER_RESPONSE),
+          messages := take n (messages S) @ drop (Suc n) (messages S)\<rparr>)))"
+
+lemma callback_invocation_deleted_cycles_inv:
+  assumes "callback_invocation_deleted_pre n S"
+  shows "total_cycles S = total_cycles (callback_invocation_deleted_post n S)"
+proof -
+  obtain ctxt_id c resp ref_cycles where msg: "messages S ! n = Response_message (From_canister ctxt_id c) resp ref_cycles"
+    using assms
+    by (auto simp: callback_invocation_deleted_pre_def split: message.splits option.splits call_origin.splits)
+  define older where "older = take n (messages S)"
+  define younger where "younger = drop (Suc n) (messages S)"
+  have msgs: "messages S = older @ Response_message (From_canister ctxt_id c) resp ref_cycles # younger" "(older @ w # younger) ! n = w"
+    "take n older = older" "take (n - length older) ws = []" "drop (Suc n) older = []"
+    "drop (Suc n - length older) (w # ws) = ws" for w ws
+    using id_take_nth_drop[of n "messages S"] assms
+    by (auto simp: callback_invocation_deleted_pre_def msg younger_def older_def nth_append)
+  show ?thesis
+    using assms
+    by (auto simp: callback_invocation_deleted_pre_def callback_invocation_deleted_post_def total_cycles_def call_ctxt_carried_cycles Let_def msgs
+        list_map_sum_in[where ?g=id and ?f="balances S"] split: option.splits)
+qed
+
+lemma callback_invocation_deleted_ic_inv:
+  assumes "callback_invocation_deleted_pre n S" "ic_inv S"
+  shows "ic_inv (callback_invocation_deleted_post n S)"
+  using assms
+  by (auto simp: ic_inv_def callback_invocation_deleted_pre_def callback_invocation_deleted_post_def Let_def
+      split: sum.splits message.splits call_origin.splits option.splits if_splits can_status.splits
+      dest!: in_set_takeD in_set_dropD nth_mem[of n "messages S"] in_set_updD)
+
+
+
+(* System transition: Respond to user request [DONE] *)
+
+definition respond_to_user_request_pre :: "nat \<Rightarrow> ('p, 'uid, 'canid, 'b, 'w, 'sm, 'c, 's, 'cid, 'pk) ic \<Rightarrow> bool" where
+  "respond_to_user_request_pre n S = (n < length (messages S) \<and> (case messages S ! n of Response_message (From_user req) resp ref_cycles \<Rightarrow>
+    (case list_map_get (requests S) req of Some Processing \<Rightarrow> True
+    | _ \<Rightarrow> False)
+  | _ \<Rightarrow> False))"
+
+definition respond_to_user_request_post :: "nat \<Rightarrow> ('p, 'uid, 'canid, 'b, 'w, 'sm, 'c, 's, 'cid, 'pk) ic \<Rightarrow> ('p, 'uid, 'canid, 'b, 'w, 'sm, 'c, 's, 'cid, 'pk) ic" where
+  "respond_to_user_request_post n S = (case messages S ! n of Response_message (From_user req) resp ref_cycles \<Rightarrow>
+    let req_resp = (case resp of Reply b \<Rightarrow> Replied b | response.Reject c b \<Rightarrow> Rejected c b) in
+    S\<lparr>messages := take n (messages S) @ drop (Suc n) (messages S),
+      requests := list_map_set (requests S) req req_resp\<rparr>)"
+
+definition respond_to_user_request_burned_cycles :: "nat \<Rightarrow> ('p, 'uid, 'canid, 'b, 'w, 'sm, 'c, 's, 'cid, 'pk) ic \<Rightarrow> nat" where
+  "respond_to_user_request_burned_cycles n S = (case messages S ! n of Response_message (From_user req) resp ref_cycles \<Rightarrow>
+    ref_cycles)"
+
+lemma respond_to_user_request_cycles_monotonic:
+  assumes "respond_to_user_request_pre n S"
+  shows "total_cycles S = total_cycles (respond_to_user_request_post n S) + respond_to_user_request_burned_cycles n S"
+proof -
+  obtain req resp ref_cycles where msg: "messages S ! n = Response_message (From_user req) resp ref_cycles"
+    using assms
+    by (auto simp: respond_to_user_request_pre_def split: message.splits option.splits call_origin.splits)
+  define older where "older = take n (messages S)"
+  define younger where "younger = drop (Suc n) (messages S)"
+  have msgs: "messages S = older @ Response_message (From_user req) resp ref_cycles # younger" "(older @ w # younger) ! n = w"
+    "take n older = older" "take (n - length older) ws = []" "drop (Suc n) older = []"
+    "drop (Suc n - length older) (w # ws) = ws" for w ws
+    using id_take_nth_drop[of n "messages S"] assms
+    by (auto simp: respond_to_user_request_pre_def msg younger_def older_def nth_append)
+  show ?thesis
+    using assms
+    by (auto simp: respond_to_user_request_pre_def respond_to_user_request_post_def respond_to_user_request_burned_cycles_def total_cycles_def call_ctxt_carried_cycles Let_def msgs
+        list_map_sum_in[where ?g=id and ?f="balances S"] split: option.splits request_status.splits)
+qed
+
+lemma respond_to_user_request_ic_inv:
+  assumes "respond_to_user_request_pre n S" "ic_inv S"
+  shows "ic_inv (respond_to_user_request_post n S)"
+  using assms
+  by (auto simp: ic_inv_def respond_to_user_request_pre_def respond_to_user_request_post_def Let_def
+      split: sum.splits message.splits call_origin.splits option.splits if_splits can_status.splits
+      dest!: in_set_takeD in_set_dropD nth_mem[of n "messages S"] in_set_updD)
+
+
+
+(* System transition: Request clean up [DONE] *)
+
+definition request_cleanup_pre :: "('b, 'p, 'uid, 'canid, 's) request \<Rightarrow> ('p, 'uid, 'canid, 'b, 'w, 'sm, 'c, 's, 'cid, 'pk) ic \<Rightarrow> bool" where
+  "request_cleanup_pre req S = (case list_map_get (requests S) req of Some req_status \<Rightarrow>
+    (case req_status of Replied _ \<Rightarrow> True | Rejected _ _ \<Rightarrow> True | _ \<Rightarrow> False)
+    | _ \<Rightarrow> False)"
+
+definition request_cleanup_post :: "('b, 'p, 'uid, 'canid, 's) request \<Rightarrow> ('p, 'uid, 'canid, 'b, 'w, 'sm, 'c, 's, 'cid, 'pk) ic \<Rightarrow> ('p, 'uid, 'canid, 'b, 'w, 'sm, 'c, 's, 'cid, 'pk) ic" where
+  "request_cleanup_post req S = (S\<lparr>requests := list_map_set (requests S) req Done\<rparr>)"
+
+lemma request_cleanup_cycles_inv:
+  assumes "request_cleanup_pre n S"
+  shows "total_cycles S = total_cycles (request_cleanup_post n S)"
+  by (auto simp: request_cleanup_post_def total_cycles_def)
+
+lemma request_cleanup_ic_inv:
+  assumes "request_cleanup_pre req S" "ic_inv S"
+  shows "ic_inv (request_cleanup_post req S)"
+  using assms
+  by (auto simp: ic_inv_def request_cleanup_pre_def request_cleanup_post_def Let_def
+      split: sum.splits message.splits call_origin.splits option.splits if_splits can_status.splits
+      dest!: in_set_takeD in_set_dropD in_set_updD)
+
+
+
+(* System transition: Request clean up (expired) [DONE] *)
+
+definition request_cleanup_expired_pre :: "('b, 'p, 'uid, 'canid, 's) request \<Rightarrow> ('p, 'uid, 'canid, 'b, 'w, 'sm, 'c, 's, 'cid, 'pk) ic \<Rightarrow> bool" where
+  "request_cleanup_expired_pre req S = (case list_map_get (requests S) req of Some req_status \<Rightarrow>
+    (case req_status of Replied _ \<Rightarrow> True | Rejected _ _ \<Rightarrow> True | Done \<Rightarrow> True | _ \<Rightarrow> False) \<and>
+    request.ingress_expiry req < system_time S
+    | _ \<Rightarrow> False)"
+
+definition request_cleanup_expired_post :: "('b, 'p, 'uid, 'canid, 's) request \<Rightarrow> ('p, 'uid, 'canid, 'b, 'w, 'sm, 'c, 's, 'cid, 'pk) ic \<Rightarrow> ('p, 'uid, 'canid, 'b, 'w, 'sm, 'c, 's, 'cid, 'pk) ic" where
+  "request_cleanup_expired_post req S = (S\<lparr>requests := list_map_del (requests S) req\<rparr>)"
+
+lemma request_cleanup_expired_cycles_inv:
+  assumes "request_cleanup_expired_pre n S"
+  shows "total_cycles S = total_cycles (request_cleanup_expired_post n S)"
+  by (auto simp: request_cleanup_expired_post_def total_cycles_def)
+
+lemma request_cleanup_expired_ic_inv:
+  assumes "request_cleanup_expired_pre req S" "ic_inv S"
+  shows "ic_inv (request_cleanup_expired_post req S)"
+  using assms
+  by (auto simp: ic_inv_def request_cleanup_expired_pre_def request_cleanup_expired_post_def Let_def
+      split: sum.splits message.splits call_origin.splits option.splits if_splits can_status.splits
+      dest!: in_set_takeD in_set_dropD in_set_updD)
+
+
+
+(* System transition: Canister out of cycles [DONE] *)
+
+definition canister_out_of_cycles_pre :: "'canid \<Rightarrow> ('p, 'uid, 'canid, 'b, 'w, 'sm, 'c, 's, 'cid, 'pk) ic \<Rightarrow> bool" where
+  "canister_out_of_cycles_pre cid S = (case list_map_get (balances S) cid of Some 0 \<Rightarrow> True
+  | _ \<Rightarrow> False)"
+
+definition canister_out_of_cycles_post :: "'canid \<Rightarrow> ('p, 'uid, 'canid, 'b, 'w, 'sm, 'c, 's, 'cid, 'pk) ic \<Rightarrow> ('p, 'uid, 'canid, 'b, 'w, 'sm, 'c, 's, 'cid, 'pk) ic" where
+  "canister_out_of_cycles_post cid S = (
+    let call_ctxt_to_msg = (\<lambda>ctxt.
+      if call_ctxt_canister ctxt = cid \<and> call_ctxt_needs_to_respond ctxt then
+        Some (Response_message (call_ctxt_origin ctxt) (response.Reject CANISTER_REJECT (encode_string ''Canister has been uninstalled'')) (call_ctxt_available_cycles ctxt))
+      else None);
+    call_ctxt_to_ctxt = (\<lambda>ctxt. if call_ctxt_canister ctxt = cid then call_ctxt_delete ctxt else ctxt) in
+    S\<lparr>canisters := list_map_set (canisters S) cid None, certified_data := list_map_set (certified_data S) cid empty_blob,
+      messages := messages S @ List.map_filter call_ctxt_to_msg (list_map_vals (call_contexts S)),
+      call_contexts := list_map_map call_ctxt_to_ctxt (call_contexts S)\<rparr>)"
+
+lemma canister_out_of_cycles_cycles_inv:
+  assumes "canister_out_of_cycles_pre cid S"
+  shows "total_cycles S = total_cycles (canister_out_of_cycles_post cid S)"
+proof -
+  have F1: "list_map_sum_vals call_ctxt_carried_cycles (call_contexts S) =
+    list_map_sum_vals id
+      (list_map_map (\<lambda>ctxt. if call_ctxt_canister ctxt = cid then call_ctxt_carried_cycles ctxt else 0) (call_contexts S)) +
+    list_map_sum_vals call_ctxt_carried_cycles
+      (list_map_map (\<lambda>ctxt. if call_ctxt_canister ctxt = cid then call_ctxt_delete ctxt else ctxt) (call_contexts S))"
+    using list_map_sum_vals_split[where ?f="call_ctxt_carried_cycles" and ?g="call_ctxt_delete", unfolded call_ctxt_delete_carried_cycles diff_zero]
+    by auto
+  show ?thesis
+    using assms
+    by (auto simp: canister_out_of_cycles_pre_def canister_out_of_cycles_post_def total_cycles_def call_ctxt_carried_cycles Let_def F1
+        split: message.splits option.splits sum.splits if_splits intro!: list_map_sum_vals_filter)
+qed
+
+lemma canister_out_of_cycles_ic_inv:
+  assumes "canister_out_of_cycles_pre cid S" "ic_inv S"
+  shows "ic_inv (canister_out_of_cycles_post cid S)"
+  using assms
+  by (auto simp: ic_inv_def canister_out_of_cycles_pre_def canister_out_of_cycles_post_def Let_def
+      split: sum.splits message.splits call_origin.splits option.splits if_splits can_status.splits
+      dest!: in_set_takeD in_set_dropD in_set_updD list_map_range_setD list_map_get_range list_map_range_del
+      in_set_map_filter_vals)
+
+
+
+(* System transition: Time progressing and cycle consumption (canister time) [DONE] *)
+
+definition canister_time_progress_pre :: "'canid \<Rightarrow> nat \<Rightarrow> ('p, 'uid, 'canid, 'b, 'w, 'sm, 'c, 's, 'cid, 'pk) ic \<Rightarrow> bool" where
+  "canister_time_progress_pre cid t1 S = (case list_map_get (time S) cid of Some t0 \<Rightarrow>
+      t0 < t1
+    | _ \<Rightarrow> False)"
+
+definition canister_time_progress_post :: "'canid \<Rightarrow> nat \<Rightarrow> ('p, 'uid, 'canid, 'b, 'w, 'sm, 'c, 's, 'cid, 'pk) ic \<Rightarrow> ('p, 'uid, 'canid, 'b, 'w, 'sm, 'c, 's, 'cid, 'pk) ic" where
+  "canister_time_progress_post cid t1 S = (S\<lparr>time := list_map_set (time S) cid t1\<rparr>)"
+
+lemma canister_time_progress_cycles_inv:
+  assumes "canister_time_progress_pre cid t1 S"
+  shows "total_cycles S = total_cycles (canister_time_progress_post cid t1 S)"
+  by (auto simp: canister_time_progress_post_def total_cycles_def)
+
+lemma canister_time_progress_ic_inv:
+  assumes "canister_time_progress_pre cid t1 S" "ic_inv S"
+  shows "ic_inv (canister_time_progress_post cid t1 S)"
+  using assms
+  by (auto simp: ic_inv_def canister_time_progress_pre_def canister_time_progress_post_def Let_def
+      split: sum.splits message.splits call_origin.splits option.splits if_splits can_status.splits
+      dest!: in_set_takeD in_set_dropD in_set_updD list_map_range_setD list_map_get_range list_map_range_del
+      in_set_map_filter_vals)
+
+
+
+(* System transition: Time progressing and cycle consumption (cycle consumption) [DONE] *)
+
+definition cycle_consumption_pre :: "'canid \<Rightarrow> nat \<Rightarrow> ('p, 'uid, 'canid, 'b, 'w, 'sm, 'c, 's, 'cid, 'pk) ic \<Rightarrow> bool" where
+  "cycle_consumption_pre cid b1 S = (case list_map_get (balances S) cid of Some b0 \<Rightarrow>
+      0 \<le> b1 \<and> b1 < b0
+    | _ \<Rightarrow> False)"
+
+definition cycle_consumption_post :: "'canid \<Rightarrow> nat \<Rightarrow> ('p, 'uid, 'canid, 'b, 'w, 'sm, 'c, 's, 'cid, 'pk) ic \<Rightarrow> ('p, 'uid, 'canid, 'b, 'w, 'sm, 'c, 's, 'cid, 'pk) ic" where
+  "cycle_consumption_post cid b1 S = (S\<lparr>balances := list_map_set (balances S) cid b1\<rparr>)"
+
+definition cycle_consumption_burned_cycles :: "'canid \<Rightarrow> nat \<Rightarrow> ('p, 'uid, 'canid, 'b, 'w, 'sm, 'c, 's, 'cid, 'pk) ic \<Rightarrow> nat" where
+  "cycle_consumption_burned_cycles cid b1 S = the (list_map_get (balances S) cid) - b1"
+
+lemma cycle_consumption_cycles_monotonic:
+  assumes "cycle_consumption_pre cid b1 S"
+  shows "total_cycles S = total_cycles (cycle_consumption_post cid b1 S) + cycle_consumption_burned_cycles cid b1 S"
+  using assms list_map_sum_in_ge[where ?g=id and ?f="balances S" and ?x=cid]
+  by (auto simp: cycle_consumption_pre_def cycle_consumption_post_def cycle_consumption_burned_cycles_def total_cycles_def
+      list_map_sum_in[where ?g=id and ?f="balances S"] split: option.splits)
+
+lemma cycle_consumption_ic_inv:
+  assumes "cycle_consumption_pre cid b1 S" "ic_inv S"
+  shows "ic_inv (cycle_consumption_post cid b1 S)"
+  using assms
+  by (auto simp: ic_inv_def cycle_consumption_pre_def cycle_consumption_post_def Let_def
+      split: sum.splits message.splits call_origin.splits option.splits if_splits can_status.splits
+      dest!: in_set_takeD in_set_dropD in_set_updD list_map_range_setD list_map_get_range list_map_range_del
+      in_set_map_filter_vals)
+
+
+
+(* System transition: Time progressing and cycle consumption (system time) [DONE] *)
+
+definition system_time_progress_pre :: "nat \<Rightarrow> ('p, 'uid, 'canid, 'b, 'w, 'sm, 'c, 's, 'cid, 'pk) ic \<Rightarrow> bool" where
+  "system_time_progress_pre t1 S = (system_time S < t1)"
+
+definition system_time_progress_post :: "nat \<Rightarrow> ('p, 'uid, 'canid, 'b, 'w, 'sm, 'c, 's, 'cid, 'pk) ic \<Rightarrow> ('p, 'uid, 'canid, 'b, 'w, 'sm, 'c, 's, 'cid, 'pk) ic" where
+  "system_time_progress_post t1 S = (S\<lparr>system_time := t1\<rparr>)"
+
+lemma system_time_progress_cycles_inv:
+  assumes "system_time_progress_pre t1 S"
+  shows "total_cycles S = total_cycles (system_time_progress_post t1 S)"
+  by (auto simp: system_time_progress_post_def total_cycles_def)
+
+lemma system_time_progress_ic_inv:
+  assumes "system_time_progress_pre t1 S" "ic_inv S"
+  shows "ic_inv (system_time_progress_post t1 S)"
+  using assms
+  by (auto simp: ic_inv_def system_time_progress_pre_def system_time_progress_post_def Let_def
+      split: sum.splits message.splits call_origin.splits option.splits if_splits can_status.splits
+      dest!: in_set_takeD in_set_dropD in_set_updD list_map_range_setD list_map_get_range list_map_range_del
+      in_set_map_filter_vals)
+
+
+
+(* State machine *)
+
+inductive ic_steps :: "'sig itself \<Rightarrow> ('p, 'uid, 'canid, 'b, 'w, 'sm, 'c, 's, 'cid, 'pk) ic \<Rightarrow>
+  nat \<Rightarrow> nat \<Rightarrow> ('p, 'uid, 'canid, 'b, 'w, 'sm, 'c, 's, 'cid, 'pk) ic \<Rightarrow> bool" where
+  ic_steps_refl: "ic_steps sig S 0 0 S"
+| request_submission: "ic_steps sig S0 minted burned S \<Longrightarrow> request_submission_pre (E :: ('b, 'p, 'uid, 'canid, 's, 'pk, 'sig) envelope) S \<Longrightarrow> ic_steps sig S0 minted (burned + request_submission_burned_cycles E S) (request_submission_post E S)"
+| request_rejection: "ic_steps sig S0 minted burned S \<Longrightarrow> request_rejection_pre (E :: ('b, 'p, 'uid, 'canid, 's, 'pk, 'sig) envelope) req code msg S \<Longrightarrow> ic_steps sig S0 minted burned (request_rejection_post E req code msg S)"
+| initiate_canister_call: "ic_steps sig S0 minted burned S \<Longrightarrow> initiate_canister_call_pre req S \<Longrightarrow> ic_steps sig S0 minted burned (initiate_canister_call_post req S)"
+| call_reject: "ic_steps sig S0 minted burned S \<Longrightarrow> call_reject_pre n S \<Longrightarrow> ic_steps sig S0 minted burned (call_reject_post n S)"
+| call_context_create: "ic_steps sig S0 minted burned S \<Longrightarrow> call_context_create_pre n ctxt_id S \<Longrightarrow> ic_steps sig S0 minted burned (call_context_create_post n ctxt_id S)"
+| call_context_heartbeat: "ic_steps sig S0 minted burned S \<Longrightarrow> call_context_heartbeat_pre cee ctxt_id S \<Longrightarrow> ic_steps sig S0 minted burned (call_context_heartbeat_post cee ctxt_id S)"
+| message_execution: "ic_steps sig S0 minted burned S \<Longrightarrow> message_execution_pre n S \<Longrightarrow> ic_steps sig S0 minted (burned + message_execution_burned_cycles n S) (message_execution_post n S)"
+| call_context_starvation: "ic_steps sig S0 minted burned S \<Longrightarrow> call_context_starvation_pre ctxt_id S \<Longrightarrow> ic_steps sig S0 minted burned (call_context_starvation_post ctxt_id S)"
+| call_context_removal: "ic_steps sig S0 minted burned S \<Longrightarrow> call_context_removal_pre ctxt_id S \<Longrightarrow> ic_steps sig S0 minted (burned + call_context_removal_burned_cycles ctxt_id S) (call_context_removal_post ctxt_id S)"
+| ic_canister_creation: "ic_steps sig S0 minted burned S \<Longrightarrow> ic_canister_creation_pre n cid t S \<Longrightarrow> ic_steps sig S0 minted burned (ic_canister_creation_post n cid t S)"
+| ic_update_settings: "ic_steps sig S0 minted burned S \<Longrightarrow> ic_update_settings_pre n S \<Longrightarrow> ic_steps sig S0 minted burned (ic_update_settings_post n S)"
+| ic_canister_status: "ic_steps sig S0 minted burned S \<Longrightarrow> ic_canister_status_pre n m S \<Longrightarrow> ic_steps sig S0 minted burned (ic_canister_status_post n m S)"
+| ic_code_installation: "ic_steps sig S0 minted burned S \<Longrightarrow> ic_code_installation_pre n S \<Longrightarrow> ic_steps sig S0 minted (burned + ic_code_installation_burned_cycles n S) (ic_code_installation_post n S)"
+| ic_code_upgrade: "ic_steps sig S0 minted burned S \<Longrightarrow> ic_code_upgrade_pre n S \<Longrightarrow> ic_steps sig S0 minted (burned + ic_code_upgrade_burned_cycles n S) (ic_code_upgrade_post n S)"
+| ic_code_uninstallation: "ic_steps sig S0 minted burned S \<Longrightarrow> ic_code_uninstallation_pre n S \<Longrightarrow> ic_steps sig S0 minted burned (ic_code_uninstallation_post n S)"
+| ic_canister_stop_running: "ic_steps sig S0 minted burned S \<Longrightarrow> ic_canister_stop_running_pre n S \<Longrightarrow> ic_steps sig S0 minted burned (ic_canister_stop_running_post n S)"
+| ic_canister_stop_stopping: "ic_steps sig S0 minted burned S \<Longrightarrow> ic_canister_stop_stopping_pre n S \<Longrightarrow> ic_steps sig S0 minted burned (ic_canister_stop_stopping_post n S)"
+| ic_canister_stop_done_stopping: "ic_steps sig S0 minted burned S \<Longrightarrow> ic_canister_stop_done_stopping_pre cid S \<Longrightarrow> ic_steps sig S0 minted burned (ic_canister_stop_done_stopping_post cid S)"
+| ic_canister_stop_stopped: "ic_steps sig S0 minted burned S \<Longrightarrow> ic_canister_stop_stopped_pre n S \<Longrightarrow> ic_steps sig S0 minted burned (ic_canister_stop_stopped_post n S)"
+| ic_canister_start_not_stopping: "ic_steps sig S0 minted burned S \<Longrightarrow> ic_canister_start_not_stopping_pre n S \<Longrightarrow> ic_steps sig S0 minted burned (ic_canister_start_not_stopping_post n S)"
+| ic_canister_start_stopping: "ic_steps sig S0 minted burned S \<Longrightarrow> ic_canister_start_stopping_pre n S \<Longrightarrow> ic_steps sig S0 minted burned (ic_canister_start_stopping_post n S)"
+| ic_canister_deletion: "ic_steps sig S0 minted burned S \<Longrightarrow> ic_canister_deletion_pre n S \<Longrightarrow> ic_steps sig S0 minted (burned + ic_canister_deletion_burned_cycles n S) (ic_canister_deletion_post n S)"
+| ic_depositing_cycles: "ic_steps sig S0 minted burned S \<Longrightarrow> ic_depositing_cycles_pre n S \<Longrightarrow> ic_steps sig S0 minted burned (ic_depositing_cycles_post n S)"
+| ic_random_numbers: "ic_steps sig S0 minted burned S \<Longrightarrow> ic_random_numbers_pre n b S \<Longrightarrow> ic_steps sig S0 minted burned (ic_random_numbers_post n b S)"
+| ic_provisional_canister_creation: "ic_steps sig S0 minted burned S \<Longrightarrow> ic_provisional_canister_creation_pre n cid t S \<Longrightarrow> ic_steps sig S0 (minted + ic_provisional_canister_creation_minted_cycles n cid t S) burned (ic_provisional_canister_creation_post n cid t S)"
+| ic_top_up_canister: "ic_steps sig S0 minted burned S \<Longrightarrow> ic_top_up_canister_pre n S \<Longrightarrow> ic_steps sig S0 (minted + ic_top_up_canister_minted_cycles n S) burned (ic_top_up_canister_post n S)"
+| callback_invocation_not_deleted: "ic_steps sig S0 minted burned S \<Longrightarrow> callback_invocation_not_deleted_pre n S \<Longrightarrow> ic_steps sig S0 minted burned (callback_invocation_not_deleted_post n S)"
+| callback_invocation_deleted: "ic_steps sig S0 minted burned S \<Longrightarrow> callback_invocation_deleted_pre n S \<Longrightarrow> ic_steps sig S0 minted burned (callback_invocation_deleted_post n S)"
+| respond_to_user_request: "ic_steps sig S0 minted burned S \<Longrightarrow> respond_to_user_request_pre n S \<Longrightarrow> ic_steps sig S0 minted (burned + respond_to_user_request_burned_cycles n S) (respond_to_user_request_post n S)"
+| request_cleanup: "ic_steps sig S0 minted burned S \<Longrightarrow> request_cleanup_pre req S \<Longrightarrow> ic_steps sig S0 minted burned (request_cleanup_post req S)"
+| request_cleanup_expired: "ic_steps sig S0 minted burned S \<Longrightarrow> request_cleanup_expired_pre req S \<Longrightarrow> ic_steps sig S0 minted burned (request_cleanup_expired_post req S)"
+| canister_out_of_cycles: "ic_steps sig S0 minted burned S \<Longrightarrow> canister_out_of_cycles_pre cid S \<Longrightarrow> ic_steps sig S0 minted burned (canister_out_of_cycles_post cid S)"
+| canister_time_progress: "ic_steps sig S0 minted burned S \<Longrightarrow> canister_time_progress_pre cid t1 S \<Longrightarrow> ic_steps sig S0 minted burned (canister_time_progress_post cid t1 S)"
+| cycle_consumption: "ic_steps sig S0 minted burned S \<Longrightarrow> cycle_consumption_pre cid b1 S \<Longrightarrow> ic_steps sig S0 minted (burned + cycle_consumption_burned_cycles cid b1 S) (cycle_consumption_post cid b1 S)"
+| system_time_progress: "ic_steps sig S0 minted burned S \<Longrightarrow> system_time_progress_pre t1 S \<Longrightarrow> ic_steps sig S0 minted burned (system_time_progress_post t1 S)"
+
+lemma total_cycles:
+  assumes "ic_steps TYPE('sig) S0 minted burned S"
+  shows "total_cycles S0 + minted = total_cycles S + burned"
+  using assms
+  apply (induction "TYPE('sig)" S0 minted burned S rule: ic_steps.induct)
+                      apply auto[1]
+  using request_submission_cycles_inv apply fastforce
+  using request_rejection_cycles_inv apply fastforce
+  using initiate_canister_call_cycles_inv apply fastforce
+  using call_reject_cycles_inv apply fastforce
+  using call_context_create_cycles_inv apply fastforce
+  using call_context_heartbeat_cycles_inv apply fastforce
+  using message_execution_cycles_monotonic apply fastforce
+  using call_context_starvation_cycles_inv apply fastforce
+  using call_context_removal_cycles_monotonic apply fastforce
+  using ic_canister_creation_cycles_inv apply fastforce
+  using ic_update_settings_cycles_inv apply fastforce
+  using ic_canister_status_cycles_inv apply fastforce
+  using ic_code_installation_cycles_inv apply fastforce
+  using ic_code_upgrade_cycles_inv apply fastforce
+  using ic_code_uninstallation_cycles_inv apply fastforce
+  using ic_canister_stop_running_cycles_inv apply fastforce
+  using ic_canister_stop_stopping_cycles_inv apply fastforce
+  using ic_canister_stop_done_stopping_cycles_inv apply fastforce
+  using ic_canister_stop_stopped_cycles_inv apply fastforce
+  using ic_canister_start_not_stopping_cycles_inv apply fastforce
+  using ic_canister_start_stopping_cycles_inv apply fastforce
+  using ic_canister_deletion_cycles_monotonic apply fastforce
+  using ic_depositing_cycles_cycles_monotonic apply fastforce
+  using ic_random_numbers_cycles_inv apply fastforce
+  using ic_provisional_canister_creation_cycles_antimonotonic apply fastforce
+  using ic_top_up_canister_cycles_antimonotonic apply fastforce
+  using callback_invocation_not_deleted_cycles_inv apply fastforce
+  using callback_invocation_deleted_cycles_inv apply fastforce
+  using respond_to_user_request_cycles_monotonic apply fastforce
+  using request_cleanup_cycles_inv apply fastforce
+  using request_cleanup_expired_cycles_inv apply fastforce
+  using canister_out_of_cycles_cycles_inv apply fastforce
+  using canister_time_progress_cycles_inv apply fastforce
+  using cycle_consumption_cycles_monotonic apply fastforce
+  using system_time_progress_cycles_inv apply fastforce
+  done
+
+lemma ic_inv:
+  assumes "ic_steps TYPE('sig) S0 minted burned S"
+  shows "ic_inv S0 \<Longrightarrow> ic_inv S"
+  using assms
+  apply (induction "TYPE('sig)" S0 minted burned S rule: ic_steps.induct)
+                      apply auto[1]
+  using request_submission_ic_inv apply fastforce
+  using request_rejection_ic_inv apply fastforce
+  using initiate_canister_call_ic_inv apply fastforce
+  using call_reject_ic_inv apply fastforce
+  using call_context_create_ic_inv apply fastforce
+  using call_context_heartbeat_ic_inv apply fastforce
+  using message_execution_ic_inv apply fastforce
+  using call_context_starvation_ic_inv apply fastforce
+  using call_context_removal_ic_inv apply fastforce
+  using ic_canister_creation_ic_inv apply fastforce
+  using ic_update_settings_ic_inv apply fastforce
+  using ic_canister_status_ic_inv apply fastforce
+  using ic_code_installation_ic_inv apply fastforce
+  using ic_code_upgrade_ic_inv apply fastforce
+  using ic_code_uninstallation_ic_inv apply fastforce
+  using ic_canister_stop_running_ic_inv apply fastforce
+  using ic_canister_stop_stopping_ic_inv apply fastforce
+  using ic_canister_stop_done_stopping_ic_inv apply fastforce
+  using ic_canister_stop_stopped_ic_inv apply fastforce
+  using ic_canister_start_not_stopping_ic_inv apply fastforce
+  using ic_canister_start_stopping_ic_inv apply fastforce
+  using ic_canister_deletion_ic_inv apply fastforce
+  using ic_depositing_cycles_ic_inv apply fastforce
+  using ic_random_numbers_ic_inv apply fastforce
+  using ic_provisional_canister_creation_ic_inv apply fastforce
+  using ic_top_up_canister_ic_inv apply fastforce
+  using callback_invocation_not_deleted_ic_inv apply fastforce
+  using callback_invocation_deleted_ic_inv apply fastforce
+  using respond_to_user_request_ic_inv apply fastforce
+  using request_cleanup_ic_inv apply fastforce
+  using request_cleanup_expired_ic_inv apply fastforce
+  using canister_out_of_cycles_ic_inv apply fastforce
+  using canister_time_progress_ic_inv apply fastforce
+  using cycle_consumption_ic_inv apply fastforce
+  using system_time_progress_ic_inv apply fastforce
+  done
 
 end
 
@@ -795,6 +2820,32 @@ export_code request_submission_pre request_submission_post
   message_execution_pre message_execution_post
   call_context_starvation_pre call_context_starvation_post
   call_context_removal_pre call_context_removal_post
+  ic_canister_creation_pre ic_canister_creation_post
+  ic_update_settings_pre ic_update_settings_post
+  ic_canister_status_pre ic_canister_status_post
+  ic_code_installation_pre ic_code_installation_post
+  ic_code_upgrade_pre ic_code_upgrade_post
+  ic_code_uninstallation_pre ic_code_uninstallation_post
+  ic_canister_stop_running_pre ic_canister_stop_running_post
+  ic_canister_stop_stopping_pre ic_canister_stop_stopping_post
+  ic_canister_stop_done_stopping_pre ic_canister_stop_done_stopping_post
+  ic_canister_stop_stopped_pre ic_canister_stop_stopped_post
+  ic_canister_start_not_stopping_pre ic_canister_start_not_stopping_post
+  ic_canister_start_stopping_pre ic_canister_start_stopping_post
+  ic_canister_deletion_pre ic_canister_deletion_post
+  ic_depositing_cycles_pre ic_depositing_cycles_post
+  ic_random_numbers_pre ic_random_numbers_post
+  ic_provisional_canister_creation_pre ic_provisional_canister_creation_post
+  ic_top_up_canister_pre ic_top_up_canister_post
+  callback_invocation_not_deleted_pre callback_invocation_not_deleted_post
+  callback_invocation_deleted_pre callback_invocation_deleted_post
+  respond_to_user_request_pre respond_to_user_request_post
+  request_cleanup_pre request_cleanup_post
+  request_cleanup_expired_pre request_cleanup_expired_post
+  canister_out_of_cycles_pre canister_out_of_cycles_post
+  canister_time_progress_pre canister_time_progress_post
+  cycle_consumption_pre cycle_consumption_post
+  system_time_progress_pre system_time_progress_post
 in Haskell module_name IC file_prefix code
 
 end
